
{
    "@context": {
        "unece": "https://service.unece.org/trade/uncefact/vocabulary/unece#",
        "rdf": "http://www.w3.org/1999/02/22-rdf-syntax-ns#",
        "rdfs": "http://www.w3.org/2000/01/rdf-schema#",
        "schema": "http://schema.org/",
        "core": "https://service.unece.org/trade/uncefact/vocabulary/unece/core#",
        "cefact": "https://service.unece.org/trade/uncefact/vocabulary/cefact#",
        "xsd": "http://www.w3.org/2001/XMLSchema#"
    },
    "@graph": [
        {
            "@id": "core:FinancialIdentity",
            "@type": "rdfs:Class",
            "rdfs:comment": "A financial identification for an organization.",
            "rdfs:label": "FinancialIdentity",
            "unece:cefactElementMetadata": [
                {
                    "@id": "cefact:Financial_Identity.Details",
                    "@type": "unece:AggregateBIE",
                    "unece:cefactUNId": "UN01013217",
                    "rdfs:comment": "A financial identification for an organization."
                }
            ]
        },
        {
            "@id": "core:FinancingFinancialAccount",
            "@type": "rdfs:Class",
            "rdfs:comment": "A financial account used internally by a bank to manage the line of credit granted to financing requesting party.",
            "rdfs:label": "FinancingFinancialAccount",
            "unece:cefactElementMetadata": [
                {
                    "@id": "cefact:Financing_FinancialAccount.Details",
                    "@type": "unece:AggregateBIE",
                    "unece:cefactUNId": "UN01013253",
                    "rdfs:comment": "A financial account used internally by a bank to manage the line of credit granted to financing requesting party."
                }
            ]
        },
        {
            "@id": "core:FinancingRequestDocument",
            "@type": "rdfs:Class",
            "rdfs:comment": "The set of characteristics shared by all individual transactions grouped for this financing request document.",
            "rdfs:label": "FinancingRequestDocument",
            "unece:cefactElementMetadata": [
                {
                    "@id": "cefact:FinancingRequest_Document.Details",
                    "@type": "unece:AggregateBIE",
                    "unece:cefactUNId": "UN01013228",
                    "rdfs:comment": "The set of characteristics shared by all individual transactions grouped for this financing request document."
                }
            ]
        },
        {
            "@id": "core:FinancingRequestResultDocument",
            "@type": "rdfs:Class",
            "rdfs:comment": "A collection of data that reports the result of a financing request.",
            "rdfs:label": "FinancingRequestResultDocument",
            "unece:cefactElementMetadata": [
                {
                    "@id": "cefact:FinancingRequestResult_Document.Details",
                    "@type": "unece:AggregateBIE",
                    "unece:cefactUNId": "UN01013224",
                    "rdfs:comment": "A collection of data that reports the result of a financing request."
                }
            ]
        },
        {
            "@id": "core:FinancingSummaryDocument",
            "@type": "rdfs:Class",
            "rdfs:comment": "A collection of financing related data that provides an overview of key points.",
            "rdfs:label": "FinancingSummaryDocument",
            "unece:cefactElementMetadata": [
                {
                    "@id": "cefact:FinancingSummary_Document.Details",
                    "@type": "unece:AggregateBIE",
                    "unece:cefactUNId": "UN01013245",
                    "rdfs:comment": "A collection of financing related data that provides an overview of key points."
                }
            ]
        },
        {
            "@id": "core:InstalmentPayment",
            "@type": "rdfs:Class",
            "rdfs:comment": "A discharge of obligations in respect of funds or securities, transferred through one of several payments, between two or more parties.",
            "rdfs:label": "InstalmentPayment",
            "unece:cefactElementMetadata": [
                {
                    "@id": "cefact:Instalment_Payment.Details",
                    "@type": "unece:AggregateBIE",
                    "unece:cefactUNId": "UN01013272",
                    "rdfs:comment": "A discharge of obligations in respect of funds or securities, transferred through one of several payments, between two or more parties."
                }
            ]
        },
        {
            "@id": "core:LogisticsLocation",
            "@type": "rdfs:Class",
            "rdfs:comment": "A logistics related physical location or place.",
            "rdfs:label": "LogisticsLocation",
            "unece:cefactElementMetadata": [
                {
                    "@id": "cefact:Logistics_Location.Details",
                    "@type": "unece:AggregateBIE",
                    "unece:cefactUNId": "UN01003679",
                    "rdfs:comment": "A logistics related physical location or place."
                }
            ]
        },
        {
            "@id": "core:PersonIdentity",
            "@type": "rdfs:Class",
            "rdfs:comment": "Identification of a person.",
            "rdfs:label": "PersonIdentity",
            "unece:cefactElementMetadata": [
                {
                    "@id": "cefact:Person_Identity.Details",
                    "@type": "unece:AggregateBIE",
                    "unece:cefactUNId": "UN01013279",
                    "rdfs:comment": "Identification of a person."
                }
            ]
        },
        {
            "@id": "core:ProprietaryIdentity",
            "@type": "rdfs:Class",
            "rdfs:comment": "Proprietary information which uniquely identifies a person or organization.",
            "rdfs:label": "ProprietaryIdentity",
            "unece:cefactElementMetadata": [
                {
                    "@id": "cefact:Proprietary_Identity.Details",
                    "@type": "unece:AggregateBIE",
                    "unece:cefactUNId": "UN01013286",
                    "rdfs:comment": "Proprietary information which uniquely identifies a person or organization."
                }
            ]
        },
        {
            "@id": "core:Referenced_TransportEvent",
            "@type": "rdfs:Class",
            "rdfs:comment": "A referenced significant occurrence or happening during transport.",
            "rdfs:label": "Referenced_TransportEvent",
            "unece:cefactElementMetadata": [
                {
                    "@id": "cefact:Referenced_Transport_Event.Details",
                    "@type": "unece:AggregateBIE",
                    "unece:cefactUNId": "UN01010081",
                    "rdfs:comment": "A referenced significant occurrence or happening during transport."
                }
            ]
        },
        {
            "@id": "core:SupplyChainEvent",
            "@type": "rdfs:Class",
            "rdfs:comment": "A significant occurrence or happening in a supply chain.",
            "rdfs:label": "SupplyChainEvent",
            "unece:cefactElementMetadata": [
                {
                    "@id": "cefact:SupplyChain_Event.Details",
                    "@type": "unece:AggregateBIE",
                    "unece:cefactUNId": "UN01004291",
                    "rdfs:comment": "A significant occurrence or happening in a supply chain."
                }
            ]
        },
        {
            "@id": "core:TradeAddress",
            "@type": "rdfs:Class",
            "rdfs:comment": "The location at which a particular trade related organization or person may be found or reached.",
            "rdfs:label": "TradeAddress",
            "unece:cefactElementMetadata": [
                {
                    "@id": "cefact:Trade_Address.Details",
                    "@type": "unece:AggregateBIE",
                    "unece:cefactUNId": "UN01004533",
                    "rdfs:comment": "The location at which a particular trade related organization or person may be found or reached."
                }
            ]
        },
        {
            "@id": "core:TradeGeopoliticalRegion",
            "@type": "rdfs:Class",
            "rdfs:comment": "A collection of countries and/or economies united for trade purposes.",
            "rdfs:label": "TradeGeopoliticalRegion",
            "unece:cefactElementMetadata": [
                {
                    "@id": "cefact:Trade_GeopoliticalRegion.Details",
                    "@type": "unece:AggregateBIE",
                    "unece:cefactUNId": "UN01004587",
                    "rdfs:comment": "A collection of countries and/or economies united for trade purposes."
                }
            ]
        },
        {
            "@id": "core:TradeParty",
            "@type": "rdfs:Class",
            "rdfs:comment": "An individual, a group, or a body having a role in a trade business function.",
            "rdfs:label": "TradeParty",
            "unece:cefactElementMetadata": [
                {
                    "@id": "cefact:Trade_Party.Details",
                    "@type": "unece:AggregateBIE",
                    "unece:cefactUNId": "UN01004594",
                    "rdfs:comment": "An individual, a group, or a body having a role in a trade business function."
                }
            ]
        },
        {
            "@id": "core:TradePaymentDiscountTerms",
            "@type": "rdfs:Class",
            "rdfs:comment": "Trade terms and conditions by which a discount is or can be applied to a payable amount.",
            "rdfs:label": "TradePaymentDiscountTerms",
            "unece:cefactElementMetadata": [
                {
                    "@id": "cefact:Trade_PaymentDiscountTerms.Details",
                    "@type": "unece:AggregateBIE",
                    "unece:cefactUNId": "UN01004617",
                    "rdfs:comment": "Trade terms and conditions by which a discount is or can be applied to a payable amount."
                }
            ]
        },
        {
            "@id": "core:TradePaymentInstruction",
            "@type": "rdfs:Class",
            "rdfs:comment": "Instructions related to the processing of a trade payment.",
            "rdfs:label": "TradePaymentInstruction",
            "unece:cefactElementMetadata": [
                {
                    "@id": "cefact:Trade_PaymentInstruction.Details",
                    "@type": "unece:AggregateBIE",
                    "unece:cefactUNId": "UN01004622",
                    "rdfs:comment": "Instructions related to the processing of a trade payment."
                }
            ]
        },
        {
            "@id": "core:TradePaymentPenaltyTerms",
            "@type": "rdfs:Class",
            "rdfs:comment": "Trade terms and conditions by which a penalty is or can be applied to a payable amount.",
            "rdfs:label": "TradePaymentPenaltyTerms",
            "unece:cefactElementMetadata": [
                {
                    "@id": "cefact:Trade_PaymentPenaltyTerms.Details",
                    "@type": "unece:AggregateBIE",
                    "unece:cefactUNId": "UN01004626",
                    "rdfs:comment": "Trade terms and conditions by which a penalty is or can be applied to a payable amount."
                }
            ]
        },
        {
            "@id": "core:TradeSettlementFinancialCard",
            "@type": "rdfs:Class",
            "rdfs:comment": "A card used to represent a financial account for a trade settlement.",
            "rdfs:label": "TradeSettlementFinancialCard",
            "unece:cefactElementMetadata": [
                {
                    "@id": "cefact:TradeSettlement_FinancialCard.Details",
                    "@type": "unece:AggregateBIE",
                    "unece:cefactUNId": "UN01004493",
                    "rdfs:comment": "A card used to represent a financial account for a trade settlement."
                }
            ]
        },
        {
            "@id": "core:TradeSettlementPaymentMeans",
            "@type": "rdfs:Class",
            "rdfs:comment": "The means by which a payment will be or has been made for trade settlement purposes.",
            "rdfs:label": "TradeSettlementPaymentMeans",
            "unece:cefactElementMetadata": [
                {
                    "@id": "cefact:TradeSettlement_PaymentMeans.Details",
                    "@type": "unece:AggregateBIE",
                    "unece:cefactUNId": "UN01004512",
                    "rdfs:comment": "The means by which a payment will be or has been made for trade settlement purposes."
                }
            ]
        },
        {
            "@id": "core:TransportServiceLocation",
            "@type": "rdfs:Class",
            "rdfs:comment": "A location where a transport service takes place.",
            "rdfs:label": "TransportServiceLocation",
            "unece:cefactElementMetadata": [
                {
                    "@id": "cefact:TransportService_Location.Details",
                    "@type": "unece:AggregateBIE",
                    "unece:cefactUNId": "UN01010086",
                    "rdfs:comment": "A location where a transport service takes place."
                }
            ]
        },
        {
            "@id": "core:acceptedTransactionOriginalTotalAmount",
            "@type": "rdf:Property",
            "schema:rangeIncludes": {
                "@id": "xsd:decimal"
            },
            "schema:domainIncludes": {
                "@id": "core:FinancingSummaryDocument"
            },
            "rdfs:comment": "An original total monetary value of accepted transactions in this financing summary document.",
            "rdfs:label": "acceptedTransactionOriginalTotalAmount",
            "unece:cefactElementMetadata": [
                {
                    "@id": "cefact:FinancingSummary_Document.AcceptedTransactionOriginal_Total.Amount",
                    "@type": "unece:BasicBIE",
                    "unece:cefactUNId": "UN01013247",
                    "unece:cefactBieDomainClass": "cefact:FinancingSummary_Document.Details",
                    "rdfs:comment": "An original total monetary value of accepted transactions in this financing summary document."
                }
            ]
        },
        {
            "@id": "core:accountName",
            "@type": "rdf:Property",
            "schema:rangeIncludes": {
                "@id": "xsd:string"
            },
            "schema:domainIncludes": {
                "@id": "core:FinancingFinancialAccount"
            },
            "rdfs:comment": "The account name, expressed as text, of this financing financial account.",
            "rdfs:label": "accountName",
            "unece:cefactElementMetadata": [
                {
                    "@id": "cefact:Financing_FinancialAccount.AccountName.Text",
                    "@type": "unece:BasicBIE",
                    "unece:cefactUNId": "UN01013260",
                    "unece:cefactBieDomainClass": "cefact:Financing_FinancialAccount.Details",
                    "rdfs:comment": "The account name, expressed as text, of this financing financial account."
                }
            ]
        },
        {
            "@id": "core:activityAuthorizedParty",
            "@type": "rdf:Property",
            "schema:rangeIncludes": {
                "@id": "core:Party"
            },
            "schema:domainIncludes": {
                "@id": ":TradeCountrySubDivision"
            },
            "rdfs:comment": "A party that is authorized to perform an activity in this trade country sub-division.",
            "rdfs:label": "activityAuthorizedParty",
            "unece:cefactElementMetadata": [
                {
                    "@id": "cefact:Trade_CountrySub-Division.Activity_Authorized.Trade_Party",
                    "@type": "unece:AssociationBIE",
                    "unece:cefactUNId": "UN01004575",
                    "unece:cefactBieDomainClass": "cefact:Trade_CountrySubDivision.Details",
                    "rdfs:comment": "A party that is authorized to perform an activity in this trade country sub-division."
                }
            ]
        },
        {
            "@id": "core:actualArrivalRelatedDateTime",
            "@type": "rdf:Property",
            "schema:rangeIncludes": {
                "@id": "xsd:dateTime"
            },
            "schema:domainIncludes": {
                "@id": ":TransportEvent"
            },
            "rdfs:comment": "The date, time, date time or other date time value of the actual arrival related to this transport event.",
            "rdfs:label": "actualArrivalRelatedDateTime",
            "unece:cefactElementMetadata": [
                {
                    "@id": "cefact:Transport_Event.ActualArrival_Related.DateTime",
                    "@type": "unece:BasicBIE",
                    "unece:cefactUNId": "UN01010148",
                    "unece:cefactBieDomainClass": "cefact:Transport_Event.Details",
                    "rdfs:comment": "The date, time, date time or other date time value of the actual arrival related to this transport event."
                }
            ]
        },
        {
            "@id": "core:actualDepartureRelatedDateTime",
            "@type": "rdf:Property",
            "schema:rangeIncludes": {
                "@id": "xsd:dateTime"
            },
            "schema:domainIncludes": {
                "@id": ":TransportEvent"
            },
            "rdfs:comment": "The date, time, date time or other date time value of the actual departure related to this transport event.",
            "rdfs:label": "actualDepartureRelatedDateTime",
            "unece:cefactElementMetadata": [
                {
                    "@id": "cefact:Transport_Event.ActualDeparture_Related.DateTime",
                    "@type": "unece:BasicBIE",
                    "unece:cefactUNId": "UN01010150",
                    "unece:cefactBieDomainClass": "cefact:Transport_Event.Details",
                    "rdfs:comment": "The date, time, date time or other date time value of the actual departure related to this transport event."
                }
            ]
        },
        {
            "@id": "core:actualDiscountAmount",
            "@type": "rdf:Property",
            "schema:rangeIncludes": {
                "@id": "xsd:decimal"
            },
            "schema:domainIncludes": {
                "@id": "core:TradePaymentDiscountTerms"
            },
            "rdfs:comment": "A monetary value of the actual discount in these trade payment discount terms.",
            "rdfs:label": "actualDiscountAmount",
            "unece:cefactElementMetadata": [
                {
                    "@id": "cefact:Trade_PaymentDiscountTerms.ActualDiscount.Amount",
                    "@type": "unece:BasicBIE",
                    "unece:cefactUNId": "UN01004871",
                    "unece:cefactBieDomainClass": "cefact:Trade_PaymentDiscountTerms.Details",
                    "rdfs:comment": "A monetary value of the actual discount in these trade payment discount terms."
                }
            ]
        },
        {
            "@id": "core:actualOccurrencePeriod",
            "@type": "rdf:Property",
            "schema:rangeIncludes": {
                "@id": "core:Period"
            },
            "schema:domainIncludes": {
                "@id": ":TransportEvent"
            },
            "rdfs:comment": "The actual period of time during which this transport event occurred.",
            "rdfs:label": "actualOccurrencePeriod",
            "unece:cefactElementMetadata": [
                {
                    "@id": "cefact:Transport_Event.Actual_Occurrence.Specified_Period",
                    "@type": "unece:AssociationBIE",
                    "unece:cefactUNId": "UN01013589",
                    "unece:cefactBieDomainClass": "cefact:Transport_Event.Details",
                    "rdfs:comment": "The actual period of time during which this transport event occurred."
                }
            ]
        },
        {
            "@id": "core:actualPenaltyAmount",
            "@type": "rdf:Property",
            "schema:rangeIncludes": {
                "@id": "xsd:decimal"
            },
            "schema:domainIncludes": {
                "@id": "core:TradePaymentPenaltyTerms"
            },
            "rdfs:comment": "A monetary value of the actual penalty in these trade payment penalty terms.",
            "rdfs:label": "actualPenaltyAmount",
            "unece:cefactElementMetadata": [
                {
                    "@id": "cefact:Trade_PaymentPenaltyTerms.ActualPenalty.Amount",
                    "@type": "unece:BasicBIE",
                    "unece:cefactUNId": "UN01004872",
                    "unece:cefactBieDomainClass": "cefact:Trade_PaymentPenaltyTerms.Details",
                    "rdfs:comment": "A monetary value of the actual penalty in these trade payment penalty terms."
                }
            ]
        },
        {
            "@id": "core:actualStatus",
            "@type": "rdf:Property",
            "schema:rangeIncludes": {
                "@id": "core:Status"
            },
            "schema:domainIncludes": {
                "@id": "core:SupplyChainEvent"
            },
            "rdfs:comment": "The actual inspection status of this supply chain event.",
            "rdfs:label": "actualStatus",
            "unece:cefactElementMetadata": [
                {
                    "@id": "cefact:SupplyChain_Event.Actual.Inspection_Status",
                    "@type": "unece:AssociationBIE",
                    "unece:cefactUNId": "UN01013120",
                    "unece:cefactBieDomainClass": "cefact:SupplyChain_Event.Details",
                    "rdfs:comment": "The actual inspection status of this supply chain event."
                }
            ]
        },
        {
            "@id": "core:additionalClearingSystemId",
            "@type": "rdf:Property",
            "schema:rangeIncludes": {
                "@id": "xsd:token"
            },
            "schema:domainIncludes": {
                "@id": "accounting:CreditorFinancialInstitution"
            },
            "rdfs:comment": "An additional clearing system identifier for this creditor financial institution.",
            "rdfs:label": "additionalClearingSystemId",
            "unece:cefactElementMetadata": [
                {
                    "@id": "cefact:Creditor_FinancialInstitution.Additional_ClearingSystem.Identifier",
                    "@type": "unece:BasicBIE",
                    "unece:cefactUNId": "UN01013209",
                    "unece:cefactBieDomainClass": "cefact:Creditor_FinancialInstitution.Details",
                    "rdfs:comment": "An additional clearing system identifier for this creditor financial institution."
                }
            ]
        },
        {
            "@id": "core:additionalInformationIncludedNote",
            "@type": "rdf:Property",
            "schema:rangeIncludes": {
                "@id": "core:Note"
            },
            "schema:domainIncludes": {
                "@id": "core:FinancingRequestDocument"
            },
            "rdfs:comment": "An additional information note included for this financing request document.",
            "rdfs:label": "additionalInformationIncludedNote",
            "unece:cefactElementMetadata": [
                {
                    "@id": "cefact:FinancingRequest_Document.AdditionalInformation_Included.Note",
                    "@type": "unece:AssociationBIE",
                    "unece:cefactUNId": "UN01013244",
                    "unece:cefactBieDomainClass": "cefact:FinancingRequest_Document.Details",
                    "rdfs:comment": "An additional information note included for this financing request document."
                }
            ]
        },
        {
            "@id": "core:additionalSecurityMeasuresApplicableNote",
            "@type": "rdf:Property",
            "schema:rangeIncludes": {
                "@id": "core:Note"
            },
            "schema:domainIncludes": {
                "@id": ":TransportEvent"
            },
            "rdfs:comment": "A note providing additional security measures applicable to this transport event.",
            "rdfs:label": "additionalSecurityMeasuresApplicableNote",
            "unece:cefactElementMetadata": [
                {
                    "@id": "cefact:Transport_Event.AdditionalSecurityMeasures_Applicable.Note",
                    "@type": "unece:AssociationBIE",
                    "unece:cefactUNId": "UN01013133",
                    "unece:cefactBieDomainClass": "cefact:Transport_Event.Details",
                    "rdfs:comment": "A note providing additional security measures applicable to this transport event."
                }
            ]
        },
        {
            "@id": "core:addressTypeCode",
            "@type": "rdf:Property",
            "schema:rangeIncludes": {
                "@id": "unece:UNECECL3131Code"
            },
            "schema:domainIncludes": {
                "@id": "core:TradeAddress"
            },
            "rdfs:comment": "A code specifying the type of this trade address, such as business address or home address.",
            "rdfs:label": "addressTypeCode",
            "unece:cefactElementMetadata": [
                {
                    "@id": "cefact:Trade_Address.Type.Code",
                    "@type": "unece:BasicBIE",
                    "unece:TDED": "3131",
                    "unece:cefactUNId": "UN01013131",
                    "unece:cefactBieDomainClass": "cefact:Trade_Address.Details",
                    "rdfs:comment": "A code specifying the type of this trade address, such as business address or home address."
                }
            ]
        },
        {
            "@id": "core:agentAssignedCustomerId",
            "@type": "rdf:Property",
            "schema:rangeIncludes": {
                "@id": "xsd:token"
            },
            "schema:domainIncludes": {
                "@id": "core:FinancialIdentity"
            },
            "rdfs:comment": "The agent assigned customer identifier for this financial identity.",
            "rdfs:label": "agentAssignedCustomerId",
            "unece:cefactElementMetadata": [
                {
                    "@id": "cefact:Financial_Identity.AgentAssignedCustomer_Identification.Identifier",
                    "@type": "unece:BasicBIE",
                    "unece:cefactUNId": "UN01013222",
                    "unece:cefactBieDomainClass": "cefact:Financial_Identity.Details",
                    "rdfs:comment": "The agent assigned customer identifier for this financial identity."
                }
            ]
        },
        {
            "@id": "core:agreementInformation",
            "@type": "rdf:Property",
            "schema:rangeIncludes": {
                "@id": "xsd:string"
            },
            "schema:domainIncludes": {
                "@id": "core:FinancingRequestDocument"
            },
            "rdfs:comment": "Agreement information, expressed as text, in this financing request document, such as a collection mandate.",
            "rdfs:label": "agreementInformation",
            "unece:cefactElementMetadata": [
                {
                    "@id": "cefact:FinancingRequest_Document.Agreement_Information.Text",
                    "@type": "unece:BasicBIE",
                    "unece:TDED": "4142",
                    "unece:cefactUNId": "UN01013237",
                    "unece:cefactBieDomainClass": "cefact:FinancingRequest_Document.Details",
                    "rdfs:comment": "Agreement information, expressed as text, in this financing request document, such as a collection mandate."
                }
            ]
        },
        {
            "@id": "core:alienRegistrationId",
            "@type": "rdf:Property",
            "schema:rangeIncludes": {
                "@id": "xsd:token"
            },
            "schema:domainIncludes": {
                "@id": "core:PersonIdentity"
            },
            "rdfs:comment": "The alien registration identifier for this person.",
            "rdfs:label": "alienRegistrationId",
            "unece:cefactElementMetadata": [
                {
                    "@id": "cefact:Person_Identity.AlienRegistration_Identification.Identifier",
                    "@type": "unece:BasicBIE",
                    "unece:cefactUNId": "UN01013284",
                    "unece:cefactBieDomainClass": "cefact:Person_Identity.Details",
                    "rdfs:comment": "The alien registration identifier for this person."
                }
            ]
        },
        {
            "@id": "core:anchorageDescription",
            "@type": "rdf:Property",
            "schema:rangeIncludes": {
                "@id": "xsd:string"
            },
            "schema:domainIncludes": {
                "@id": ":TransportEvent"
            },
            "rdfs:comment": "A textual description of an anchorage for this transport event.",
            "rdfs:label": "anchorageDescription",
            "unece:cefactElementMetadata": [
                {
                    "@id": "cefact:Transport_Event.Anchorage_Description.Text",
                    "@type": "unece:BasicBIE",
                    "unece:cefactUNId": "UN01015102",
                    "unece:cefactBieDomainClass": "cefact:Transport_Event.Details",
                    "rdfs:comment": "A textual description of an anchorage for this transport event."
                }
            ]
        },
        {
            "@id": "core:anchorageExpectedIndicator",
            "@type": "rdf:Property",
            "schema:rangeIncludes": {
                "@id": "xsd:boolean"
            },
            "schema:domainIncludes": {
                "@id": ":TransportEvent"
            },
            "rdfs:comment": "The indication of whether or not this anchorage transport event is or was expected.",
            "rdfs:label": "anchorageExpectedIndicator",
            "unece:cefactElementMetadata": [
                {
                    "@id": "cefact:Transport_Event.Anchorage_Expected.Indicator",
                    "@type": "unece:BasicBIE",
                    "unece:cefactUNId": "UN01015104",
                    "unece:cefactBieDomainClass": "cefact:Transport_Event.Details",
                    "rdfs:comment": "The indication of whether or not this anchorage transport event is or was expected."
                }
            ]
        },
        {
            "@id": "core:applicableCertificate",
            "@type": "rdf:Property",
            "schema:rangeIncludes": {
                "@id": "core:Certificate"
            },
            "schema:domainIncludes": {
                "@id": "core:TradeParty"
            },
            "rdfs:comment": [
                "A process certificate applicable to this trade party.",
                "A product batch certificate applicable to this trade party.",
                "A product certificate applicable to this trade party.",
                "An organizational certificate applicable to this trade party."
            ],
            "rdfs:label": "applicableCertificate",
            "unece:cefactElementMetadata": [
                {
                    "@id": "cefact:Trade_Party.Applicable.ProductBatch_Certificate",
                    "@type": "unece:AssociationBIE",
                    "unece:cefactUNId": "UN01014539",
                    "unece:cefactBieDomainClass": "cefact:Trade_Party.Details",
                    "rdfs:comment": "A product batch certificate applicable to this trade party."
                },
                {
                    "@id": "cefact:Trade_Party.Applicable.Product_Certificate",
                    "@type": "unece:AssociationBIE",
                    "unece:cefactUNId": "UN01014540",
                    "unece:cefactBieDomainClass": "cefact:Trade_Party.Details",
                    "rdfs:comment": "A product certificate applicable to this trade party."
                },
                {
                    "@id": "cefact:Trade_Party.Applicable.Process_Certificate",
                    "@type": "unece:AssociationBIE",
                    "unece:cefactUNId": "UN01014538",
                    "unece:cefactBieDomainClass": "cefact:Trade_Party.Details",
                    "rdfs:comment": "A process certificate applicable to this trade party."
                },
                {
                    "@id": "cefact:Trade_Party.Applicable.Organizational_Certificate",
                    "@type": "unece:AssociationBIE",
                    "unece:cefactUNId": "UN01014541",
                    "unece:cefactBieDomainClass": "cefact:Trade_Party.Details",
                    "rdfs:comment": "An organizational certificate applicable to this trade party."
                }
            ]
        },
        {
            "@id": "core:applicableCertification",
            "@type": "rdf:Property",
            "schema:rangeIncludes": {
                "@id": "core:Certification"
            },
            "schema:domainIncludes": {
                "@id": "core:TradeParty"
            },
            "rdfs:comment": "An organizational certification applicable to this trade party.",
            "rdfs:label": "applicableCertification",
            "unece:cefactElementMetadata": [
                {
                    "@id": "cefact:Trade_Party.Applicable.Organizational_Certification",
                    "@type": "unece:AssociationBIE",
                    "unece:cefactUNId": "UN01014537",
                    "unece:cefactBieDomainClass": "cefact:Trade_Party.Details",
                    "rdfs:comment": "An organizational certification applicable to this trade party."
                }
            ]
        },
        {
            "@id": "core:applicableCharacteristic",
            "@type": "rdf:Property",
            "schema:rangeIncludes": {
                "@id": "core:Characteristic"
            },
            "schema:domainIncludes": {
                "@id": "core:TradeParty"
            },
            "rdfs:comment": [
                "A sustainability characteristic applicable to this trade party.",
                "A technical characteristic applicable to this trade party."
            ],
            "rdfs:label": "applicableCharacteristic",
            "unece:cefactElementMetadata": [
                {
                    "@id": "cefact:Trade_Party.Applicable.Sustainability_Characteristic",
                    "@type": "unece:AssociationBIE",
                    "unece:cefactUNId": "UN01014542",
                    "unece:cefactBieDomainClass": "cefact:Trade_Party.Details",
                    "rdfs:comment": "A sustainability characteristic applicable to this trade party."
                },
                {
                    "@id": "cefact:Trade_Party.Applicable.Technical_Characteristic",
                    "@type": "unece:AssociationBIE",
                    "unece:cefactUNId": "UN01014543",
                    "unece:cefactBieDomainClass": "cefact:Trade_Party.Details",
                    "rdfs:comment": "A technical characteristic applicable to this trade party."
                }
            ]
        },
        {
            "@id": "core:applicableDeclaration",
            "@type": "rdf:Property",
            "schema:rangeIncludes": {
                "@id": "core:Declaration"
            },
            "schema:domainIncludes": {
                "@id": "core:TradeParty"
            },
            "rdfs:comment": "A specified declaration applicable to this trade party.",
            "rdfs:label": "applicableDeclaration",
            "unece:cefactElementMetadata": [
                {
                    "@id": "cefact:Trade_Party.Applicable.Specified_Declaration",
                    "@type": "unece:AssociationBIE",
                    "unece:cefactUNId": "UN01015037",
                    "unece:cefactBieDomainClass": "cefact:Trade_Party.Details",
                    "rdfs:comment": "A specified declaration applicable to this trade party."
                }
            ]
        },
        {
            "@id": "core:applicableFinancialCard",
            "@type": "rdf:Property",
            "schema:rangeIncludes": {
                "@id": "core:FinancialCard"
            },
            "schema:domainIncludes": {
                "@id": "core:TradeSettlementPaymentMeans"
            },
            "rdfs:comment": "A financial card applicable to this trade settlement payment means.",
            "rdfs:label": "applicableFinancialCard",
            "unece:cefactElementMetadata": [
                {
                    "@id": "cefact:TradeSettlement_PaymentMeans.Applicable.TradeSettlement_FinancialCard",
                    "@type": "unece:AssociationBIE",
                    "unece:cefactUNId": "UN01004517",
                    "unece:cefactBieDomainClass": "cefact:TradeSettlement_PaymentMeans.Details",
                    "rdfs:comment": "A financial card applicable to this trade settlement payment means."
                }
            ]
        },
        {
            "@id": "core:applicableIndicator",
            "@type": "rdf:Property",
            "schema:rangeIncludes": {
                "@id": "xsd:boolean"
            },
            "schema:domainIncludes": {
                "@id": "core:TradeSettlementFinancialCard"
            },
            "rdfs:comment": "The indication of whether or not this trade settlement financial card is applicable.",
            "rdfs:label": "applicableIndicator",
            "unece:cefactElementMetadata": [
                {
                    "@id": "cefact:TradeSettlement_FinancialCard.Applicable.Indicator",
                    "@type": "unece:BasicBIE",
                    "unece:cefactUNId": "UN01015457",
                    "unece:cefactBieDomainClass": "cefact:TradeSettlement_FinancialCard.Details",
                    "rdfs:comment": "The indication of whether or not this trade settlement financial card is applicable."
                }
            ]
        },
        {
            "@id": "core:applicableInspection",
            "@type": "rdf:Property",
            "schema:rangeIncludes": {
                "@id": "core:Inspection"
            },
            "schema:domainIncludes": {
                "@id": "core:TradeParty"
            },
            "rdfs:comment": [
                "A specified inspection applicable to this trade party.",
                "A sustainability inspection applicable to this trade party."
            ],
            "rdfs:label": "applicableInspection",
            "unece:cefactElementMetadata": [
                {
                    "@id": "cefact:Trade_Party.Applicable.Sustainability_Inspection",
                    "@type": "unece:AssociationBIE",
                    "unece:cefactUNId": "UN01014548",
                    "unece:cefactBieDomainClass": "cefact:Trade_Party.Details",
                    "rdfs:comment": "A sustainability inspection applicable to this trade party."
                },
                {
                    "@id": "cefact:Trade_Party.Applicable.Specified_Inspection",
                    "@type": "unece:AssociationBIE",
                    "unece:cefactUNId": "UN01014547",
                    "unece:cefactBieDomainClass": "cefact:Trade_Party.Details",
                    "rdfs:comment": "A specified inspection applicable to this trade party."
                }
            ]
        },
        {
            "@id": "core:applicableLicence",
            "@type": "rdf:Property",
            "schema:rangeIncludes": {
                "@id": "core:Licence"
            },
            "schema:domainIncludes": {
                "@id": "core:TradeParty"
            },
            "rdfs:comment": "A specified licence applicable to this trade party.",
            "rdfs:label": "applicableLicence",
            "unece:cefactElementMetadata": [
                {
                    "@id": "cefact:Trade_Party.Applicable.Specified_Licence",
                    "@type": "unece:AssociationBIE",
                    "unece:cefactUNId": "UN01015036",
                    "unece:cefactBieDomainClass": "cefact:Trade_Party.Details",
                    "rdfs:comment": "A specified licence applicable to this trade party."
                }
            ]
        },
        {
            "@id": "core:applicableNote",
            "@type": "rdf:Property",
            "schema:rangeIncludes": {
                "@id": "core:Note"
            },
            "schema:domainIncludes": {
                "@id": ":TransportEvent"
            },
            "rdfs:comment": "A note providing information applicable to this transport event.",
            "rdfs:label": "applicableNote",
            "unece:cefactElementMetadata": [
                {
                    "@id": "cefact:Transport_Event.Applicable.Note",
                    "@type": "unece:AssociationBIE",
                    "unece:cefactUNId": "UN01012582",
                    "unece:cefactBieDomainClass": "cefact:Transport_Event.Details",
                    "rdfs:comment": "A note providing information applicable to this transport event."
                }
            ]
        },
        {
            "@id": "core:applicablePaymentDiscountTerms",
            "@type": "rdf:Property",
            "schema:rangeIncludes": {
                "@id": "core:PaymentDiscountTerms"
            },
            "schema:domainIncludes": {
                "@id": ":TradePaymentTerms"
            },
            "rdfs:comment": "Trade payment discount terms applicable to these trade payment terms.",
            "rdfs:label": "applicablePaymentDiscountTerms",
            "unece:cefactElementMetadata": [
                {
                    "@id": "cefact:Trade_PaymentTerms.Applicable.Trade_PaymentDiscountTerms",
                    "@type": "unece:AssociationBIE",
                    "unece:cefactUNId": "UN01004640",
                    "unece:cefactBieDomainClass": "cefact:Trade_PaymentTerms.Details",
                    "rdfs:comment": "Trade payment discount terms applicable to these trade payment terms."
                }
            ]
        },
        {
            "@id": "core:applicablePaymentPenaltyTerms",
            "@type": "rdf:Property",
            "schema:rangeIncludes": {
                "@id": "core:PaymentPenaltyTerms"
            },
            "schema:domainIncludes": {
                "@id": ":TradePaymentTerms"
            },
            "rdfs:comment": "Trade payment penalty terms applicable to these trade payment terms.",
            "rdfs:label": "applicablePaymentPenaltyTerms",
            "unece:cefactElementMetadata": [
                {
                    "@id": "cefact:Trade_PaymentTerms.Applicable.Trade_PaymentPenaltyTerms",
                    "@type": "unece:AssociationBIE",
                    "unece:cefactUNId": "UN01004639",
                    "unece:cefactBieDomainClass": "cefact:Trade_PaymentTerms.Details",
                    "rdfs:comment": "Trade payment penalty terms applicable to these trade payment terms."
                }
            ]
        },
        {
            "@id": "core:applicableServiceCharge",
            "@type": "rdf:Property",
            "schema:rangeIncludes": {
                "@id": "core:ServiceCharge"
            },
            "schema:domainIncludes": {
                "@id": "core:TradeParty"
            },
            "rdfs:comment": "A logistics service charge applicable to this trade party.",
            "rdfs:label": "applicableServiceCharge",
            "unece:cefactElementMetadata": [
                {
                    "@id": "cefact:Trade_Party.Applicable.Logistics_ServiceCharge",
                    "@type": "unece:AssociationBIE",
                    "unece:cefactUNId": "UN01009008",
                    "unece:cefactBieDomainClass": "cefact:Trade_Party.Details",
                    "rdfs:comment": "A logistics service charge applicable to this trade party."
                }
            ]
        },
        {
            "@id": "core:associatedGeographicalFeature",
            "@type": "rdf:Property",
            "schema:rangeIncludes": {
                "@id": "core:GeographicalFeature"
            },
            "schema:domainIncludes": [
                {
                    "@id": "core:LogisticsLocation"
                },
                {
                    "@id": ":TransportEvent"
                }
            ],
            "rdfs:comment": [
                "A geographical feature associated with this logistics location.",
                "A geographical feature associated with this transport event."
            ],
            "rdfs:label": "associatedGeographicalFeature",
            "unece:cefactElementMetadata": [
                {
                    "@id": "cefact:Logistics_Location.Associated.Specified_GeographicalFeature",
                    "@type": "unece:AssociationBIE",
                    "unece:cefactUNId": "UN01013608",
                    "unece:cefactBieDomainClass": "cefact:Logistics_Location.Details",
                    "rdfs:comment": "A geographical feature associated with this logistics location."
                },
                {
                    "@id": "cefact:Transport_Event.Associated.Specified_GeographicalFeature",
                    "@type": "unece:AssociationBIE",
                    "unece:cefactUNId": "UN01013587",
                    "unece:cefactBieDomainClass": "cefact:Transport_Event.Details",
                    "rdfs:comment": "A geographical feature associated with this transport event."
                }
            ]
        },
        {
            "@id": "core:associatedParty",
            "@type": "rdf:Property",
            "schema:rangeIncludes": {
                "@id": "core:Party"
            },
            "schema:domainIncludes": {
                "@id": "core:TradeParty"
            },
            "rdfs:comment": "A party associated with this trade party, such as a local agent of a shipping line.",
            "rdfs:label": "associatedParty",
            "unece:cefactElementMetadata": [
                {
                    "@id": "cefact:Trade_Party.Associated.Trade_Party",
                    "@type": "unece:AssociationBIE",
                    "unece:cefactUNId": "UN01004609",
                    "unece:cefactBieDomainClass": "cefact:Trade_Party.Details",
                    "rdfs:comment": "A party associated with this trade party, such as a local agent of a shipping line."
                }
            ]
        },
        {
            "@id": "core:associatedReference",
            "@type": "rdf:Property",
            "schema:rangeIncludes": {
                "@id": "core:Reference"
            },
            "schema:domainIncludes": {
                "@id": "core:SupplyChainEvent"
            },
            "rdfs:comment": "A reference associated with this supply chain event.",
            "rdfs:label": "associatedReference",
            "unece:cefactElementMetadata": [
                {
                    "@id": "cefact:SupplyChain_Event.Associated.SupplyChain_Reference",
                    "@type": "unece:AssociationBIE",
                    "unece:cefactUNId": "UN01014986",
                    "unece:cefactBieDomainClass": "cefact:SupplyChain_Event.Details",
                    "rdfs:comment": "A reference associated with this supply chain event."
                }
            ]
        },
        {
            "@id": "core:attentionOf",
            "@type": "rdf:Property",
            "schema:rangeIncludes": {
                "@id": "xsd:string"
            },
            "schema:domainIncludes": {
                "@id": "core:TradeAddress"
            },
            "rdfs:comment": "The name, expressed as text, of a person or department in the organization to whom incoming mail is marked with words such as 'for the attention of' or 'FAO' or 'ATTN' for this trade address.",
            "rdfs:label": "attentionOf",
            "unece:cefactElementMetadata": [
                {
                    "@id": "cefact:Trade_Address.AttentionOf.Text",
                    "@type": "unece:BasicBIE",
                    "unece:cefactUNId": "UN01004550",
                    "unece:cefactBieDomainClass": "cefact:Trade_Address.Details",
                    "rdfs:comment": "The name, expressed as text, of a person or department in the organization to whom incoming mail is marked with words such as 'for the attention of' or 'FAO' or 'ATTN' for this trade address."
                }
            ]
        },
        {
            "@id": "core:australianSNId",
            "@type": "rdf:Property",
            "schema:rangeIncludes": {
                "@id": "xsd:token"
            },
            "schema:domainIncludes": {
                "@id": "accounting:CreditorFinancialInstitution"
            },
            "rdfs:comment": "The Australian Small Network (SN) identifier as assigned by the Australian Payments Clearing Association (APCA) for this creditor financial institution.",
            "rdfs:label": "australianSNId",
            "unece:cefactElementMetadata": [
                {
                    "@id": "cefact:Creditor_FinancialInstitution.AustralianSN_Identification.Identifier",
                    "@type": "unece:BasicBIE",
                    "unece:TDED": "3433",
                    "unece:cefactUNId": "UN01013208",
                    "unece:cefactBieDomainClass": "cefact:Creditor_FinancialInstitution.Details",
                    "rdfs:comment": "The Australian Small Network (SN) identifier as assigned by the Australian Payments Clearing Association (APCA) for this creditor financial institution."
                }
            ]
        },
        {
            "@id": "core:authorization",
            "@type": "rdf:Property",
            "schema:rangeIncludes": {
                "@id": "xsd:string"
            },
            "schema:domainIncludes": {
                "@id": "core:FinancingRequestDocument"
            },
            "rdfs:comment": "An authorization, expressed as text, for this financing request document.",
            "rdfs:label": "authorization",
            "unece:cefactElementMetadata": [
                {
                    "@id": "cefact:FinancingRequest_Document.Authorization.Text",
                    "@type": "unece:BasicBIE",
                    "unece:cefactUNId": "UN01013234",
                    "unece:cefactBieDomainClass": "cefact:FinancingRequest_Document.Details",
                    "rdfs:comment": "An authorization, expressed as text, for this financing request document."
                }
            ]
        },
        {
            "@id": "core:bBANId",
            "@type": "rdf:Property",
            "schema:rangeIncludes": {
                "@id": "xsd:token"
            },
            "schema:domainIncludes": {
                "@id": "core:FinancingFinancialAccount"
            },
            "rdfs:comment": "The unique Basic Bank Account Number (BBAN) identifier used as part of a National Account Numbering Scheme for this financing financial account.",
            "rdfs:label": "bBANId",
            "unece:cefactElementMetadata": [
                {
                    "@id": "cefact:Financing_FinancialAccount.BBAN_Identification.Identifier",
                    "@type": "unece:BasicBIE",
                    "unece:TDED": "3492",
                    "unece:cefactUNId": "UN01013255",
                    "unece:cefactBieDomainClass": "cefact:Financing_FinancialAccount.Details",
                    "rdfs:comment": "The unique Basic Bank Account Number (BBAN) identifier used as part of a National Account Numbering Scheme for this financing financial account."
                }
            ]
        },
        {
            "@id": "core:bEIId",
            "@type": "rdf:Property",
            "schema:rangeIncludes": {
                "@id": "xsd:token"
            },
            "schema:domainIncludes": [
                {
                    "@id": "core:FinancialIdentity"
                },
                {
                    "@id": ":RequestingParty"
                }
            ],
            "rdfs:comment": [
                "The Business Entity Identifier (BEI) as defined by ISO 9362 (Banking telecommunication messages, Bank Identifier Codes) for this financial identity.",
                "The unique Business Entity Identifier (BEI) as defined by ISO 9362 (Banking telecommunication messages, Bank Identifier Codes) for this requesting party."
            ],
            "rdfs:label": "bEIId",
            "unece:cefactElementMetadata": [
                {
                    "@id": "cefact:Financial_Identity.BEI_Identification.Identifier",
                    "@type": "unece:BasicBIE",
                    "unece:cefactUNId": "UN01013220",
                    "unece:cefactBieDomainClass": "cefact:Financial_Identity.Details",
                    "rdfs:comment": "The Business Entity Identifier (BEI) as defined by ISO 9362 (Banking telecommunication messages, Bank Identifier Codes) for this financial identity."
                },
                {
                    "@id": "cefact:Requesting_Party.BEI_Identification.Identifier",
                    "@type": "unece:BasicBIE",
                    "unece:TDED": "3039",
                    "unece:cefactUNId": "UN01013291",
                    "unece:cefactBieDomainClass": "cefact:Requesting_Party.Details",
                    "rdfs:comment": "The unique Business Entity Identifier (BEI) as defined by ISO 9362 (Banking telecommunication messages, Bank Identifier Codes) for this requesting party."
                }
            ]
        },
        {
            "@id": "core:bICId",
            "@type": "rdf:Property",
            "schema:rangeIncludes": {
                "@id": "xsd:token"
            },
            "schema:domainIncludes": {
                "@id": "core:FinancialIdentity"
            },
            "rdfs:comment": "The Bank Identifier Code (BIC) as defined by ISO 9362 (Banking telecommunication messages, Bank Identifier Codes) for this financial identity.",
            "rdfs:label": "bICId",
            "unece:cefactElementMetadata": [
                {
                    "@id": "cefact:Financial_Identity.BIC_Identification.Identifier",
                    "@type": "unece:BasicBIE",
                    "unece:cefactUNId": "UN01013218",
                    "unece:cefactBieDomainClass": "cefact:Financial_Identity.Details",
                    "rdfs:comment": "The Bank Identifier Code (BIC) as defined by ISO 9362 (Banking telecommunication messages, Bank Identifier Codes) for this financial identity."
                }
            ]
        },
        {
            "@id": "core:bankAssignedId",
            "@type": "rdf:Property",
            "schema:rangeIncludes": {
                "@id": "xsd:token"
            },
            "schema:domainIncludes": {
                "@id": "core:FinancialIdentity"
            },
            "rdfs:comment": "The bank assigned identifier for this financial identity.",
            "rdfs:label": "bankAssignedId",
            "unece:cefactElementMetadata": [
                {
                    "@id": "cefact:Financial_Identity.BankAssigned_Identification.Identifier",
                    "@type": "unece:BasicBIE",
                    "unece:cefactUNId": "UN01013223",
                    "unece:cefactBieDomainClass": "cefact:Financial_Identity.Details",
                    "rdfs:comment": "The bank assigned identifier for this financial identity."
                }
            ]
        },
        {
            "@id": "core:basisAmount",
            "@type": "rdf:Property",
            "schema:rangeIncludes": {
                "@id": "xsd:decimal"
            },
            "schema:domainIncludes": [
                {
                    "@id": "core:TradePaymentDiscountTerms"
                },
                {
                    "@id": "core:TradePaymentPenaltyTerms"
                }
            ],
            "rdfs:comment": [
                "A monetary value used as a basis to calculate the discount in these trade payment discount terms.",
                "A monetary value used as a basis to calculate these trade payment penalty terms."
            ],
            "rdfs:label": "basisAmount",
            "unece:cefactElementMetadata": [
                {
                    "@id": "cefact:Trade_PaymentPenaltyTerms.Basis.Amount",
                    "@type": "unece:BasicBIE",
                    "unece:cefactUNId": "UN01004629",
                    "unece:cefactBieDomainClass": "cefact:Trade_PaymentPenaltyTerms.Details",
                    "rdfs:comment": "A monetary value used as a basis to calculate these trade payment penalty terms."
                },
                {
                    "@id": "cefact:Trade_PaymentDiscountTerms.Basis.Amount",
                    "@type": "unece:BasicBIE",
                    "unece:cefactUNId": "UN01004620",
                    "unece:cefactBieDomainClass": "cefact:Trade_PaymentDiscountTerms.Details",
                    "rdfs:comment": "A monetary value used as a basis to calculate the discount in these trade payment discount terms."
                }
            ]
        },
        {
            "@id": "core:basisDateTime",
            "@type": "rdf:Property",
            "schema:rangeIncludes": {
                "@id": "xsd:dateTime"
            },
            "schema:domainIncludes": [
                {
                    "@id": "core:TradePaymentDiscountTerms"
                },
                {
                    "@id": "core:TradePaymentPenaltyTerms"
                }
            ],
            "rdfs:comment": [
                "The date, time, date time, or other date time value used as the basis to calculate the discount in the trade payment discount terms.",
                "The date, time, date time, or other date time value used as the basis to calculate these trade payment penalty terms."
            ],
            "rdfs:label": "basisDateTime",
            "unece:cefactElementMetadata": [
                {
                    "@id": "cefact:Trade_PaymentPenaltyTerms.Basis.DateTime",
                    "@type": "unece:BasicBIE",
                    "unece:cefactUNId": "UN01004627",
                    "unece:cefactBieDomainClass": "cefact:Trade_PaymentPenaltyTerms.Details",
                    "rdfs:comment": "The date, time, date time, or other date time value used as the basis to calculate these trade payment penalty terms."
                },
                {
                    "@id": "cefact:Trade_PaymentDiscountTerms.Basis.DateTime",
                    "@type": "unece:BasicBIE",
                    "unece:cefactUNId": "UN01004618",
                    "unece:cefactBieDomainClass": "cefact:Trade_PaymentDiscountTerms.Details",
                    "rdfs:comment": "The date, time, date time, or other date time value used as the basis to calculate the discount in the trade payment discount terms."
                }
            ]
        },
        {
            "@id": "core:basisPeriodMeasure",
            "@type": "rdf:Property",
            "schema:rangeIncludes": {
                "@id": "xsd:decimal"
            },
            "schema:domainIncludes": [
                {
                    "@id": "core:TradePaymentDiscountTerms"
                },
                {
                    "@id": "core:TradePaymentPenaltyTerms"
                }
            ],
            "rdfs:comment": [
                "The measure of the basis period for these trade payment discount terms.",
                "The measure of the period used as a basis to calculate these trade payment penalty terms."
            ],
            "rdfs:label": "basisPeriodMeasure",
            "unece:cefactElementMetadata": [
                {
                    "@id": "cefact:Trade_PaymentDiscountTerms.BasisPeriod.Measure",
                    "@type": "unece:BasicBIE",
                    "unece:cefactUNId": "UN01004619",
                    "unece:cefactBieDomainClass": "cefact:Trade_PaymentDiscountTerms.Details",
                    "rdfs:comment": "The measure of the basis period for these trade payment discount terms."
                },
                {
                    "@id": "cefact:Trade_PaymentPenaltyTerms.BasisPeriod.Measure",
                    "@type": "unece:BasicBIE",
                    "unece:cefactUNId": "UN01004628",
                    "unece:cefactBieDomainClass": "cefact:Trade_PaymentPenaltyTerms.Details",
                    "rdfs:comment": "The measure of the period used as a basis to calculate these trade payment penalty terms."
                }
            ]
        },
        {
            "@id": "core:brandName",
            "@type": "rdf:Property",
            "schema:rangeIncludes": {
                "@id": "xsd:string"
            },
            "schema:domainIncludes": {
                "@id": "core:TradeParty"
            },
            "rdfs:comment": "The brand name, expressed as text, for this trade party.",
            "rdfs:label": "brandName",
            "unece:cefactElementMetadata": [
                {
                    "@id": "cefact:Trade_Party.Brand_Name.Text",
                    "@type": "unece:BasicBIE",
                    "unece:TDED": "3036",
                    "unece:cefactUNId": "UN01014533",
                    "unece:cefactBieDomainClass": "cefact:Trade_Party.Details",
                    "rdfs:comment": "The brand name, expressed as text, for this trade party."
                }
            ]
        },
        {
            "@id": "core:buildingName",
            "@type": "rdf:Property",
            "schema:rangeIncludes": {
                "@id": "xsd:string"
            },
            "schema:domainIncludes": {
                "@id": "core:TradeAddress"
            },
            "rdfs:comment": "The name, expressed as text, of a building, a house or other structure on a street at this trade address.",
            "rdfs:label": "buildingName",
            "unece:cefactElementMetadata": [
                {
                    "@id": "cefact:Trade_Address.BuildingName.Text",
                    "@type": "unece:BasicBIE",
                    "unece:cefactUNId": "UN01004537",
                    "unece:cefactBieDomainClass": "cefact:Trade_Address.Details",
                    "rdfs:comment": "The name, expressed as text, of a building, a house or other structure on a street at this trade address."
                }
            ]
        },
        {
            "@id": "core:buildingNumber",
            "@type": "rdf:Property",
            "schema:rangeIncludes": {
                "@id": "xsd:string"
            },
            "schema:domainIncludes": {
                "@id": "core:TradeAddress"
            },
            "rdfs:comment": "The building number, expressed as text, in this trade address.",
            "rdfs:label": "buildingNumber",
            "unece:cefactElementMetadata": [
                {
                    "@id": "cefact:Trade_Address.BuildingNumber.Text",
                    "@type": "unece:BasicBIE",
                    "unece:cefactUNId": "UN01006053",
                    "unece:cefactBieDomainClass": "cefact:Trade_Address.Details",
                    "rdfs:comment": "The building number, expressed as text, in this trade address."
                }
            ]
        },
        {
            "@id": "core:cAGEId",
            "@type": "rdf:Property",
            "schema:rangeIncludes": {
                "@id": "xsd:token"
            },
            "schema:domainIncludes": {
                "@id": "core:TradeParty"
            },
            "rdfs:comment": "The unique Commercial And Government Entity (CAGE) identifier for this trade party.",
            "rdfs:label": "cAGEId",
            "unece:cefactElementMetadata": [
                {
                    "@id": "cefact:Trade_Party.CAGE_Identification.Identifier",
                    "@type": "unece:BasicBIE",
                    "unece:TDED": "3039",
                    "unece:cefactUNId": "UN01006089",
                    "unece:cefactBieDomainClass": "cefact:Trade_Party.Details",
                    "rdfs:comment": "The unique Commercial And Government Entity (CAGE) identifier for this trade party."
                }
            ]
        },
        {
            "@id": "core:cHIPSUniversalId",
            "@type": "rdf:Property",
            "schema:rangeIncludes": {
                "@id": "xsd:token"
            },
            "schema:domainIncludes": {
                "@id": "core:FinancialIdentity"
            },
            "rdfs:comment": "The (United States) Clearing House Interbank Payments System (CHIPS) Universal Identification (UID) as assigned by the New York Clearing House for this financial identity.",
            "rdfs:label": "cHIPSUniversalId",
            "unece:cefactElementMetadata": [
                {
                    "@id": "cefact:Financial_Identity.CHIPSUniversal_Identification.Identifier",
                    "@type": "unece:BasicBIE",
                    "unece:cefactUNId": "UN01013221",
                    "unece:cefactBieDomainClass": "cefact:Financial_Identity.Details",
                    "rdfs:comment": "The (United States) Clearing House Interbank Payments System (CHIPS) Universal Identification (UID) as assigned by the New York Clearing House for this financial identity."
                }
            ]
        },
        {
            "@id": "core:calculationPercent",
            "@type": "rdf:Property",
            "schema:rangeIncludes": {
                "@id": "xsd:decimal"
            },
            "schema:domainIncludes": [
                {
                    "@id": "core:TradePaymentDiscountTerms"
                },
                {
                    "@id": "core:TradePaymentPenaltyTerms"
                }
            ],
            "rdfs:comment": [
                "The percent applied to calculate these trade payment penalty terms.",
                "The percent used to calculate the discount in these trade payment discount terms."
            ],
            "rdfs:label": "calculationPercent",
            "unece:cefactElementMetadata": [
                {
                    "@id": "cefact:Trade_PaymentPenaltyTerms.Calculation.Percent",
                    "@type": "unece:BasicBIE",
                    "unece:cefactUNId": "UN01004630",
                    "unece:cefactBieDomainClass": "cefact:Trade_PaymentPenaltyTerms.Details",
                    "rdfs:comment": "The percent applied to calculate these trade payment penalty terms."
                },
                {
                    "@id": "cefact:Trade_PaymentDiscountTerms.Calculation.Percent",
                    "@type": "unece:BasicBIE",
                    "unece:TDED": "5056",
                    "unece:cefactUNId": "UN01004621",
                    "unece:cefactBieDomainClass": "cefact:Trade_PaymentDiscountTerms.Details",
                    "rdfs:comment": "The percent used to calculate the discount in these trade payment discount terms."
                }
            ]
        },
        {
            "@id": "core:cancellationReason",
            "@type": "rdf:Property",
            "schema:rangeIncludes": {
                "@id": "xsd:string"
            },
            "schema:domainIncludes": {
                "@id": "core:FinancingRequestDocument"
            },
            "rdfs:comment": "A cancellation reason, expressed as text, in this financing request document.",
            "rdfs:label": "cancellationReason",
            "unece:cefactElementMetadata": [
                {
                    "@id": "cefact:FinancingRequest_Document.CancellationReason.Text",
                    "@type": "unece:BasicBIE",
                    "unece:cefactUNId": "UN01013235",
                    "unece:cefactBieDomainClass": "cefact:FinancingRequest_Document.Details",
                    "rdfs:comment": "A cancellation reason, expressed as text, in this financing request document."
                }
            ]
        },
        {
            "@id": "core:cardholderName",
            "@type": "rdf:Property",
            "schema:rangeIncludes": {
                "@id": "xsd:string"
            },
            "schema:domainIncludes": {
                "@id": "core:TradeSettlementFinancialCard"
            },
            "rdfs:comment": "The cardholder name as it appears on this trade settlement financial card. This may include both an individual authorized to use the card as well as the organization that owns the card.",
            "rdfs:label": "cardholderName",
            "unece:cefactElementMetadata": [
                {
                    "@id": "cefact:TradeSettlement_FinancialCard.CardholderName.Text",
                    "@type": "unece:BasicBIE",
                    "unece:cefactUNId": "UN01004497",
                    "unece:cefactBieDomainClass": "cefact:TradeSettlement_FinancialCard.Details",
                    "rdfs:comment": "The cardholder name as it appears on this trade settlement financial card. This may include both an individual authorized to use the card as well as the organization that owns the card."
                }
            ]
        },
        {
            "@id": "core:careOf",
            "@type": "rdf:Property",
            "schema:rangeIncludes": {
                "@id": "xsd:string"
            },
            "schema:domainIncludes": {
                "@id": "core:TradeAddress"
            },
            "rdfs:comment": "The name, expressed as text, of a person or organization at this trade address to whom incoming mail is marked with words such as 'care of' or 'C/O'.",
            "rdfs:label": "careOf",
            "unece:cefactElementMetadata": [
                {
                    "@id": "cefact:Trade_Address.CareOf.Text",
                    "@type": "unece:BasicBIE",
                    "unece:cefactUNId": "UN01004551",
                    "unece:cefactBieDomainClass": "cefact:Trade_Address.Details",
                    "rdfs:comment": "The name, expressed as text, of a person or organization at this trade address to whom incoming mail is marked with words such as 'care of' or 'C/O'."
                }
            ]
        },
        {
            "@id": "core:cashAccountTypeCode",
            "@type": "rdf:Property",
            "schema:rangeIncludes": {
                "@id": "unece:UNECECL4437Code"
            },
            "schema:domainIncludes": {
                "@id": "core:FinancingFinancialAccount"
            },
            "rdfs:comment": "The code specifying the type of financing financial account.",
            "rdfs:label": "cashAccountTypeCode",
            "unece:cefactElementMetadata": [
                {
                    "@id": "cefact:Financing_FinancialAccount.Type.Code",
                    "@type": "unece:BasicBIE",
                    "unece:TDED": "4437",
                    "unece:cefactUNId": "UN01013257",
                    "unece:cefactBieDomainClass": "cefact:Financing_FinancialAccount.Details",
                    "rdfs:comment": "The code specifying the type of financing financial account."
                }
            ]
        },
        {
            "@id": "core:cityId",
            "@type": "rdf:Property",
            "schema:rangeIncludes": {
                "@id": "xsd:token"
            },
            "schema:domainIncludes": {
                "@id": "core:TradeAddress"
            },
            "rdfs:comment": "The identifier of the city for this trade address, such as United Nations Location Code (UNLOCODE).",
            "rdfs:label": "cityId",
            "unece:cefactElementMetadata": [
                {
                    "@id": "cefact:Trade_Address.City.Identifier",
                    "@type": "unece:BasicBIE",
                    "unece:cefactUNId": "UN01013130",
                    "unece:cefactBieDomainClass": "cefact:Trade_Address.Details",
                    "rdfs:comment": "The identifier of the city for this trade address, such as United Nations Location Code (UNLOCODE)."
                }
            ]
        },
        {
            "@id": "core:cityName",
            "@type": "rdf:Property",
            "schema:rangeIncludes": {
                "@id": "xsd:string"
            },
            "schema:domainIncludes": {
                "@id": "core:TradeAddress"
            },
            "rdfs:comment": "The name, expressed as text, of the city, town or village of this trade address.",
            "rdfs:label": "cityName",
            "unece:cefactElementMetadata": [
                {
                    "@id": "cefact:Trade_Address.CityName.Text",
                    "@type": "unece:BasicBIE",
                    "unece:TDED": "3164",
                    "unece:cefactUNId": "UN01004544",
                    "unece:cefactBieDomainClass": "cefact:Trade_Address.Details",
                    "rdfs:comment": "The name, expressed as text, of the city, town or village of this trade address."
                }
            ]
        },
        {
            "@id": "core:citySubDivisionName",
            "@type": "rdf:Property",
            "schema:rangeIncludes": {
                "@id": "xsd:string"
            },
            "schema:domainIncludes": {
                "@id": "core:TradeAddress"
            },
            "rdfs:comment": "A name, expressed as text, of a sub-division of a city for this trade address, for example a district or borough.",
            "rdfs:label": "citySubDivisionName",
            "unece:cefactElementMetadata": [
                {
                    "@id": "cefact:Trade_Address.CitySub-DivisionName.Text",
                    "@type": "unece:BasicBIE",
                    "unece:cefactUNId": "UN01004545",
                    "unece:cefactBieDomainClass": "cefact:Trade_Address.Details",
                    "rdfs:comment": "A name, expressed as text, of a sub-division of a city for this trade address, for example a district or borough."
                }
            ]
        },
        {
            "@id": "core:contractualClause",
            "@type": "rdf:Property",
            "schema:rangeIncludes": {
                "@id": "core:Clause"
            },
            "schema:domainIncludes": {
                "@id": "core:FinancingRequestDocument"
            },
            "rdfs:comment": "A contractual document clause specified for this financing request document.",
            "rdfs:label": "contractualClause",
            "unece:cefactElementMetadata": [
                {
                    "@id": "cefact:FinancingRequest_Document.Contractual.Document_Clause",
                    "@type": "unece:AssociationBIE",
                    "unece:cefactUNId": "UN01013243",
                    "unece:cefactBieDomainClass": "cefact:FinancingRequest_Document.Details",
                    "rdfs:comment": "A contractual document clause specified for this financing request document."
                }
            ]
        },
        {
            "@id": "core:copyIndicator",
            "@type": "rdf:Property",
            "schema:rangeIncludes": {
                "@id": "xsd:boolean"
            },
            "schema:domainIncludes": {
                "@id": "core:FinancingRequestDocument"
            },
            "rdfs:comment": "The indication of whether or not this financing request document is a copy rather than an original.",
            "rdfs:label": "copyIndicator",
            "unece:cefactElementMetadata": [
                {
                    "@id": "cefact:FinancingRequest_Document.Copy.Indicator",
                    "@type": "unece:BasicBIE",
                    "unece:cefactUNId": "UN01013233",
                    "unece:cefactBieDomainClass": "cefact:FinancingRequest_Document.Details",
                    "rdfs:comment": "The indication of whether or not this financing request document is a copy rather than an original."
                }
            ]
        },
        {
            "@id": "core:countryId",
            "@type": "rdf:Property",
            "schema:rangeIncludes": {
                "@id": "xsd:token"
            },
            "schema:domainIncludes": [
                {
                    "@id": "accounting:BirthAddress"
                },
                {
                    "@id": "core:TradeAddress"
                }
            ],
            "rdfs:comment": [
                "The identifier of a country for this birth address.",
                "The unique identifier of a country for this trade address."
            ],
            "rdfs:label": "countryId",
            "unece:cefactElementMetadata": [
                {
                    "@id": "cefact:Trade_Address.Country.Identifier",
                    "@type": "unece:BasicBIE",
                    "unece:TDED": "3207",
                    "unece:cefactUNId": "UN01004546",
                    "unece:cefactBieDomainClass": "cefact:Trade_Address.Details",
                    "rdfs:comment": "The unique identifier of a country for this trade address."
                },
                {
                    "@id": "cefact:Birth_Address.Country.Identifier",
                    "@type": "unece:BasicBIE",
                    "unece:cefactUNId": "UN01003172",
                    "unece:cefactBieDomainClass": "cefact:Birth_Address.Details",
                    "rdfs:comment": "The identifier of a country for this birth address."
                }
            ]
        },
        {
            "@id": "core:countryIdentificationCountry",
            "@type": "rdf:Property",
            "schema:rangeIncludes": {
                "@id": "core:Country"
            },
            "schema:domainIncludes": {
                "@id": "core:TradeAddress"
            },
            "rdfs:comment": "The unique identifier of the country for this trade address.",
            "rdfs:label": "countryIdentificationCountry",
            "unece:cefactElementMetadata": [
                {
                    "@id": "cefact:Trade_Address.CountryIdentification.Trade_Country",
                    "@type": "unece:AssociationBIE",
                    "unece:cefactUNId": "UN01004552",
                    "unece:cefactBieDomainClass": "cefact:Trade_Address.Details",
                    "rdfs:comment": "The unique identifier of the country for this trade address."
                }
            ]
        },
        {
            "@id": "core:countryName",
            "@type": "rdf:Property",
            "schema:rangeIncludes": {
                "@id": "xsd:string"
            },
            "schema:domainIncludes": {
                "@id": "core:TradeAddress"
            },
            "rdfs:comment": "A name, expressed as text, of the country for this trade address.",
            "rdfs:label": "countryName",
            "unece:cefactElementMetadata": [
                {
                    "@id": "cefact:Trade_Address.CountryName.Text",
                    "@type": "unece:BasicBIE",
                    "unece:cefactUNId": "UN01004547",
                    "unece:cefactBieDomainClass": "cefact:Trade_Address.Details",
                    "rdfs:comment": "A name, expressed as text, of the country for this trade address."
                }
            ]
        },
        {
            "@id": "core:countrySubDivisionId",
            "@type": "rdf:Property",
            "schema:rangeIncludes": {
                "@id": "xsd:token"
            },
            "schema:domainIncludes": [
                {
                    "@id": "core:LogisticsLocation"
                },
                {
                    "@id": "core:TradeAddress"
                }
            ],
            "rdfs:comment": [
                "A unique identifier of the country sub-division for this trade address.",
                "The identifier of the country sub-division for this logistics related location."
            ],
            "rdfs:label": "countrySubDivisionId",
            "unece:cefactElementMetadata": [
                {
                    "@id": "cefact:Logistics_Location.CountrySub-Division.Identifier",
                    "@type": "unece:BasicBIE",
                    "unece:cefactUNId": "UN01013369",
                    "unece:cefactBieDomainClass": "cefact:Logistics_Location.Details",
                    "rdfs:comment": "The identifier of the country sub-division for this logistics related location."
                },
                {
                    "@id": "cefact:Trade_Address.CountrySub-Division.Identifier",
                    "@type": "unece:BasicBIE",
                    "unece:TDED": "3229",
                    "unece:cefactUNId": "UN01004548",
                    "unece:cefactBieDomainClass": "cefact:Trade_Address.Details",
                    "rdfs:comment": "A unique identifier of the country sub-division for this trade address."
                }
            ]
        },
        {
            "@id": "core:countrySubDivisionName",
            "@type": "rdf:Property",
            "schema:rangeIncludes": {
                "@id": "xsd:string"
            },
            "schema:domainIncludes": {
                "@id": "core:TradeAddress"
            },
            "rdfs:comment": "A name, expressed as text, of the sub-division of a country for this trade address.",
            "rdfs:label": "countrySubDivisionName",
            "unece:cefactElementMetadata": [
                {
                    "@id": "cefact:Trade_Address.CountrySub-DivisionName.Text",
                    "@type": "unece:BasicBIE",
                    "unece:TDED": "3228",
                    "unece:cefactUNId": "UN01004549",
                    "unece:cefactBieDomainClass": "cefact:Trade_Address.Details",
                    "rdfs:comment": "A name, expressed as text, of the sub-division of a country for this trade address."
                }
            ]
        },
        {
            "@id": "core:creationDateTime",
            "@type": "rdf:Property",
            "schema:rangeIncludes": {
                "@id": "xsd:dateTime"
            },
            "schema:domainIncludes": [
                {
                    "@id": ":ExchangedDocument"
                },
                {
                    "@id": "core:FinancingRequestDocument"
                }
            ],
            "rdfs:comment": [
                "The date, time, date time or other date time value for the creation of this financing request document.",
                "The date, time, date time, or other date time value of a creation of this exchanged document."
            ],
            "rdfs:label": "creationDateTime",
            "unece:cefactElementMetadata": [
                {
                    "@id": "cefact:FinancingRequest_Document.Creation.DateTime",
                    "@type": "unece:BasicBIE",
                    "unece:cefactUNId": "UN01013232",
                    "unece:cefactBieDomainClass": "cefact:FinancingRequest_Document.Details",
                    "rdfs:comment": "The date, time, date time or other date time value for the creation of this financing request document."
                },
                {
                    "@id": "cefact:Exchanged_Document.Creation.DateTime",
                    "@type": "unece:BasicBIE",
                    "unece:cefactUNId": "UN01012584",
                    "unece:cefactBieDomainClass": "cefact:Exchanged_Document.Details",
                    "rdfs:comment": "The date, time, date time, or other date time value of a creation of this exchanged document."
                }
            ]
        },
        {
            "@id": "core:creditAvailableAmount",
            "@type": "rdf:Property",
            "schema:rangeIncludes": {
                "@id": "xsd:decimal"
            },
            "schema:domainIncludes": {
                "@id": "core:TradeSettlementFinancialCard"
            },
            "rdfs:comment": "A monetary value of the credit available for this trade settlement financial card.",
            "rdfs:label": "creditAvailableAmount",
            "unece:cefactElementMetadata": [
                {
                    "@id": "cefact:TradeSettlement_FinancialCard.CreditAvailable.Amount",
                    "@type": "unece:BasicBIE",
                    "unece:cefactUNId": "UN01006086",
                    "unece:cefactBieDomainClass": "cefact:TradeSettlement_FinancialCard.Details",
                    "rdfs:comment": "A monetary value of the credit available for this trade settlement financial card."
                }
            ]
        },
        {
            "@id": "core:creditLimitAmount",
            "@type": "rdf:Property",
            "schema:rangeIncludes": {
                "@id": "xsd:decimal"
            },
            "schema:domainIncludes": {
                "@id": "core:TradeSettlementFinancialCard"
            },
            "rdfs:comment": "A monetary value of the credit limit for this trade settlement financial card.",
            "rdfs:label": "creditLimitAmount",
            "unece:cefactElementMetadata": [
                {
                    "@id": "cefact:TradeSettlement_FinancialCard.CreditLimit.Amount",
                    "@type": "unece:BasicBIE",
                    "unece:cefactUNId": "UN01006085",
                    "unece:cefactBieDomainClass": "cefact:TradeSettlement_FinancialCard.Details",
                    "rdfs:comment": "A monetary value of the credit limit for this trade settlement financial card."
                }
            ]
        },
        {
            "@id": "core:creditorAgentInformation",
            "@type": "rdf:Property",
            "schema:rangeIncludes": {
                "@id": "xsd:string"
            },
            "schema:domainIncludes": {
                "@id": "core:TradePaymentInstruction"
            },
            "rdfs:comment": "Creditor agent information, expressed as text, for this trade payment instruction, such as processing information that may need to be acted upon by the creditor agent.",
            "rdfs:label": "creditorAgentInformation",
            "unece:cefactElementMetadata": [
                {
                    "@id": "cefact:Trade_PaymentInstruction.CreditorAgentInformation.Text",
                    "@type": "unece:BasicBIE",
                    "unece:cefactUNId": "UN01004624",
                    "unece:cefactBieDomainClass": "cefact:Trade_PaymentInstruction.Details",
                    "rdfs:comment": "Creditor agent information, expressed as text, for this trade payment instruction, such as processing information that may need to be acted upon by the creditor agent."
                }
            ]
        },
        {
            "@id": "core:creditorSpecifiedFinancialInstitution",
            "@type": "rdf:Property",
            "schema:rangeIncludes": {
                "@id": "core:FinancialInstitution"
            },
            "schema:domainIncludes": {
                "@id": "core:TradeSettlementPaymentMeans"
            },
            "rdfs:comment": "A creditor financial institution specified for this trade settlement payment means.",
            "rdfs:label": "creditorSpecifiedFinancialInstitution",
            "unece:cefactElementMetadata": [
                {
                    "@id": "cefact:TradeSettlement_PaymentMeans.Creditor_Specified.Payment_FinancialInstitution",
                    "@type": "unece:AssociationBIE",
                    "unece:cefactUNId": "UN01015460",
                    "unece:cefactBieDomainClass": "cefact:TradeSettlement_PaymentMeans.Details",
                    "rdfs:comment": "A creditor financial institution specified for this trade settlement payment means."
                }
            ]
        },
        {
            "@id": "core:currencyCode",
            "@type": "rdf:Property",
            "schema:rangeIncludes": {
                "@id": "xsd:token"
            },
            "schema:domainIncludes": [
                {
                    "@id": "core:FinancingFinancialAccount"
                },
                {
                    "@id": "core:FinancingRequestDocument"
                }
            ],
            "rdfs:comment": [
                "The code specifying the currency in this financing request document.",
                "The code specifying the currency of this financing financial account."
            ],
            "rdfs:label": "currencyCode",
            "unece:cefactElementMetadata": [
                {
                    "@id": "cefact:FinancingRequest_Document.Currency.Code",
                    "@type": "unece:BasicBIE",
                    "unece:TDED": "6345",
                    "unece:cefactUNId": "UN01013236",
                    "unece:cefactBieDomainClass": "cefact:FinancingRequest_Document.Details",
                    "rdfs:comment": "The code specifying the currency in this financing request document."
                },
                {
                    "@id": "cefact:Financing_FinancialAccount.Currency.Code",
                    "@type": "unece:BasicBIE",
                    "unece:cefactUNId": "UN01013259",
                    "unece:cefactBieDomainClass": "cefact:Financing_FinancialAccount.Details",
                    "rdfs:comment": "The code specifying the currency of this financing financial account."
                }
            ]
        },
        {
            "@id": "core:dODAACId",
            "@type": "rdf:Property",
            "schema:rangeIncludes": {
                "@id": "xsd:token"
            },
            "schema:domainIncludes": {
                "@id": "core:TradeParty"
            },
            "rdfs:comment": "The unique Department Of Defense Activity Address Code (DODAAC) identifier for this trade party.",
            "rdfs:label": "dODAACId",
            "unece:cefactElementMetadata": [
                {
                    "@id": "cefact:Trade_Party.DODAAC_Identification.Identifier",
                    "@type": "unece:BasicBIE",
                    "unece:TDED": "3039",
                    "unece:cefactUNId": "UN01006088",
                    "unece:cefactBieDomainClass": "cefact:Trade_Party.Details",
                    "rdfs:comment": "The unique Department Of Defense Activity Address Code (DODAAC) identifier for this trade party."
                }
            ]
        },
        {
            "@id": "core:dUNSId",
            "@type": "rdf:Property",
            "schema:rangeIncludes": {
                "@id": "xsd:token"
            },
            "schema:domainIncludes": {
                "@id": "core:TradeParty"
            },
            "rdfs:comment": "The unique nine-digit Data Universal Numbering System (DUNS) identifier for this trade party.",
            "rdfs:label": "dUNSId",
            "unece:cefactElementMetadata": [
                {
                    "@id": "cefact:Trade_Party.DUNS_Identification.Identifier",
                    "@type": "unece:BasicBIE",
                    "unece:TDED": "3039",
                    "unece:cefactUNId": "UN01006091",
                    "unece:cefactBieDomainClass": "cefact:Trade_Party.Details",
                    "rdfs:comment": "The unique nine-digit Data Universal Numbering System (DUNS) identifier for this trade party."
                }
            ]
        },
        {
            "@id": "core:debtorAgentInformation",
            "@type": "rdf:Property",
            "schema:rangeIncludes": {
                "@id": "xsd:string"
            },
            "schema:domainIncludes": {
                "@id": "core:TradePaymentInstruction"
            },
            "rdfs:comment": "Debtor agent information, expressed as text, for this trade payment instruction, such as processing information that may need to be acted upon by the debtor agent.",
            "rdfs:label": "debtorAgentInformation",
            "unece:cefactElementMetadata": [
                {
                    "@id": "cefact:Trade_PaymentInstruction.DebtorAgentInformation.Text",
                    "@type": "unece:BasicBIE",
                    "unece:cefactUNId": "UN01004625",
                    "unece:cefactBieDomainClass": "cefact:Trade_PaymentInstruction.Details",
                    "rdfs:comment": "Debtor agent information, expressed as text, for this trade payment instruction, such as processing information that may need to be acted upon by the debtor agent."
                }
            ]
        },
        {
            "@id": "core:debtorSpecifiedFinancialInstitution",
            "@type": "rdf:Property",
            "schema:rangeIncludes": {
                "@id": "core:FinancialInstitution"
            },
            "schema:domainIncludes": {
                "@id": "core:TradeSettlementPaymentMeans"
            },
            "rdfs:comment": "A debtor financial institution specified for this trade settlement payment means.",
            "rdfs:label": "debtorSpecifiedFinancialInstitution",
            "unece:cefactElementMetadata": [
                {
                    "@id": "cefact:TradeSettlement_PaymentMeans.Debtor_Specified.Payment_FinancialInstitution",
                    "@type": "unece:AssociationBIE",
                    "unece:cefactUNId": "UN01015459",
                    "unece:cefactBieDomainClass": "cefact:TradeSettlement_PaymentMeans.Details",
                    "rdfs:comment": "A debtor financial institution specified for this trade settlement payment means."
                }
            ]
        },
        {
            "@id": "core:definedContact",
            "@type": "rdf:Property",
            "schema:rangeIncludes": {
                "@id": "core:Contact"
            },
            "schema:domainIncludes": {
                "@id": "core:TradeParty"
            },
            "rdfs:comment": "A trade contact defined for this trade party.",
            "rdfs:label": "definedContact",
            "unece:cefactElementMetadata": [
                {
                    "@id": "cefact:Trade_Party.Defined.Trade_Contact",
                    "@type": "unece:AssociationBIE",
                    "unece:cefactUNId": "UN01004602",
                    "unece:cefactBieDomainClass": "cefact:Trade_Party.Details",
                    "rdfs:comment": "A trade contact defined for this trade party."
                }
            ]
        },
        {
            "@id": "core:delaySpecifiedEvent",
            "@type": "rdf:Property",
            "schema:rangeIncludes": {
                "@id": "core:Event"
            },
            "schema:domainIncludes": {
                "@id": ":TransportEvent"
            },
            "rdfs:comment": "A delay specified for this referenced transport event.",
            "rdfs:label": "delaySpecifiedEvent",
            "unece:cefactElementMetadata": [
                {
                    "@id": "cefact:Transport_Event.Delay_Specified.Referenced_Transport_Event",
                    "@type": "unece:AssociationBIE",
                    "unece:cefactUNId": "UN01010153",
                    "unece:cefactBieDomainClass": "cefact:Transport_Event.Details",
                    "rdfs:comment": "A delay specified for this referenced transport event."
                }
            ]
        },
        {
            "@id": "core:description",
            "@type": "rdf:Property",
            "schema:rangeIncludes": {
                "@id": "xsd:string"
            },
            "schema:domainIncludes": [
                {
                    "@id": "core:LogisticsLocation"
                },
                {
                    "@id": "core:SupplyChainEvent"
                },
                {
                    "@id": "core:TradeAddress"
                },
                {
                    "@id": "core:TradeParty"
                },
                {
                    "@id": ":TradePaymentTerms"
                }
            ],
            "rdfs:comment": [
                "A textual description of these trade payment terms.",
                "A textual description of this logistics related location.",
                "A textual description of this supply chain event.",
                "A textual description of this trade address.",
                "A textual description of this trade party."
            ],
            "rdfs:label": "description",
            "unece:cefactElementMetadata": [
                {
                    "@id": "cefact:Trade_Address.Description.Text",
                    "@type": "unece:BasicBIE",
                    "unece:cefactUNId": "UN01015408",
                    "unece:cefactBieDomainClass": "cefact:Trade_Address.Details",
                    "rdfs:comment": "A textual description of this trade address."
                },
                {
                    "@id": "cefact:SupplyChain_Event.Description.Text",
                    "@type": "unece:BasicBIE",
                    "unece:cefactUNId": "UN01004295",
                    "unece:cefactBieDomainClass": "cefact:SupplyChain_Event.Details",
                    "rdfs:comment": "A textual description of this supply chain event."
                },
                {
                    "@id": "cefact:Trade_Party.Description.Text",
                    "@type": "unece:BasicBIE",
                    "unece:cefactUNId": "UN01010146",
                    "unece:cefactBieDomainClass": "cefact:Trade_Party.Details",
                    "rdfs:comment": "A textual description of this trade party."
                },
                {
                    "@id": "cefact:Trade_PaymentTerms.Description.Text",
                    "@type": "unece:BasicBIE",
                    "unece:TDED": "4276",
                    "unece:cefactUNId": "UN01004631",
                    "unece:cefactBieDomainClass": "cefact:Trade_PaymentTerms.Details",
                    "rdfs:comment": "A textual description of these trade payment terms."
                },
                {
                    "@id": "cefact:Logistics_Location.Description.Text",
                    "@type": "unece:BasicBIE",
                    "unece:cefactUNId": "UN01003683",
                    "unece:cefactBieDomainClass": "cefact:Logistics_Location.Details",
                    "rdfs:comment": "A textual description of this logistics related location."
                }
            ]
        },
        {
            "@id": "core:descriptionBinaryObject",
            "@type": "rdf:Property",
            "schema:rangeIncludes": {
                "@id": "xsd:base64Binary"
            },
            "schema:domainIncludes": {
                "@id": "core:SupplyChainEvent"
            },
            "rdfs:comment": "Binary object data, such as a photograph, describing this supply chain event.",
            "rdfs:label": "descriptionBinaryObject",
            "unece:cefactElementMetadata": [
                {
                    "@id": "cefact:SupplyChain_Event.Description.BinaryObject",
                    "@type": "unece:BasicBIE",
                    "unece:cefactUNId": "UN01004296",
                    "unece:cefactBieDomainClass": "cefact:SupplyChain_Event.Details",
                    "rdfs:comment": "Binary object data, such as a photograph, describing this supply chain event."
                }
            ]
        },
        {
            "@id": "core:directTelephoneCommunication",
            "@type": "rdf:Property",
            "schema:rangeIncludes": {
                "@id": "core:Communication"
            },
            "schema:domainIncludes": {
                "@id": ":TradeContact"
            },
            "rdfs:comment": "The direct telephone communication information for this trade contact.",
            "rdfs:label": "directTelephoneCommunication",
            "unece:cefactElementMetadata": [
                {
                    "@id": "cefact:Trade_Contact.Direct_Telephone.Universal_Communication",
                    "@type": "unece:AssociationBIE",
                    "unece:cefactUNId": "UN01004565",
                    "unece:cefactBieDomainClass": "cefact:Trade_Contact.Details",
                    "rdfs:comment": "The direct telephone communication information for this trade contact."
                }
            ]
        },
        {
            "@id": "core:disembarkationDateTime",
            "@type": "rdf:Property",
            "schema:rangeIncludes": {
                "@id": "xsd:dateTime"
            },
            "schema:domainIncludes": {
                "@id": ":TransportPerson"
            },
            "rdfs:comment": "A date, time, date time, or other date time value that this person disembarked from a means of transport.",
            "rdfs:label": "disembarkationDateTime",
            "unece:cefactElementMetadata": [
                {
                    "@id": "cefact:Transport_Person.Disembarkation.DateTime",
                    "@type": "unece:BasicBIE",
                    "unece:cefactUNId": "UN01014804",
                    "unece:cefactBieDomainClass": "cefact:Transport_Person.Details",
                    "rdfs:comment": "A date, time, date time, or other date time value that this person disembarked from a means of transport."
                }
            ]
        },
        {
            "@id": "core:driversLicenceId",
            "@type": "rdf:Property",
            "schema:rangeIncludes": {
                "@id": "xsd:token"
            },
            "schema:domainIncludes": {
                "@id": "core:PersonIdentity"
            },
            "rdfs:comment": "The drivers licence identifier for this person.",
            "rdfs:label": "driversLicenceId",
            "unece:cefactElementMetadata": [
                {
                    "@id": "cefact:Person_Identity.DriversLicence_Identification.Identifier",
                    "@type": "unece:BasicBIE",
                    "unece:cefactUNId": "UN01013283",
                    "unece:cefactBieDomainClass": "cefact:Person_Identity.Details",
                    "rdfs:comment": "The drivers licence identifier for this person."
                }
            ]
        },
        {
            "@id": "core:dueDateTime",
            "@type": "rdf:Property",
            "schema:rangeIncludes": {
                "@id": "xsd:dateTime"
            },
            "schema:domainIncludes": [
                {
                    "@id": "core:InstalmentPayment"
                },
                {
                    "@id": "core:SupplyChainEvent"
                },
                {
                    "@id": ":TradePaymentTerms"
                }
            ],
            "rdfs:comment": [
                "The date, time, date time, or other date time value for a due date specified by these trade payment terms.",
                "The date, time, date time, or other date time value of the due date specified by these trade payment terms.",
                "The due date for this instalment payment.",
                "The due date, time, date time, or other date time value of this supply chain event."
            ],
            "rdfs:label": "dueDateTime",
            "unece:cefactElementMetadata": [
                {
                    "@id": "cefact:Trade_PaymentTerms.Due.DateTime",
                    "@type": "unece:BasicBIE",
                    "unece:cefactUNId": "UN01012587",
                    "unece:cefactBieDomainClass": "cefact:Trade_PaymentTerms.Details",
                    "rdfs:comment": "The date, time, date time, or other date time value of the due date specified by these trade payment terms."
                },
                {
                    "@id": "cefact:SupplyChain_Event.Due.DateTime",
                    "@type": "unece:BasicBIE",
                    "unece:cefactUNId": "UN01013373",
                    "unece:cefactBieDomainClass": "cefact:SupplyChain_Event.Details",
                    "rdfs:comment": "The due date, time, date time, or other date time value of this supply chain event."
                },
                {
                    "@id": "cefact:Instalment_Payment.Due.DateTime",
                    "@type": "unece:BasicBIE",
                    "unece:TDED": "2481",
                    "unece:cefactUNId": "UN01013275",
                    "unece:cefactBieDomainClass": "cefact:Instalment_Payment.Details",
                    "rdfs:comment": "The due date for this instalment payment."
                },
                {
                    "@id": "cefact:Trade_PaymentTerms.DueDate.DateTime",
                    "@type": "unece:BasicBIE",
                    "unece:cefactUNId": "UN01004632",
                    "unece:cefactBieDomainClass": "cefact:Trade_PaymentTerms.Details",
                    "rdfs:comment": "The date, time, date time, or other date time value for a due date specified by these trade payment terms."
                }
            ]
        },
        {
            "@id": "core:durationMeasure",
            "@type": "rdf:Property",
            "schema:rangeIncludes": {
                "@id": "xsd:decimal"
            },
            "schema:domainIncludes": {
                "@id": ":TradePaymentTerms"
            },
            "rdfs:comment": "The measure of a length of time duration specified for these trade payment terms, such as 12 hours, 15 days, 2 weeks, 3 months, 5 years.",
            "rdfs:label": "durationMeasure",
            "unece:cefactElementMetadata": [
                {
                    "@id": "cefact:Trade_PaymentTerms.Duration.Measure",
                    "@type": "unece:BasicBIE",
                    "unece:TDED": "6411",
                    "unece:cefactUNId": "UN01004633",
                    "unece:cefactBieDomainClass": "cefact:Trade_PaymentTerms.Details",
                    "rdfs:comment": "The measure of a length of time duration specified for these trade payment terms, such as 12 hours, 15 days, 2 weeks, 3 months, 5 years."
                }
            ]
        },
        {
            "@id": "core:eDICommunication",
            "@type": "rdf:Property",
            "schema:rangeIncludes": {
                "@id": "core:Communication"
            },
            "schema:domainIncludes": {
                "@id": ":TradeContact"
            },
            "rdfs:comment": "Electronic Data Interchange (EDI) communication information for this trade contact.",
            "rdfs:label": "eDICommunication",
            "unece:cefactElementMetadata": [
                {
                    "@id": "cefact:Trade_Contact.EDI.Universal_Communication",
                    "@type": "unece:AssociationBIE",
                    "unece:cefactUNId": "UN01010144",
                    "unece:cefactBieDomainClass": "cefact:Trade_Contact.Details",
                    "rdfs:comment": "Electronic Data Interchange (EDI) communication information for this trade contact."
                }
            ]
        },
        {
            "@id": "core:emailURICommunication",
            "@type": "rdf:Property",
            "schema:rangeIncludes": {
                "@id": "core:Communication"
            },
            "schema:domainIncludes": [
                {
                    "@id": ":TradeContact"
                },
                {
                    "@id": "core:TradeParty"
                }
            ],
            "rdfs:comment": [
                "The email URI communication information for this trade contact.",
                "The email communication for this trade party."
            ],
            "rdfs:label": "emailURICommunication",
            "unece:cefactElementMetadata": [
                {
                    "@id": "cefact:Trade_Party.Email_URI.Universal_Communication",
                    "@type": "unece:AssociationBIE",
                    "unece:cefactUNId": "UN01004607",
                    "unece:cefactBieDomainClass": "cefact:Trade_Party.Details",
                    "rdfs:comment": "The email communication for this trade party."
                },
                {
                    "@id": "cefact:Trade_Contact.Email_URI.Universal_Communication",
                    "@type": "unece:AssociationBIE",
                    "unece:cefactUNId": "UN01004569",
                    "unece:cefactBieDomainClass": "cefact:Trade_Contact.Details",
                    "rdfs:comment": "The email URI communication information for this trade contact."
                }
            ]
        },
        {
            "@id": "core:embarkationDateTime",
            "@type": "rdf:Property",
            "schema:rangeIncludes": {
                "@id": "xsd:dateTime"
            },
            "schema:domainIncludes": {
                "@id": ":TransportPerson"
            },
            "rdfs:comment": "A date, time, date time, or other date time value that this person embarked upon a means of transport.",
            "rdfs:label": "embarkationDateTime",
            "unece:cefactElementMetadata": [
                {
                    "@id": "cefact:Transport_Person.Embarkation.DateTime",
                    "@type": "unece:BasicBIE",
                    "unece:cefactUNId": "UN01014803",
                    "unece:cefactBieDomainClass": "cefact:Transport_Person.Details",
                    "rdfs:comment": "A date, time, date time, or other date time value that this person embarked upon a means of transport."
                }
            ]
        },
        {
            "@id": "core:endPointURICommunication",
            "@type": "rdf:Property",
            "schema:rangeIncludes": {
                "@id": "core:Communication"
            },
            "schema:domainIncludes": {
                "@id": "core:TradeParty"
            },
            "rdfs:comment": "The communication address of the end point URI for this trade party.",
            "rdfs:label": "endPointURICommunication",
            "unece:cefactElementMetadata": [
                {
                    "@id": "cefact:Trade_Party.EndPoint_URI.Universal_Communication",
                    "@type": "unece:AssociationBIE",
                    "unece:cefactUNId": "UN01004613",
                    "unece:cefactBieDomainClass": "cefact:Trade_Party.Details",
                    "rdfs:comment": "The communication address of the end point URI for this trade party."
                }
            ]
        },
        {
            "@id": "core:equivalentAmount",
            "@type": "rdf:Property",
            "schema:rangeIncludes": {
                "@id": "xsd:decimal"
            },
            "schema:domainIncludes": {
                "@id": ":TradePaymentTerms"
            },
            "rdfs:comment": "An equivalent monetary value to be transferred between debtor and creditor before deduction of charges for these trade payment terms, expressed in the currency of the debtor's account which is different from the currency in which it is to be transferred.",
            "rdfs:label": "equivalentAmount",
            "unece:cefactElementMetadata": [
                {
                    "@id": "cefact:Trade_PaymentTerms.Equivalent.Amount",
                    "@type": "unece:BasicBIE",
                    "unece:cefactUNId": "UN01004635",
                    "unece:cefactBieDomainClass": "cefact:Trade_PaymentTerms.Details",
                    "rdfs:comment": "An equivalent monetary value to be transferred between debtor and creditor before deduction of charges for these trade payment terms, expressed in the currency of the debtor's account which is different from the currency in which it is to be transferred."
                }
            ]
        },
        {
            "@id": "core:expectedIndicator",
            "@type": "rdf:Property",
            "schema:rangeIncludes": {
                "@id": "xsd:boolean"
            },
            "schema:domainIncludes": {
                "@id": ":TransportEvent"
            },
            "rdfs:comment": "The indication of whether or not this transport event is or was expected.",
            "rdfs:label": "expectedIndicator",
            "unece:cefactElementMetadata": [
                {
                    "@id": "cefact:Transport_Event.Expected.Indicator",
                    "@type": "unece:BasicBIE",
                    "unece:cefactUNId": "UN01013585",
                    "unece:cefactBieDomainClass": "cefact:Transport_Event.Details",
                    "rdfs:comment": "The indication of whether or not this transport event is or was expected."
                }
            ]
        },
        {
            "@id": "core:expiryDate",
            "@type": "rdf:Property",
            "schema:rangeIncludes": {
                "@id": "xsd:base64Binary"
            },
            "schema:domainIncludes": {
                "@id": "core:TradeSettlementFinancialCard"
            },
            "rdfs:comment": "The date of expiry up to which this trade settlement financial card is valid.",
            "rdfs:label": "expiryDate",
            "unece:cefactElementMetadata": [
                {
                    "@id": "cefact:TradeSettlement_FinancialCard.Expiry.Date",
                    "@type": "unece:BasicBIE",
                    "unece:cefactUNId": "UN01004498",
                    "unece:cefactBieDomainClass": "cefact:TradeSettlement_FinancialCard.Details",
                    "rdfs:comment": "The date of expiry up to which this trade settlement financial card is valid."
                }
            ]
        },
        {
            "@id": "core:expiryDateTime",
            "@type": "rdf:Property",
            "schema:rangeIncludes": {
                "@id": "xsd:dateTime"
            },
            "schema:domainIncludes": {
                "@id": "core:TradeSettlementFinancialCard"
            },
            "rdfs:comment": "The date of expiry up to which this trade settlement financial card is valid.",
            "rdfs:label": "expiryDateTime",
            "unece:cefactElementMetadata": [
                {
                    "@id": "cefact:TradeSettlement_FinancialCard.Expiry.DateTime",
                    "@type": "unece:BasicBIE",
                    "unece:cefactUNId": "UN01015456",
                    "unece:cefactBieDomainClass": "cefact:TradeSettlement_FinancialCard.Details",
                    "rdfs:comment": "The date of expiry up to which this trade settlement financial card is valid."
                }
            ]
        },
        {
            "@id": "core:facilityLocation",
            "@type": "rdf:Property",
            "schema:rangeIncludes": {
                "@id": "core:Location"
            },
            "schema:domainIncludes": {
                "@id": "core:LogisticsLocation"
            },
            "rdfs:comment": "A facility location referenced for this logistics location.",
            "rdfs:label": "facilityLocation",
            "unece:cefactElementMetadata": [
                {
                    "@id": "cefact:Logistics_Location.Facility.Referenced_Location",
                    "@type": "unece:AssociationBIE",
                    "unece:cefactUNId": "UN01014785",
                    "unece:cefactBieDomainClass": "cefact:Logistics_Location.Details",
                    "rdfs:comment": "A facility location referenced for this logistics location."
                }
            ]
        },
        {
            "@id": "core:faxCommunication",
            "@type": "rdf:Property",
            "schema:rangeIncludes": {
                "@id": "core:Communication"
            },
            "schema:domainIncludes": [
                {
                    "@id": ":TradeContact"
                },
                {
                    "@id": "core:TradeParty"
                }
            ],
            "rdfs:comment": [
                "A fax communication for this trade party.",
                "Fax communication information for this trade contact."
            ],
            "rdfs:label": "faxCommunication",
            "unece:cefactElementMetadata": [
                {
                    "@id": "cefact:Trade_Contact.Fax.Universal_Communication",
                    "@type": "unece:AssociationBIE",
                    "unece:cefactUNId": "UN01004567",
                    "unece:cefactBieDomainClass": "cefact:Trade_Contact.Details",
                    "rdfs:comment": "Fax communication information for this trade contact."
                },
                {
                    "@id": "cefact:Trade_Party.Fax.Universal_Communication",
                    "@type": "unece:AssociationBIE",
                    "unece:cefactUNId": "UN01004605",
                    "unece:cefactBieDomainClass": "cefact:Trade_Party.Details",
                    "rdfs:comment": "A fax communication for this trade party."
                }
            ]
        },
        {
            "@id": "core:financedAppliedRatePercent",
            "@type": "rdf:Property",
            "schema:rangeIncludes": {
                "@id": "xsd:decimal"
            },
            "schema:domainIncludes": {
                "@id": "core:FinancingSummaryDocument"
            },
            "rdfs:comment": "The financed applied rate, expressed as a percentage, in this financing summary document.",
            "rdfs:label": "financedAppliedRatePercent",
            "unece:cefactElementMetadata": [
                {
                    "@id": "cefact:FinancingSummary_Document.FinancedApplied_Rate.Percent",
                    "@type": "unece:BasicBIE",
                    "unece:cefactUNId": "UN01013249",
                    "unece:cefactBieDomainClass": "cefact:FinancingSummary_Document.Details",
                    "rdfs:comment": "The financed applied rate, expressed as a percentage, in this financing summary document."
                }
            ]
        },
        {
            "@id": "core:financedRatePercent",
            "@type": "rdf:Property",
            "schema:rangeIncludes": {
                "@id": "xsd:decimal"
            },
            "schema:domainIncludes": {
                "@id": "core:FinancingRequestResultDocument"
            },
            "rdfs:comment": "The financed rate, expressed as a percentage, in this financing request result document.",
            "rdfs:label": "financedRatePercent",
            "unece:cefactElementMetadata": [
                {
                    "@id": "cefact:FinancingRequestResult_Document.Financed_Rate.Percent",
                    "@type": "unece:BasicBIE",
                    "unece:cefactUNId": "UN01013226",
                    "unece:cefactBieDomainClass": "cefact:FinancingRequestResult_Document.Details",
                    "rdfs:comment": "The financed rate, expressed as a percentage, in this financing request result document."
                }
            ]
        },
        {
            "@id": "core:financedTotalAmount",
            "@type": "rdf:Property",
            "schema:rangeIncludes": {
                "@id": "xsd:decimal"
            },
            "schema:domainIncludes": [
                {
                    "@id": "core:FinancingRequestResultDocument"
                },
                {
                    "@id": "core:FinancingSummaryDocument"
                }
            ],
            "rdfs:comment": [
                "A financed total monetary value in this financing summary document.",
                "A monetary value of the financed total amount in this financing request result document."
            ],
            "rdfs:label": "financedTotalAmount",
            "unece:cefactElementMetadata": [
                {
                    "@id": "cefact:FinancingRequestResult_Document.Financed_Total.Amount",
                    "@type": "unece:BasicBIE",
                    "unece:cefactUNId": "UN01013225",
                    "unece:cefactBieDomainClass": "cefact:FinancingRequestResult_Document.Details",
                    "rdfs:comment": "A monetary value of the financed total amount in this financing request result document."
                },
                {
                    "@id": "cefact:FinancingSummary_Document.Financed_Total.Amount",
                    "@type": "unece:BasicBIE",
                    "unece:cefactUNId": "UN01013248",
                    "unece:cefactBieDomainClass": "cefact:FinancingSummary_Document.Details",
                    "rdfs:comment": "A financed total monetary value in this financing summary document."
                }
            ]
        },
        {
            "@id": "core:financedTransactionSpecifiedQuantity",
            "@type": "rdf:Property",
            "schema:rangeIncludes": {
                "@id": "xsd:decimal"
            },
            "schema:domainIncludes": {
                "@id": "core:FinancingSummaryDocument"
            },
            "rdfs:comment": "The number of financed transactions specified in this financing summary document.",
            "rdfs:label": "financedTransactionSpecifiedQuantity",
            "unece:cefactElementMetadata": [
                {
                    "@id": "cefact:FinancingSummary_Document.FinancedTransaction_Specified.Quantity",
                    "@type": "unece:BasicBIE",
                    "unece:cefactUNId": "UN01013246",
                    "unece:cefactBieDomainClass": "cefact:FinancingSummary_Document.Details",
                    "rdfs:comment": "The number of financed transactions specified in this financing summary document."
                }
            ]
        },
        {
            "@id": "core:firstAgentSpecifiedFinancialInstitution",
            "@type": "rdf:Property",
            "schema:rangeIncludes": {
                "@id": "core:FinancialInstitution"
            },
            "schema:domainIncludes": {
                "@id": "core:FinancingRequestDocument"
            },
            "rdfs:comment": "The creditor financial institution specified as the first agent in this financing request document.",
            "rdfs:label": "firstAgentSpecifiedFinancialInstitution",
            "unece:cefactElementMetadata": [
                {
                    "@id": "cefact:FinancingRequest_Document.FirstAgent_Specified.Creditor_FinancialInstitution",
                    "@type": "unece:AssociationBIE",
                    "unece:cefactUNId": "UN01013238",
                    "unece:cefactBieDomainClass": "cefact:FinancingRequest_Document.Details",
                    "rdfs:comment": "The creditor financial institution specified as the first agent in this financing request document."
                }
            ]
        },
        {
            "@id": "core:gLNId",
            "@type": "rdf:Property",
            "schema:rangeIncludes": {
                "@id": "xsd:token"
            },
            "schema:domainIncludes": {
                "@id": "core:TradeParty"
            },
            "rdfs:comment": "A Global Location Number (GLN) identifier for this trade party.",
            "rdfs:label": "gLNId",
            "unece:cefactElementMetadata": [
                {
                    "@id": "cefact:Trade_Party.GLN_Identification.Identifier",
                    "@type": "unece:BasicBIE",
                    "unece:TDED": "3039",
                    "unece:cefactUNId": "UN01006092",
                    "unece:cefactBieDomainClass": "cefact:Trade_Party.Details",
                    "rdfs:comment": "A Global Location Number (GLN) identifier for this trade party."
                }
            ]
        },
        {
            "@id": "core:geoCoordinateIdentificationGeographicalCoordinate",
            "@type": "rdf:Property",
            "schema:rangeIncludes": {
                "@id": "core:GeographicalCoordinate"
            },
            "schema:domainIncludes": {
                "@id": "core:TradeAddress"
            },
            "rdfs:comment": "An identification of a set of geographical coordinates for this trade address.",
            "rdfs:label": "geoCoordinateIdentificationGeographicalCoordinate",
            "unece:cefactElementMetadata": [
                {
                    "@id": "cefact:Trade_Address.Geo-CoordinateIdentification.GeographicalCoordinate",
                    "@type": "unece:AssociationBIE",
                    "unece:cefactUNId": "UN01004553",
                    "unece:cefactBieDomainClass": "cefact:Trade_Address.Details",
                    "rdfs:comment": "An identification of a set of geographical coordinates for this trade address."
                }
            ]
        },
        {
            "@id": "core:globalId",
            "@type": "rdf:Property",
            "schema:rangeIncludes": {
                "@id": "xsd:token"
            },
            "schema:domainIncludes": {
                "@id": "core:TradeParty"
            },
            "rdfs:comment": "A globally unique identifier of this trade party.",
            "rdfs:label": "globalId",
            "unece:cefactElementMetadata": [
                {
                    "@id": "cefact:Trade_Party.Global_Identification.Identifier",
                    "@type": "unece:BasicBIE",
                    "unece:TDED": "3039",
                    "unece:cefactUNId": "UN01004596",
                    "unece:cefactBieDomainClass": "cefact:Trade_Party.Details",
                    "rdfs:comment": "A globally unique identifier of this trade party."
                }
            ]
        },
        {
            "@id": "core:groupId",
            "@type": "rdf:Property",
            "schema:rangeIncludes": {
                "@id": "xsd:token"
            },
            "schema:domainIncludes": {
                "@id": "core:FinancingRequestDocument"
            },
            "rdfs:comment": "The group identifier in this financing request document.",
            "rdfs:label": "groupId",
            "unece:cefactElementMetadata": [
                {
                    "@id": "cefact:FinancingRequest_Document.Group_Identification.Identifier",
                    "@type": "unece:BasicBIE",
                    "unece:TDED": "1004",
                    "unece:cefactUNId": "UN01013229",
                    "unece:cefactBieDomainClass": "cefact:FinancingRequest_Document.Details",
                    "rdfs:comment": "The group identifier in this financing request document."
                }
            ]
        },
        {
            "@id": "core:groupedTransactionSpecifiedQuantity",
            "@type": "rdf:Property",
            "schema:rangeIncludes": {
                "@id": "xsd:decimal"
            },
            "schema:domainIncludes": {
                "@id": "core:FinancingRequestDocument"
            },
            "rdfs:comment": "The number of grouped transactions specified in this financing request document.",
            "rdfs:label": "groupedTransactionSpecifiedQuantity",
            "unece:cefactElementMetadata": [
                {
                    "@id": "cefact:FinancingRequest_Document.GroupedTransaction_Specified.Quantity",
                    "@type": "unece:BasicBIE",
                    "unece:cefactUNId": "UN01013230",
                    "unece:cefactBieDomainClass": "cefact:FinancingRequest_Document.Details",
                    "rdfs:comment": "The number of grouped transactions specified in this financing request document."
                }
            ]
        },
        {
            "@id": "core:groupedTransactionTotalAmount",
            "@type": "rdf:Property",
            "schema:rangeIncludes": {
                "@id": "xsd:decimal"
            },
            "schema:domainIncludes": {
                "@id": "core:FinancingRequestDocument"
            },
            "rdfs:comment": "A total monetary value of grouped transactions in this financing request document.",
            "rdfs:label": "groupedTransactionTotalAmount",
            "unece:cefactElementMetadata": [
                {
                    "@id": "cefact:FinancingRequest_Document.GroupedTransaction_Total.Amount",
                    "@type": "unece:BasicBIE",
                    "unece:cefactUNId": "UN01013231",
                    "unece:cefactBieDomainClass": "cefact:FinancingRequest_Document.Details",
                    "rdfs:comment": "A total monetary value of grouped transactions in this financing request document."
                }
            ]
        },
        {
            "@id": "core:healthAffectedAreaIndicator",
            "@type": "rdf:Property",
            "schema:rangeIncludes": {
                "@id": "xsd:boolean"
            },
            "schema:domainIncludes": {
                "@id": "core:LogisticsLocation"
            },
            "rdfs:comment": "The indication of whether or not this logistics location is in a health affected area.",
            "rdfs:label": "healthAffectedAreaIndicator",
            "unece:cefactElementMetadata": [
                {
                    "@id": "cefact:Logistics_Location.HealthAffectedArea.Indicator",
                    "@type": "unece:BasicBIE",
                    "unece:cefactUNId": "UN01013704",
                    "unece:cefactBieDomainClass": "cefact:Logistics_Location.Details",
                    "rdfs:comment": "The indication of whether or not this logistics location is in a health affected area."
                }
            ]
        },
        {
            "@id": "core:iBANId",
            "@type": "rdf:Property",
            "schema:rangeIncludes": {
                "@id": "xsd:token"
            },
            "schema:domainIncludes": {
                "@id": "core:FinancingFinancialAccount"
            },
            "rdfs:comment": "The unique International Bank Account Number (IBAN) identifier for this financing financial account.",
            "rdfs:label": "iBANId",
            "unece:cefactElementMetadata": [
                {
                    "@id": "cefact:Financing_FinancialAccount.IBAN_Identification.Identifier",
                    "@type": "unece:BasicBIE",
                    "unece:TDED": "3492",
                    "unece:cefactUNId": "UN01013254",
                    "unece:cefactBieDomainClass": "cefact:Financing_FinancialAccount.Details",
                    "rdfs:comment": "The unique International Bank Account Number (IBAN) identifier for this financing financial account."
                }
            ]
        },
        {
            "@id": "core:iBEIId",
            "@type": "rdf:Property",
            "schema:rangeIncludes": {
                "@id": "xsd:token"
            },
            "schema:domainIncludes": {
                "@id": "core:FinancialIdentity"
            },
            "rdfs:comment": "The International Business Entity Identifier (IBEI) for this financial identity.",
            "rdfs:label": "iBEIId",
            "unece:cefactElementMetadata": [
                {
                    "@id": "cefact:Financial_Identity.IBEI_Identification.Identifier",
                    "@type": "unece:BasicBIE",
                    "unece:cefactUNId": "UN01013219",
                    "unece:cefactBieDomainClass": "cefact:Financial_Identity.Details",
                    "rdfs:comment": "The International Business Entity Identifier (IBEI) for this financial identity."
                }
            ]
        },
        {
            "@id": "core:id",
            "@type": "rdf:Property",
            "schema:rangeIncludes": {
                "@id": "xsd:token"
            },
            "schema:domainIncludes": [
                {
                    "@id": "core:LogisticsLocation"
                },
                {
                    "@id": "core:ProprietaryIdentity"
                },
                {
                    "@id": "core:SupplyChainEvent"
                },
                {
                    "@id": "core:TradeAddress"
                },
                {
                    "@id": "core:TradeGeopoliticalRegion"
                },
                {
                    "@id": "core:TradeParty"
                },
                {
                    "@id": "core:TradeSettlementFinancialCard"
                },
                {
                    "@id": "core:TransportServiceLocation"
                }
            ],
            "rdfs:comment": [
                "A proprietary identifier.",
                "A unique identifier for this logistics related location, such as a United Nations Location Code (UNLOCODE) or GS1 Global Location Number (GLN).",
                "A unique identifier for this trade address.",
                "A unique identifier of this trade party.",
                "An identifier for this transport service location, such as a United Nations Location Code (UNLOCODE) or GS1 Global Location Number (GLN).",
                "The unique identifier for this supply chain event.",
                "The unique identifier for this trade geopolitical region.",
                "The unique identifier, commonly known as the card number, of this trade settlement financial card."
            ],
            "rdfs:label": "id",
            "unece:cefactElementMetadata": [
                {
                    "@id": "cefact:Proprietary_Identity.Identification.Identifier",
                    "@type": "unece:BasicBIE",
                    "unece:cefactUNId": "UN01013287",
                    "unece:cefactBieDomainClass": "cefact:Proprietary_Identity.Details",
                    "rdfs:comment": "A proprietary identifier."
                },
                {
                    "@id": "cefact:TradeSettlement_FinancialCard.Identification.Identifier",
                    "@type": "unece:BasicBIE",
                    "unece:cefactUNId": "UN01004495",
                    "unece:cefactBieDomainClass": "cefact:TradeSettlement_FinancialCard.Details",
                    "rdfs:comment": "The unique identifier, commonly known as the card number, of this trade settlement financial card."
                },
                {
                    "@id": "cefact:SupplyChain_Event.Identification.Identifier",
                    "@type": "unece:BasicBIE",
                    "unece:TDED": "1007",
                    "unece:cefactUNId": "UN01004292",
                    "unece:cefactBieDomainClass": "cefact:SupplyChain_Event.Details",
                    "rdfs:comment": "The unique identifier for this supply chain event."
                },
                {
                    "@id": "cefact:Trade_GeopoliticalRegion.Identification.Identifier",
                    "@type": "unece:BasicBIE",
                    "unece:cefactUNId": "UN01004588",
                    "unece:cefactBieDomainClass": "cefact:Trade_GeopoliticalRegion.Details",
                    "rdfs:comment": "The unique identifier for this trade geopolitical region."
                },
                {
                    "@id": "cefact:TransportService_Location.Identification.Identifier",
                    "@type": "unece:BasicBIE",
                    "unece:TDED": "3225",
                    "unece:cefactUNId": "UN01010087",
                    "unece:cefactBieDomainClass": "cefact:TransportService_Location.Details",
                    "rdfs:comment": "An identifier for this transport service location, such as a United Nations Location Code (UNLOCODE) or GS1 Global Location Number (GLN)."
                },
                {
                    "@id": "cefact:Trade_Address.Identification.Identifier",
                    "@type": "unece:BasicBIE",
                    "unece:cefactUNId": "UN01004534",
                    "unece:cefactBieDomainClass": "cefact:Trade_Address.Details",
                    "rdfs:comment": "A unique identifier for this trade address."
                },
                {
                    "@id": "cefact:Logistics_Location.Identification.Identifier",
                    "@type": "unece:BasicBIE",
                    "unece:TDED": "3225",
                    "unece:cefactUNId": "UN01003680",
                    "unece:cefactBieDomainClass": "cefact:Logistics_Location.Details",
                    "rdfs:comment": "A unique identifier for this logistics related location, such as a United Nations Location Code (UNLOCODE) or GS1 Global Location Number (GLN)."
                },
                {
                    "@id": "cefact:Trade_Party.Identification.Identifier",
                    "@type": "unece:BasicBIE",
                    "unece:TDED": "3039",
                    "unece:cefactUNId": "UN01004595",
                    "unece:cefactBieDomainClass": "cefact:Trade_Party.Details",
                    "rdfs:comment": "A unique identifier of this trade party."
                }
            ]
        },
        {
            "@id": "core:identificationType",
            "@type": "rdf:Property",
            "schema:rangeIncludes": {
                "@id": "xsd:string"
            },
            "schema:domainIncludes": {
                "@id": "core:ProprietaryIdentity"
            },
            "rdfs:comment": "An identifier type, expressed as text, for this proprietary identity.",
            "rdfs:label": "identificationType",
            "unece:cefactElementMetadata": [
                {
                    "@id": "cefact:Proprietary_Identity.Identification_Type.Text",
                    "@type": "unece:BasicBIE",
                    "unece:cefactUNId": "UN01013288",
                    "unece:cefactBieDomainClass": "cefact:Proprietary_Identity.Details",
                    "rdfs:comment": "An identifier type, expressed as text, for this proprietary identity."
                }
            ]
        },
        {
            "@id": "core:identifiedCash",
            "@type": "rdf:Property",
            "schema:rangeIncludes": {
                "@id": "core:Cash"
            },
            "schema:domainIncludes": {
                "@id": "core:TradeSettlementPaymentMeans"
            },
            "rdfs:comment": "A cash payment identified for this trade settlement payment means.",
            "rdfs:label": "identifiedCash",
            "unece:cefactElementMetadata": [
                {
                    "@id": "cefact:TradeSettlement_PaymentMeans.Identified.Payment_Cash",
                    "@type": "unece:AssociationBIE",
                    "unece:cefactUNId": "UN01015462",
                    "unece:cefactBieDomainClass": "cefact:TradeSettlement_PaymentMeans.Details",
                    "rdfs:comment": "A cash payment identified for this trade settlement payment means."
                }
            ]
        },
        {
            "@id": "core:identifiedCheque",
            "@type": "rdf:Property",
            "schema:rangeIncludes": {
                "@id": "core:Cheque"
            },
            "schema:domainIncludes": {
                "@id": "core:TradeSettlementPaymentMeans"
            },
            "rdfs:comment": "A cheque payment identified for this trade settlement payment means.",
            "rdfs:label": "identifiedCheque",
            "unece:cefactElementMetadata": [
                {
                    "@id": "cefact:TradeSettlement_PaymentMeans.Identified.Payment_Cheque",
                    "@type": "unece:AssociationBIE",
                    "unece:cefactUNId": "UN01015463",
                    "unece:cefactBieDomainClass": "cefact:TradeSettlement_PaymentMeans.Details",
                    "rdfs:comment": "A cheque payment identified for this trade settlement payment means."
                }
            ]
        },
        {
            "@id": "core:identifiedDigitalMethod",
            "@type": "rdf:Property",
            "schema:rangeIncludes": {
                "@id": "core:DigitalMethod"
            },
            "schema:domainIncludes": {
                "@id": "core:TradeSettlementPaymentMeans"
            },
            "rdfs:comment": "A digital payment method identified for this trade settlement payment means.",
            "rdfs:label": "identifiedDigitalMethod",
            "unece:cefactElementMetadata": [
                {
                    "@id": "cefact:TradeSettlement_PaymentMeans.Identified.Payment_DigitalMethod",
                    "@type": "unece:AssociationBIE",
                    "unece:cefactUNId": "UN01015461",
                    "unece:cefactBieDomainClass": "cefact:TradeSettlement_PaymentMeans.Details",
                    "rdfs:comment": "A digital payment method identified for this trade settlement payment means."
                }
            ]
        },
        {
            "@id": "core:identifiedStowaway",
            "@type": "rdf:Property",
            "schema:rangeIncludes": {
                "@id": "core:Stowaway"
            },
            "schema:domainIncludes": {
                "@id": ":TransportPerson"
            },
            "rdfs:comment": "A transport person identified as a found stowaway.",
            "rdfs:label": "identifiedStowaway",
            "unece:cefactElementMetadata": [
                {
                    "@id": "cefact:Transport_Person.Identified.Found_Stowaway",
                    "@type": "unece:AssociationBIE",
                    "unece:cefactUNId": "UN01014805",
                    "unece:cefactBieDomainClass": "cefact:Transport_Person.Details",
                    "rdfs:comment": "A transport person identified as a found stowaway."
                }
            ]
        },
        {
            "@id": "core:identifiedVoucher",
            "@type": "rdf:Property",
            "schema:rangeIncludes": {
                "@id": "core:Voucher"
            },
            "schema:domainIncludes": {
                "@id": "core:TradeSettlementPaymentMeans"
            },
            "rdfs:comment": "An experience item voucher identified for this trade settlement payment means.",
            "rdfs:label": "identifiedVoucher",
            "unece:cefactElementMetadata": [
                {
                    "@id": "cefact:TradeSettlement_PaymentMeans.Identified.ExperienceItem_Voucher",
                    "@type": "unece:AssociationBIE",
                    "unece:cefactUNId": "UN01015464",
                    "unece:cefactBieDomainClass": "cefact:TradeSettlement_PaymentMeans.Details",
                    "rdfs:comment": "An experience item voucher identified for this trade settlement payment means."
                }
            ]
        },
        {
            "@id": "core:identityCardId",
            "@type": "rdf:Property",
            "schema:rangeIncludes": {
                "@id": "xsd:token"
            },
            "schema:domainIncludes": {
                "@id": "core:PersonIdentity"
            },
            "rdfs:comment": "The identity card identifier for this person.",
            "rdfs:label": "identityCardId",
            "unece:cefactElementMetadata": [
                {
                    "@id": "cefact:Person_Identity.IdentityCard_Identification.Identifier",
                    "@type": "unece:BasicBIE",
                    "unece:cefactUNId": "UN01013282",
                    "unece:cefactBieDomainClass": "cefact:Person_Identity.Details",
                    "rdfs:comment": "The identity card identifier for this person."
                }
            ]
        },
        {
            "@id": "core:includedAmount",
            "@type": "rdf:Property",
            "schema:rangeIncludes": {
                "@id": "xsd:decimal"
            },
            "schema:domainIncludes": {
                "@id": ":ReferencedDocument"
            },
            "rdfs:comment": "A monetary value included in this referenced document.",
            "rdfs:label": "includedAmount",
            "unece:cefactElementMetadata": [
                {
                    "@id": "cefact:Referenced_Document.Included.Amount",
                    "@type": "unece:BasicBIE",
                    "unece:cefactUNId": "UN01013310",
                    "unece:cefactBieDomainClass": "cefact:Referenced_Document.Details",
                    "rdfs:comment": "A monetary value included in this referenced document."
                }
            ]
        },
        {
            "@id": "core:includedCountry",
            "@type": "rdf:Property",
            "schema:rangeIncludes": {
                "@id": "core:Country"
            },
            "schema:domainIncludes": {
                "@id": "core:TradeGeopoliticalRegion"
            },
            "rdfs:comment": "A country included in this trade geopolitical region.",
            "rdfs:label": "includedCountry",
            "unece:cefactElementMetadata": [
                {
                    "@id": "cefact:Trade_GeopoliticalRegion.Included.Trade_Country",
                    "@type": "unece:AssociationBIE",
                    "unece:cefactUNId": "UN01004591",
                    "unece:cefactBieDomainClass": "cefact:Trade_GeopoliticalRegion.Details",
                    "rdfs:comment": "A country included in this trade geopolitical region."
                }
            ]
        },
        {
            "@id": "core:includedTax",
            "@type": "rdf:Property",
            "schema:rangeIncludes": {
                "@id": "core:Tax"
            },
            "schema:domainIncludes": {
                "@id": ":AdvancePayment"
            },
            "rdfs:comment": "A tax included in this advance payment.",
            "rdfs:label": "includedTax",
            "unece:cefactElementMetadata": [
                {
                    "@id": "cefact:Advance_Payment.Included.Trade_Tax",
                    "@type": "unece:AssociationBIE",
                    "unece:cefactUNId": "UN01012134",
                    "unece:cefactBieDomainClass": "cefact:Advance_Payment.Details",
                    "rdfs:comment": "A tax included in this advance payment."
                }
            ]
        },
        {
            "@id": "core:information",
            "@type": "rdf:Property",
            "schema:rangeIncludes": {
                "@id": "xsd:string"
            },
            "schema:domainIncludes": {
                "@id": ":TradePaymentTerms"
            },
            "rdfs:comment": "Information, expressed as text, for these trade payment terms.",
            "rdfs:label": "information",
            "unece:cefactElementMetadata": [
                {
                    "@id": "cefact:Trade_PaymentTerms.Information.Text",
                    "@type": "unece:BasicBIE",
                    "unece:cefactUNId": "UN01004637",
                    "unece:cefactBieDomainClass": "cefact:Trade_PaymentTerms.Details",
                    "rdfs:comment": "Information, expressed as text, for these trade payment terms."
                }
            ]
        },
        {
            "@id": "core:informationTypeCode",
            "@type": "rdf:Property",
            "schema:rangeIncludes": {
                "@id": "xsd:token"
            },
            "schema:domainIncludes": {
                "@id": "core:TradePaymentInstruction"
            },
            "rdfs:comment": "The code specifying the type of information for this trade payment instruction, such as processing requirements.",
            "rdfs:label": "informationTypeCode",
            "unece:cefactElementMetadata": [
                {
                    "@id": "cefact:Trade_PaymentInstruction.InformationType.Code",
                    "@type": "unece:BasicBIE",
                    "unece:cefactUNId": "UN01004623",
                    "unece:cefactBieDomainClass": "cefact:Trade_PaymentInstruction.Details",
                    "rdfs:comment": "The code specifying the type of information for this trade payment instruction, such as processing requirements."
                }
            ]
        },
        {
            "@id": "core:inspectionEvent",
            "@type": "rdf:Property",
            "schema:rangeIncludes": {
                "@id": "core:Event"
            },
            "schema:domainIncludes": {
                "@id": "core:LogisticsLocation"
            },
            "rdfs:comment": "A supply chain inspection event at this logistics location.",
            "rdfs:label": "inspectionEvent",
            "unece:cefactElementMetadata": [
                {
                    "@id": "cefact:Logistics_Location.Inspection.SupplyChain_Event",
                    "@type": "unece:AssociationBIE",
                    "unece:cefactUNId": "UN01013121",
                    "unece:cefactBieDomainClass": "cefact:Logistics_Location.Details",
                    "rdfs:comment": "A supply chain inspection event at this logistics location."
                }
            ]
        },
        {
            "@id": "core:instantMessagingCommunication",
            "@type": "rdf:Property",
            "schema:rangeIncludes": {
                "@id": "core:Communication"
            },
            "schema:domainIncludes": {
                "@id": ":TradeContact"
            },
            "rdfs:comment": "Instant messaging communication information for this trade contact.",
            "rdfs:label": "instantMessagingCommunication",
            "unece:cefactElementMetadata": [
                {
                    "@id": "cefact:Trade_Contact.InstantMessaging.Universal_Communication",
                    "@type": "unece:AssociationBIE",
                    "unece:cefactUNId": "UN01004572",
                    "unece:cefactBieDomainClass": "cefact:Trade_Contact.Details",
                    "rdfs:comment": "Instant messaging communication information for this trade contact."
                }
            ]
        },
        {
            "@id": "core:instructedAmount",
            "@type": "rdf:Property",
            "schema:rangeIncludes": {
                "@id": "xsd:decimal"
            },
            "schema:domainIncludes": {
                "@id": ":TradePaymentTerms"
            },
            "rdfs:comment": "A monetary value that has been instructed to be transferred between debtor and creditor for these trade payment terms before deduction of charges.",
            "rdfs:label": "instructedAmount",
            "unece:cefactElementMetadata": [
                {
                    "@id": "cefact:Trade_PaymentTerms.Instructed.Amount",
                    "@type": "unece:BasicBIE",
                    "unece:cefactUNId": "UN01004636",
                    "unece:cefactBieDomainClass": "cefact:Trade_PaymentTerms.Details",
                    "rdfs:comment": "A monetary value that has been instructed to be transferred between debtor and creditor for these trade payment terms before deduction of charges."
                }
            ]
        },
        {
            "@id": "core:interestRatePercent",
            "@type": "rdf:Property",
            "schema:rangeIncludes": {
                "@id": "xsd:decimal"
            },
            "schema:domainIncludes": {
                "@id": "core:TradeSettlementFinancialCard"
            },
            "rdfs:comment": "The interest rate expressed as a percentage for this trade settlement financial card.",
            "rdfs:label": "interestRatePercent",
            "unece:cefactElementMetadata": [
                {
                    "@id": "cefact:TradeSettlement_FinancialCard.InterestRate.Percent",
                    "@type": "unece:BasicBIE",
                    "unece:cefactUNId": "UN01006087",
                    "unece:cefactBieDomainClass": "cefact:TradeSettlement_FinancialCard.Details",
                    "rdfs:comment": "The interest rate expressed as a percentage for this trade settlement financial card."
                }
            ]
        },
        {
            "@id": "core:intermediarySpecifiedFinancialInstitution",
            "@type": "rdf:Property",
            "schema:rangeIncludes": {
                "@id": "core:FinancialInstitution"
            },
            "schema:domainIncludes": {
                "@id": "core:FinancingRequestDocument"
            },
            "rdfs:comment": "The creditor financial institution specified as the intermediary in this financing request document.",
            "rdfs:label": "intermediarySpecifiedFinancialInstitution",
            "unece:cefactElementMetadata": [
                {
                    "@id": "cefact:FinancingRequest_Document.Intermediary_Specified.Creditor_FinancialInstitution",
                    "@type": "unece:AssociationBIE",
                    "unece:cefactUNId": "UN01013239",
                    "unece:cefactBieDomainClass": "cefact:FinancingRequest_Document.Details",
                    "rdfs:comment": "The creditor financial institution specified as the intermediary in this financing request document."
                }
            ]
        },
        {
            "@id": "core:invalidIndicator",
            "@type": "rdf:Property",
            "schema:rangeIncludes": {
                "@id": "xsd:boolean"
            },
            "schema:domainIncludes": {
                "@id": "core:TradeAddress"
            },
            "rdfs:comment": "The indication of whether or not this trade address is invalid.",
            "rdfs:label": "invalidIndicator",
            "unece:cefactElementMetadata": [
                {
                    "@id": "cefact:Trade_Address.Invalid.Indicator",
                    "@type": "unece:BasicBIE",
                    "unece:cefactUNId": "UN01015407",
                    "unece:cefactBieDomainClass": "cefact:Trade_Address.Details",
                    "rdfs:comment": "The indication of whether or not this trade address is invalid."
                }
            ]
        },
        {
            "@id": "core:issuedNotificationReferencedDocument",
            "@type": "rdf:Property",
            "schema:rangeIncludes": {
                "@id": "core:Document"
            },
            "schema:domainIncludes": {
                "@id": "core:TradeParty"
            },
            "rdfs:comment": "A referenced notification document issued to this trade party.",
            "rdfs:label": "issuedNotificationReferencedDocument",
            "unece:cefactElementMetadata": [
                {
                    "@id": "cefact:Trade_Party.IssuedNotification_Referenced.Referenced_Document",
                    "@type": "unece:AssociationBIE",
                    "unece:cefactUNId": "UN01004615",
                    "unece:cefactBieDomainClass": "cefact:Trade_Party.Details",
                    "rdfs:comment": "A referenced notification document issued to this trade party."
                }
            ]
        },
        {
            "@id": "core:issuerSpecifiedInstructions",
            "@type": "rdf:Property",
            "schema:rangeIncludes": {
                "@id": "core:Instructions"
            },
            "schema:domainIncludes": {
                "@id": ":ReferencedDocument"
            },
            "rdfs:comment": "Handling instructions specified by the issuer for this referenced document.",
            "rdfs:label": "issuerSpecifiedInstructions",
            "unece:cefactElementMetadata": [
                {
                    "@id": "cefact:Referenced_Document.Issuer_Specified.DocumentHandling_Instructions",
                    "@type": "unece:AssociationBIE",
                    "unece:cefactUNId": "UN01013650",
                    "unece:cefactBieDomainClass": "cefact:Referenced_Document.Details",
                    "rdfs:comment": "Handling instructions specified by the issuer for this referenced document."
                }
            ]
        },
        {
            "@id": "core:jobTitle",
            "@type": "rdf:Property",
            "schema:rangeIncludes": {
                "@id": "xsd:string"
            },
            "schema:domainIncludes": {
                "@id": ":TradeContact"
            },
            "rdfs:comment": "The job title, position or designation, expressed as text, of this trade contact within an organization, such as Director, Software Engineer, Purchasing Manager.",
            "rdfs:label": "jobTitle",
            "unece:cefactElementMetadata": [
                {
                    "@id": "cefact:Trade_Contact.JobTitle.Text",
                    "@type": "unece:BasicBIE",
                    "unece:cefactUNId": "UN01004561",
                    "unece:cefactBieDomainClass": "cefact:Trade_Contact.Details",
                    "rdfs:comment": "The job title, position or designation, expressed as text, of this trade contact within an organization, such as Director, Software Engineer, Purchasing Manager."
                }
            ]
        },
        {
            "@id": "core:languageCode",
            "@type": "rdf:Property",
            "schema:rangeIncludes": {
                "@id": "xsd:token"
            },
            "schema:domainIncludes": {
                "@id": "core:TradeParty"
            },
            "rdfs:comment": "A code specifying a language for this trade party.",
            "rdfs:label": "languageCode",
            "unece:cefactElementMetadata": [
                {
                    "@id": "cefact:Trade_Party.Language.Code",
                    "@type": "unece:BasicBIE",
                    "unece:TDED": "3453",
                    "unece:cefactUNId": "UN01009017",
                    "unece:cefactBieDomainClass": "cefact:Trade_Party.Details",
                    "rdfs:comment": "A code specifying a language for this trade party."
                }
            ]
        },
        {
            "@id": "core:lineFive",
            "@type": "rdf:Property",
            "schema:rangeIncludes": {
                "@id": "xsd:string"
            },
            "schema:domainIncludes": {
                "@id": "core:TradeAddress"
            },
            "rdfs:comment": "The fifth free form line, expressed as text, of this trade address.",
            "rdfs:label": "lineFive",
            "unece:cefactElementMetadata": [
                {
                    "@id": "cefact:Trade_Address.LineFive.Text",
                    "@type": "unece:BasicBIE",
                    "unece:TDED": "3286",
                    "unece:cefactUNId": "UN01004542",
                    "unece:cefactBieDomainClass": "cefact:Trade_Address.Details",
                    "rdfs:comment": "The fifth free form line, expressed as text, of this trade address."
                }
            ]
        },
        {
            "@id": "core:lineFour",
            "@type": "rdf:Property",
            "schema:rangeIncludes": {
                "@id": "xsd:string"
            },
            "schema:domainIncludes": {
                "@id": "core:TradeAddress"
            },
            "rdfs:comment": "The fourth free form line, expressed as text, of this trade address.",
            "rdfs:label": "lineFour",
            "unece:cefactElementMetadata": [
                {
                    "@id": "cefact:Trade_Address.LineFour.Text",
                    "@type": "unece:BasicBIE",
                    "unece:TDED": "3286",
                    "unece:cefactUNId": "UN01004541",
                    "unece:cefactBieDomainClass": "cefact:Trade_Address.Details",
                    "rdfs:comment": "The fourth free form line, expressed as text, of this trade address."
                }
            ]
        },
        {
            "@id": "core:lineOfCreditSpecifiedFinancialAccount",
            "@type": "rdf:Property",
            "schema:rangeIncludes": {
                "@id": "core:FinancialAccount"
            },
            "schema:domainIncludes": [
                {
                    "@id": "core:FinancingSummaryDocument"
                },
                {
                    "@id": ":RequestingParty"
                }
            ],
            "rdfs:comment": [
                "The financing financial account, used for managing the line of credit, specified for this financing summary document.",
                "The financing financial account, used for managing the line of credit, specified for this requesting party."
            ],
            "rdfs:label": "lineOfCreditSpecifiedFinancialAccount",
            "unece:cefactElementMetadata": [
                {
                    "@id": "cefact:FinancingSummary_Document.LineOfCredit_Specified.Financing_FinancialAccount",
                    "@type": "unece:AssociationBIE",
                    "unece:cefactUNId": "UN01013251",
                    "unece:cefactBieDomainClass": "cefact:FinancingSummary_Document.Details",
                    "rdfs:comment": "The financing financial account, used for managing the line of credit, specified for this financing summary document."
                },
                {
                    "@id": "cefact:Requesting_Party.LineOfCredit_Specified.Financing_FinancialAccount",
                    "@type": "unece:AssociationBIE",
                    "unece:cefactUNId": "UN01013293",
                    "unece:cefactBieDomainClass": "cefact:Requesting_Party.Details",
                    "rdfs:comment": "The financing financial account, used for managing the line of credit, specified for this requesting party."
                }
            ]
        },
        {
            "@id": "core:lineOne",
            "@type": "rdf:Property",
            "schema:rangeIncludes": {
                "@id": "xsd:string"
            },
            "schema:domainIncludes": {
                "@id": "core:TradeAddress"
            },
            "rdfs:comment": "The first free form line, expressed as text, of this trade address.",
            "rdfs:label": "lineOne",
            "unece:cefactElementMetadata": [
                {
                    "@id": "cefact:Trade_Address.LineOne.Text",
                    "@type": "unece:BasicBIE",
                    "unece:TDED": "3286",
                    "unece:cefactUNId": "UN01004538",
                    "unece:cefactBieDomainClass": "cefact:Trade_Address.Details",
                    "rdfs:comment": "The first free form line, expressed as text, of this trade address."
                }
            ]
        },
        {
            "@id": "core:lineThree",
            "@type": "rdf:Property",
            "schema:rangeIncludes": {
                "@id": "xsd:string"
            },
            "schema:domainIncludes": {
                "@id": "core:TradeAddress"
            },
            "rdfs:comment": "The third free form line, expressed as text, of this trade address.",
            "rdfs:label": "lineThree",
            "unece:cefactElementMetadata": [
                {
                    "@id": "cefact:Trade_Address.LineThree.Text",
                    "@type": "unece:BasicBIE",
                    "unece:TDED": "3286",
                    "unece:cefactUNId": "UN01004540",
                    "unece:cefactBieDomainClass": "cefact:Trade_Address.Details",
                    "rdfs:comment": "The third free form line, expressed as text, of this trade address."
                }
            ]
        },
        {
            "@id": "core:lineTwo",
            "@type": "rdf:Property",
            "schema:rangeIncludes": {
                "@id": "xsd:string"
            },
            "schema:domainIncludes": {
                "@id": "core:TradeAddress"
            },
            "rdfs:comment": "The second free form line, expressed as text, of this trade address.",
            "rdfs:label": "lineTwo",
            "unece:cefactElementMetadata": [
                {
                    "@id": "cefact:Trade_Address.LineTwo.Text",
                    "@type": "unece:BasicBIE",
                    "unece:TDED": "3286",
                    "unece:cefactUNId": "UN01004539",
                    "unece:cefactBieDomainClass": "cefact:Trade_Address.Details",
                    "rdfs:comment": "The second free form line, expressed as text, of this trade address."
                }
            ]
        },
        {
            "@id": "core:locationFunctionTypeCode",
            "@type": "rdf:Property",
            "schema:rangeIncludes": {
                "@id": "unece:UNECECL3227Code"
            },
            "schema:domainIncludes": [
                {
                    "@id": "core:LogisticsLocation"
                },
                {
                    "@id": "core:TransportServiceLocation"
                }
            ],
            "rdfs:comment": [
                "A code specifying the type of this logistics related location.",
                "A code specifying the type of transport service location."
            ],
            "rdfs:label": "locationFunctionTypeCode",
            "unece:cefactElementMetadata": [
                {
                    "@id": "cefact:Logistics_Location.Type.Code",
                    "@type": "unece:BasicBIE",
                    "unece:TDED": "3227",
                    "unece:cefactUNId": "UN01003682",
                    "unece:cefactBieDomainClass": "cefact:Logistics_Location.Details",
                    "rdfs:comment": "A code specifying the type of this logistics related location."
                },
                {
                    "@id": "cefact:TransportService_Location.Type.Code",
                    "@type": "unece:BasicBIE",
                    "unece:TDED": "3227",
                    "unece:cefactUNId": "UN01010089",
                    "unece:cefactBieDomainClass": "cefact:TransportService_Location.Details",
                    "rdfs:comment": "A code specifying the type of transport service location."
                }
            ]
        },
        {
            "@id": "core:logoAssociatedBinaryFile",
            "@type": "rdf:Property",
            "schema:rangeIncludes": {
                "@id": "core:BinaryFile"
            },
            "schema:domainIncludes": {
                "@id": "core:TradeParty"
            },
            "rdfs:comment": "A file containing a specified binary representation of a logo associated with this trade party.",
            "rdfs:label": "logoAssociatedBinaryFile",
            "unece:cefactElementMetadata": [
                {
                    "@id": "cefact:Trade_Party.Logo_Associated.Specified_BinaryFile",
                    "@type": "unece:AssociationBIE",
                    "unece:cefactUNId": "UN01006723",
                    "unece:cefactBieDomainClass": "cefact:Trade_Party.Details",
                    "rdfs:comment": "A file containing a specified binary representation of a logo associated with this trade party."
                }
            ]
        },
        {
            "@id": "core:logoReferencedDocument",
            "@type": "rdf:Property",
            "schema:rangeIncludes": {
                "@id": "core:Document"
            },
            "schema:domainIncludes": {
                "@id": "core:TradeParty"
            },
            "rdfs:comment": "The referenced logo document for this trade party.",
            "rdfs:label": "logoReferencedDocument",
            "unece:cefactElementMetadata": [
                {
                    "@id": "cefact:Trade_Party.Logo_Referenced.Referenced_Document",
                    "@type": "unece:AssociationBIE",
                    "unece:cefactUNId": "UN01004616",
                    "unece:cefactBieDomainClass": "cefact:Trade_Party.Details",
                    "rdfs:comment": "The referenced logo document for this trade party."
                }
            ]
        },
        {
            "@id": "core:maritimeAnchorageIndicator",
            "@type": "rdf:Property",
            "schema:rangeIncludes": {
                "@id": "xsd:boolean"
            },
            "schema:domainIncludes": {
                "@id": ":TransportEvent"
            },
            "rdfs:comment": "The indication of whether or not this transport event is a maritime anchorage.",
            "rdfs:label": "maritimeAnchorageIndicator",
            "unece:cefactElementMetadata": [
                {
                    "@id": "cefact:Transport_Event.MaritimeAnchorage.Indicator",
                    "@type": "unece:BasicBIE",
                    "unece:cefactUNId": "UN01015100",
                    "unece:cefactBieDomainClass": "cefact:Transport_Event.Details",
                    "rdfs:comment": "The indication of whether or not this transport event is a maritime anchorage."
                }
            ]
        },
        {
            "@id": "core:microchipIndicator",
            "@type": "rdf:Property",
            "schema:rangeIncludes": {
                "@id": "xsd:boolean"
            },
            "schema:domainIncludes": {
                "@id": "core:TradeSettlementFinancialCard"
            },
            "rdfs:comment": "The indication of whether or not this trade settlement financial card has a microchip.",
            "rdfs:label": "microchipIndicator",
            "unece:cefactElementMetadata": [
                {
                    "@id": "cefact:TradeSettlement_FinancialCard.Microchip.Indicator",
                    "@type": "unece:BasicBIE",
                    "unece:cefactUNId": "UN01004494",
                    "unece:cefactBieDomainClass": "cefact:TradeSettlement_FinancialCard.Details",
                    "rdfs:comment": "The indication of whether or not this trade settlement financial card has a microchip."
                }
            ]
        },
        {
            "@id": "core:mobileTelephoneCommunication",
            "@type": "rdf:Property",
            "schema:rangeIncludes": {
                "@id": "core:Communication"
            },
            "schema:domainIncludes": {
                "@id": ":TradeContact"
            },
            "rdfs:comment": "The mobile telephone communication information for this trade contact.",
            "rdfs:label": "mobileTelephoneCommunication",
            "unece:cefactElementMetadata": [
                {
                    "@id": "cefact:Trade_Contact.Mobile_Telephone.Universal_Communication",
                    "@type": "unece:AssociationBIE",
                    "unece:cefactUNId": "UN01004566",
                    "unece:cefactBieDomainClass": "cefact:Trade_Contact.Details",
                    "rdfs:comment": "The mobile telephone communication information for this trade contact."
                }
            ]
        },
        {
            "@id": "core:name",
            "@type": "rdf:Property",
            "schema:rangeIncludes": {
                "@id": "xsd:string"
            },
            "schema:domainIncludes": [
                {
                    "@id": "core:LogisticsLocation"
                },
                {
                    "@id": "core:TradeGeopoliticalRegion"
                },
                {
                    "@id": "core:TradeParty"
                },
                {
                    "@id": "core:TransportServiceLocation"
                }
            ],
            "rdfs:comment": [
                "A name, expressed as text, of this logistics related location.",
                "A name, expressed as text, of this transport service location.",
                "The name, expressed as text, for this trade party.",
                "The name, expressed as text, of this trade geopolitical region."
            ],
            "rdfs:label": "name",
            "unece:cefactElementMetadata": [
                {
                    "@id": "cefact:Trade_GeopoliticalRegion.Name.Text",
                    "@type": "unece:BasicBIE",
                    "unece:cefactUNId": "UN01004590",
                    "unece:cefactBieDomainClass": "cefact:Trade_GeopoliticalRegion.Details",
                    "rdfs:comment": "The name, expressed as text, of this trade geopolitical region."
                },
                {
                    "@id": "cefact:Logistics_Location.Name.Text",
                    "@type": "unece:BasicBIE",
                    "unece:TDED": "3224",
                    "unece:cefactUNId": "UN01003681",
                    "unece:cefactBieDomainClass": "cefact:Logistics_Location.Details",
                    "rdfs:comment": "A name, expressed as text, of this logistics related location."
                },
                {
                    "@id": "cefact:Trade_Party.Name.Text",
                    "@type": "unece:BasicBIE",
                    "unece:TDED": "3036",
                    "unece:cefactUNId": "UN01004598",
                    "unece:cefactBieDomainClass": "cefact:Trade_Party.Details",
                    "rdfs:comment": "The name, expressed as text, for this trade party."
                },
                {
                    "@id": "cefact:TransportService_Location.Name.Text",
                    "@type": "unece:BasicBIE",
                    "unece:TDED": "3224",
                    "unece:cefactUNId": "UN01010088",
                    "unece:cefactBieDomainClass": "cefact:TransportService_Location.Details",
                    "rdfs:comment": "A name, expressed as text, of this transport service location."
                }
            ]
        },
        {
            "@id": "core:occurrenceDateTime",
            "@type": "rdf:Property",
            "schema:rangeIncludes": {
                "@id": "xsd:dateTime"
            },
            "schema:domainIncludes": {
                "@id": "core:SupplyChainEvent"
            },
            "rdfs:comment": "A date, time, date time, or other date time value of an occurrence of this supply chain event.",
            "rdfs:label": "occurrenceDateTime",
            "unece:cefactElementMetadata": [
                {
                    "@id": "cefact:SupplyChain_Event.Occurrence.DateTime",
                    "@type": "unece:BasicBIE",
                    "unece:TDED": "2193",
                    "unece:cefactUNId": "UN01004293",
                    "unece:cefactBieDomainClass": "cefact:SupplyChain_Event.Details",
                    "rdfs:comment": "A date, time, date time, or other date time value of an occurrence of this supply chain event."
                }
            ]
        },
        {
            "@id": "core:occurrenceLocation",
            "@type": "rdf:Property",
            "schema:rangeIncludes": {
                "@id": "core:Location"
            },
            "schema:domainIncludes": {
                "@id": "core:SupplyChainEvent"
            },
            "rdfs:comment": [
                "A logistics location where this supply chain event occurs.",
                "The referenced location for the occurrence of this supply chain event."
            ],
            "rdfs:label": "occurrenceLocation",
            "unece:cefactElementMetadata": [
                {
                    "@id": "cefact:SupplyChain_Event.Occurrence.Logistics_Location",
                    "@type": "unece:AssociationBIE",
                    "unece:cefactUNId": "UN01004299",
                    "unece:cefactBieDomainClass": "cefact:SupplyChain_Event.Details",
                    "rdfs:comment": "A logistics location where this supply chain event occurs."
                },
                {
                    "@id": "cefact:SupplyChain_Event.Occurrence.Referenced_Location",
                    "@type": "unece:AssociationBIE",
                    "unece:cefactUNId": "UN01014451",
                    "unece:cefactBieDomainClass": "cefact:SupplyChain_Event.Details",
                    "rdfs:comment": "The referenced location for the occurrence of this supply chain event."
                }
            ]
        },
        {
            "@id": "core:occurrencePeriod",
            "@type": "rdf:Property",
            "schema:rangeIncludes": {
                "@id": "core:Period"
            },
            "schema:domainIncludes": [
                {
                    "@id": "core:Referenced_TransportEvent"
                },
                {
                    "@id": "core:SupplyChainEvent"
                }
            ],
            "rdfs:comment": [
                "A specified period of time during which this supply chain event occurs.",
                "A specified period of time for the occurrence of this referenced transport event."
            ],
            "rdfs:label": "occurrencePeriod",
            "unece:cefactElementMetadata": [
                {
                    "@id": "cefact:Referenced_Transport_Event.Occurrence.Specified_Period",
                    "@type": "unece:AssociationBIE",
                    "unece:cefactUNId": "UN01010085",
                    "unece:cefactBieDomainClass": "cefact:Referenced_Transport_Event.Details",
                    "rdfs:comment": "A specified period of time for the occurrence of this referenced transport event."
                },
                {
                    "@id": "cefact:SupplyChain_Event.Occurrence.Specified_Period",
                    "@type": "unece:AssociationBIE",
                    "unece:cefactUNId": "UN01004298",
                    "unece:cefactBieDomainClass": "cefact:SupplyChain_Event.Details",
                    "rdfs:comment": "A specified period of time during which this supply chain event occurs."
                }
            ]
        },
        {
            "@id": "core:ownedFinancialAccount",
            "@type": "rdf:Property",
            "schema:rangeIncludes": {
                "@id": "core:FinancialAccount"
            },
            "schema:domainIncludes": {
                "@id": "core:TradeParty"
            },
            "rdfs:comment": "The creditor financial account owned by this trade party.",
            "rdfs:label": "ownedFinancialAccount",
            "unece:cefactElementMetadata": [
                {
                    "@id": "cefact:Trade_Party.Owned.Creditor_FinancialAccount",
                    "@type": "unece:AssociationBIE",
                    "unece:cefactUNId": "UN01013304",
                    "unece:cefactBieDomainClass": "cefact:Trade_Party.Details",
                    "rdfs:comment": "The creditor financial account owned by this trade party."
                }
            ]
        },
        {
            "@id": "core:paidAmount",
            "@type": "rdf:Property",
            "schema:rangeIncludes": {
                "@id": "xsd:decimal"
            },
            "schema:domainIncludes": {
                "@id": "core:InstalmentPayment"
            },
            "rdfs:comment": "A monetary value paid or to be paid for this instalment payment.",
            "rdfs:label": "paidAmount",
            "unece:cefactElementMetadata": [
                {
                    "@id": "cefact:Instalment_Payment.Paid.Amount",
                    "@type": "unece:BasicBIE",
                    "unece:TDED": "5082",
                    "unece:cefactUNId": "UN01013274",
                    "unece:cefactBieDomainClass": "cefact:Instalment_Payment.Details",
                    "rdfs:comment": "A monetary value paid or to be paid for this instalment payment."
                }
            ]
        },
        {
            "@id": "core:partialPaymentPercent",
            "@type": "rdf:Property",
            "schema:rangeIncludes": {
                "@id": "xsd:decimal"
            },
            "schema:domainIncludes": {
                "@id": ":TradePaymentTerms"
            },
            "rdfs:comment": "A partial payment, expressed as a percent, in these trade payment terms.",
            "rdfs:label": "partialPaymentPercent",
            "unece:cefactElementMetadata": [
                {
                    "@id": "cefact:Trade_PaymentTerms.PartialPayment.Percent",
                    "@type": "unece:BasicBIE",
                    "unece:cefactUNId": "UN01006047",
                    "unece:cefactBieDomainClass": "cefact:Trade_PaymentTerms.Details",
                    "rdfs:comment": "A partial payment, expressed as a percent, in these trade payment terms."
                }
            ]
        },
        {
            "@id": "core:partyRoleCode",
            "@type": "rdf:Property",
            "schema:rangeIncludes": {
                "@id": "unece:UNECECL3035Code"
            },
            "schema:domainIncludes": {
                "@id": "core:TradeParty"
            },
            "rdfs:comment": "A code specifying the role of this trade party.",
            "rdfs:label": "partyRoleCode",
            "unece:cefactElementMetadata": [
                {
                    "@id": "cefact:Trade_Party.Role.Code",
                    "@type": "unece:BasicBIE",
                    "unece:TDED": "3035",
                    "unece:cefactUNId": "UN01004599",
                    "unece:cefactBieDomainClass": "cefact:Trade_Party.Details",
                    "rdfs:comment": "A code specifying the role of this trade party."
                }
            ]
        },
        {
            "@id": "core:passportId",
            "@type": "rdf:Property",
            "schema:rangeIncludes": {
                "@id": "xsd:token"
            },
            "schema:domainIncludes": {
                "@id": "core:PersonIdentity"
            },
            "rdfs:comment": "The passport identifier for this person.",
            "rdfs:label": "passportId",
            "unece:cefactElementMetadata": [
                {
                    "@id": "cefact:Person_Identity.Passport_Identification.Identifier",
                    "@type": "unece:BasicBIE",
                    "unece:cefactUNId": "UN01013280",
                    "unece:cefactBieDomainClass": "cefact:Person_Identity.Details",
                    "rdfs:comment": "The passport identifier for this person."
                }
            ]
        },
        {
            "@id": "core:payeePartyFinancialAccount",
            "@type": "rdf:Property",
            "schema:rangeIncludes": {
                "@id": "core:FinancialAccount"
            },
            "schema:domainIncludes": {
                "@id": "core:TradeSettlementPaymentMeans"
            },
            "rdfs:comment": "A creditor financial account of the payee party for this trade settlement payment means.",
            "rdfs:label": "payeePartyFinancialAccount",
            "unece:cefactElementMetadata": [
                {
                    "@id": "cefact:TradeSettlement_PaymentMeans.Payee_Party.Creditor_FinancialAccount",
                    "@type": "unece:AssociationBIE",
                    "unece:cefactUNId": "UN01004519",
                    "unece:cefactBieDomainClass": "cefact:TradeSettlement_PaymentMeans.Details",
                    "rdfs:comment": "A creditor financial account of the payee party for this trade settlement payment means."
                }
            ]
        },
        {
            "@id": "core:payeeSpecifiedFinancialInstitution",
            "@type": "rdf:Property",
            "schema:rangeIncludes": {
                "@id": "core:FinancialInstitution"
            },
            "schema:domainIncludes": {
                "@id": "core:TradeSettlementPaymentMeans"
            },
            "rdfs:comment": "The creditor financial institution of the payee party specified for this trade settlement payment means.",
            "rdfs:label": "payeeSpecifiedFinancialInstitution",
            "unece:cefactElementMetadata": [
                {
                    "@id": "cefact:TradeSettlement_PaymentMeans.Payee_Specified.Creditor_FinancialInstitution",
                    "@type": "unece:AssociationBIE",
                    "unece:cefactUNId": "UN01004521",
                    "unece:cefactBieDomainClass": "cefact:TradeSettlement_PaymentMeans.Details",
                    "rdfs:comment": "The creditor financial institution of the payee party specified for this trade settlement payment means."
                }
            ]
        },
        {
            "@id": "core:payerPartyFinancialAccount",
            "@type": "rdf:Property",
            "schema:rangeIncludes": {
                "@id": "core:FinancialAccount"
            },
            "schema:domainIncludes": {
                "@id": "core:TradeSettlementPaymentMeans"
            },
            "rdfs:comment": "The debtor financial account of the payer party for this trade settlement payment means.",
            "rdfs:label": "payerPartyFinancialAccount",
            "unece:cefactElementMetadata": [
                {
                    "@id": "cefact:TradeSettlement_PaymentMeans.Payer_Party.Debtor_FinancialAccount",
                    "@type": "unece:AssociationBIE",
                    "unece:cefactUNId": "UN01004518",
                    "unece:cefactBieDomainClass": "cefact:TradeSettlement_PaymentMeans.Details",
                    "rdfs:comment": "The debtor financial account of the payer party for this trade settlement payment means."
                }
            ]
        },
        {
            "@id": "core:payerSpecifiedFinancialInstitution",
            "@type": "rdf:Property",
            "schema:rangeIncludes": {
                "@id": "core:FinancialInstitution"
            },
            "schema:domainIncludes": {
                "@id": "core:TradeSettlementPaymentMeans"
            },
            "rdfs:comment": "The debtor financial institution of the payer party specified for this trade settlement payment means.",
            "rdfs:label": "payerSpecifiedFinancialInstitution",
            "unece:cefactElementMetadata": [
                {
                    "@id": "cefact:TradeSettlement_PaymentMeans.Payer_Specified.Debtor_FinancialInstitution",
                    "@type": "unece:AssociationBIE",
                    "unece:cefactUNId": "UN01004520",
                    "unece:cefactBieDomainClass": "cefact:TradeSettlement_PaymentMeans.Details",
                    "rdfs:comment": "The debtor financial institution of the payer party specified for this trade settlement payment means."
                }
            ]
        },
        {
            "@id": "core:paymentGuaranteeMeansGuaranteeMethodCode",
            "@type": "rdf:Property",
            "schema:rangeIncludes": {
                "@id": "unece:UNECECL4431Code"
            },
            "schema:domainIncludes": {
                "@id": "core:TradeSettlementPaymentMeans"
            },
            "rdfs:comment": "The code specifying the method of guarantee for this trade settlement payment means.",
            "rdfs:label": "paymentGuaranteeMeansGuaranteeMethodCode",
            "unece:cefactElementMetadata": [
                {
                    "@id": "cefact:TradeSettlement_PaymentMeans.GuaranteeMethod.Code",
                    "@type": "unece:BasicBIE",
                    "unece:TDED": "4431",
                    "unece:cefactUNId": "UN01004515",
                    "unece:cefactBieDomainClass": "cefact:TradeSettlement_PaymentMeans.Details",
                    "rdfs:comment": "The code specifying the method of guarantee for this trade settlement payment means."
                }
            ]
        },
        {
            "@id": "core:paymentMeansChannelPaymentChannelCode",
            "@type": "rdf:Property",
            "schema:rangeIncludes": {
                "@id": "unece:UNECECL4435Code"
            },
            "schema:domainIncludes": {
                "@id": "core:TradeSettlementPaymentMeans"
            },
            "rdfs:comment": "The code specifying the payment channel through which this trade settlement payment is to be processed (Reference United Nations Code List (UNCL) 4435).",
            "rdfs:label": "paymentMeansChannelPaymentChannelCode",
            "unece:cefactElementMetadata": [
                {
                    "@id": "cefact:TradeSettlement_PaymentMeans.PaymentChannel.Code",
                    "@type": "unece:BasicBIE",
                    "unece:TDED": "4435",
                    "unece:cefactUNId": "UN01004513",
                    "unece:cefactBieDomainClass": "cefact:TradeSettlement_PaymentMeans.Details",
                    "rdfs:comment": "The code specifying the payment channel through which this trade settlement payment is to be processed (Reference United Nations Code List (UNCL) 4435)."
                }
            ]
        },
        {
            "@id": "core:paymentMeansTypeCode",
            "@type": "rdf:Property",
            "schema:rangeIncludes": {
                "@id": "unece:UNECECL4461Code"
            },
            "schema:domainIncludes": {
                "@id": "core:TradeSettlementPaymentMeans"
            },
            "rdfs:comment": "The code specifying the type of trade settlement payment means, such as cash or check.",
            "rdfs:label": "paymentMeansTypeCode",
            "unece:cefactElementMetadata": [
                {
                    "@id": "cefact:TradeSettlement_PaymentMeans.Type.Code",
                    "@type": "unece:BasicBIE",
                    "unece:TDED": "4461",
                    "unece:cefactUNId": "UN01004514",
                    "unece:cefactBieDomainClass": "cefact:TradeSettlement_PaymentMeans.Details",
                    "rdfs:comment": "The code specifying the type of trade settlement payment means, such as cash or check."
                }
            ]
        },
        {
            "@id": "core:paymentMethodCode",
            "@type": "rdf:Property",
            "schema:rangeIncludes": {
                "@id": "xsd:token"
            },
            "schema:domainIncludes": {
                "@id": "core:TradeSettlementPaymentMeans"
            },
            "rdfs:comment": "The code specifying the method by which a payment may be made for this trade settlement payment means.",
            "rdfs:label": "paymentMethodCode",
            "unece:cefactElementMetadata": [
                {
                    "@id": "cefact:TradeSettlement_PaymentMeans.PaymentMethod.Code",
                    "@type": "unece:BasicBIE",
                    "unece:cefactUNId": "UN01004516",
                    "unece:cefactBieDomainClass": "cefact:TradeSettlement_PaymentMeans.Details",
                    "rdfs:comment": "The code specifying the method by which a payment may be made for this trade settlement payment means."
                }
            ]
        },
        {
            "@id": "core:paymentTermsTypeCode",
            "@type": "rdf:Property",
            "schema:rangeIncludes": {
                "@id": "unece:UNECECL4279Code"
            },
            "schema:domainIncludes": {
                "@id": ":TradePaymentTerms"
            },
            "rdfs:comment": "A code specifying the type of trade payment terms.",
            "rdfs:label": "paymentTermsTypeCode",
            "unece:cefactElementMetadata": [
                {
                    "@id": "cefact:Trade_PaymentTerms.Type.Code",
                    "@type": "unece:BasicBIE",
                    "unece:TDED": "4279",
                    "unece:cefactUNId": "UN01004634",
                    "unece:cefactBieDomainClass": "cefact:Trade_PaymentTerms.Details",
                    "rdfs:comment": "A code specifying the type of trade payment terms."
                }
            ]
        },
        {
            "@id": "core:personId",
            "@type": "rdf:Property",
            "schema:rangeIncludes": {
                "@id": "xsd:token"
            },
            "schema:domainIncludes": {
                "@id": ":TradeContact"
            },
            "rdfs:comment": "A unique identifier for this trade contact person.",
            "rdfs:label": "personId",
            "unece:cefactElementMetadata": [
                {
                    "@id": "cefact:Trade_Contact.Person_Identification.Identifier",
                    "@type": "unece:BasicBIE",
                    "unece:TDED": "3413",
                    "unece:cefactUNId": "UN01004563",
                    "unece:cefactBieDomainClass": "cefact:Trade_Contact.Details",
                    "rdfs:comment": "A unique identifier for this trade contact person."
                }
            ]
        },
        {
            "@id": "core:physicalGeographicalCoordinate",
            "@type": "rdf:Property",
            "schema:rangeIncludes": {
                "@id": "core:GeographicalCoordinate"
            },
            "schema:domainIncludes": [
                {
                    "@id": "core:LogisticsLocation"
                },
                {
                    "@id": "core:TransportServiceLocation"
                }
            ],
            "rdfs:comment": [
                "Geographical coordinate information for this logistics related location.",
                "Geographical coordinate information for this physical transport service location."
            ],
            "rdfs:label": "physicalGeographicalCoordinate",
            "unece:cefactElementMetadata": [
                {
                    "@id": "cefact:TransportService_Location.Physical.GeographicalCoordinate",
                    "@type": "unece:AssociationBIE",
                    "unece:cefactUNId": "UN01010090",
                    "unece:cefactBieDomainClass": "cefact:TransportService_Location.Details",
                    "rdfs:comment": "Geographical coordinate information for this physical transport service location."
                },
                {
                    "@id": "cefact:Logistics_Location.Physical.GeographicalCoordinate",
                    "@type": "unece:AssociationBIE",
                    "unece:cefactUNId": "UN01003685",
                    "unece:cefactBieDomainClass": "cefact:Logistics_Location.Details",
                    "rdfs:comment": "Geographical coordinate information for this logistics related location."
                }
            ]
        },
        {
            "@id": "core:pilotBoardingPlace",
            "@type": "rdf:Property",
            "schema:rangeIncludes": {
                "@id": "xsd:string"
            },
            "schema:domainIncludes": {
                "@id": ":TransportEvent"
            },
            "rdfs:comment": "A pilot boarding place, expressed as text, for this transport event.",
            "rdfs:label": "pilotBoardingPlace",
            "unece:cefactElementMetadata": [
                {
                    "@id": "cefact:Transport_Event.PilotBoardingPlace.Text",
                    "@type": "unece:BasicBIE",
                    "unece:cefactUNId": "UN01015101",
                    "unece:cefactBieDomainClass": "cefact:Transport_Event.Details",
                    "rdfs:comment": "A pilot boarding place, expressed as text, for this transport event."
                }
            ]
        },
        {
            "@id": "core:postOfficeBox",
            "@type": "rdf:Property",
            "schema:rangeIncludes": {
                "@id": "xsd:string"
            },
            "schema:domainIncludes": {
                "@id": "core:TradeAddress"
            },
            "rdfs:comment": "The unique identifier, expressed as text, of a container commonly referred to as a box, in a post office or other postal service location, assigned to a person or organization, where postal items may be kept for this trade address.",
            "rdfs:label": "postOfficeBox",
            "unece:cefactElementMetadata": [
                {
                    "@id": "cefact:Trade_Address.PostOfficeBox.Text",
                    "@type": "unece:BasicBIE",
                    "unece:TDED": "3042",
                    "unece:cefactUNId": "UN01004536",
                    "unece:cefactBieDomainClass": "cefact:Trade_Address.Details",
                    "rdfs:comment": "The unique identifier, expressed as text, of a container commonly referred to as a box, in a post office or other postal service location, assigned to a person or organization, where postal items may be kept for this trade address."
                }
            ]
        },
        {
            "@id": "core:postalAddress",
            "@type": "rdf:Property",
            "schema:rangeIncludes": {
                "@id": "core:Address"
            },
            "schema:domainIncludes": [
                {
                    "@id": "core:LogisticsLocation"
                },
                {
                    "@id": "core:TradeParty"
                }
            ],
            "rdfs:comment": [
                "The postal address for this trade party.",
                "The postal trade address information for this logistics related location."
            ],
            "rdfs:label": "postalAddress",
            "unece:cefactElementMetadata": [
                {
                    "@id": "cefact:Trade_Party.Postal.Trade_Address",
                    "@type": "unece:AssociationBIE",
                    "unece:cefactUNId": "UN01004603",
                    "unece:cefactBieDomainClass": "cefact:Trade_Party.Details",
                    "rdfs:comment": "The postal address for this trade party."
                },
                {
                    "@id": "cefact:Logistics_Location.Postal.Trade_Address",
                    "@type": "unece:AssociationBIE",
                    "unece:cefactUNId": "UN01003686",
                    "unece:cefactBieDomainClass": "cefact:Logistics_Location.Details",
                    "rdfs:comment": "The postal trade address information for this logistics related location."
                }
            ]
        },
        {
            "@id": "core:postcodeCode",
            "@type": "rdf:Property",
            "schema:rangeIncludes": {
                "@id": "xsd:token"
            },
            "schema:domainIncludes": {
                "@id": "core:TradeAddress"
            },
            "rdfs:comment": "A code specifying the postcode of this trade address.",
            "rdfs:label": "postcodeCode",
            "unece:cefactElementMetadata": [
                {
                    "@id": "cefact:Trade_Address.Postcode.Code",
                    "@type": "unece:BasicBIE",
                    "unece:TDED": "3251",
                    "unece:cefactUNId": "UN01004535",
                    "unece:cefactBieDomainClass": "cefact:Trade_Address.Details",
                    "rdfs:comment": "A code specifying the postcode of this trade address."
                }
            ]
        },
        {
            "@id": "core:previousAssociatedGeographicalFeature",
            "@type": "rdf:Property",
            "schema:rangeIncludes": {
                "@id": "core:GeographicalFeature"
            },
            "schema:domainIncludes": [
                {
                    "@id": "core:LogisticsLocation"
                },
                {
                    "@id": ":TransportEvent"
                }
            ],
            "rdfs:comment": [
                "A geographical feature previously associated with this logistics location.",
                "A geographical feature previously associated with this transport event."
            ],
            "rdfs:label": "previousAssociatedGeographicalFeature",
            "unece:cefactElementMetadata": [
                {
                    "@id": "cefact:Transport_Event.Previous_Associated.Specified_GeographicalFeature",
                    "@type": "unece:AssociationBIE",
                    "unece:cefactUNId": "UN01013588",
                    "unece:cefactBieDomainClass": "cefact:Transport_Event.Details",
                    "rdfs:comment": "A geographical feature previously associated with this transport event."
                },
                {
                    "@id": "cefact:Logistics_Location.Previous_Associated.Specified_GeographicalFeature",
                    "@type": "unece:AssociationBIE",
                    "unece:cefactUNId": "UN01013609",
                    "unece:cefactBieDomainClass": "cefact:Logistics_Location.Details",
                    "rdfs:comment": "A geographical feature previously associated with this logistics location."
                }
            ]
        },
        {
            "@id": "core:proprietaryId",
            "@type": "rdf:Property",
            "schema:rangeIncludes": {
                "@id": "xsd:token"
            },
            "schema:domainIncludes": {
                "@id": "core:FinancingFinancialAccount"
            },
            "rdfs:comment": "The proprietary identifier for this financing financial account.",
            "rdfs:label": "proprietaryId",
            "unece:cefactElementMetadata": [
                {
                    "@id": "cefact:Financing_FinancialAccount.Proprietary_Identification.Identifier",
                    "@type": "unece:BasicBIE",
                    "unece:TDED": "3492",
                    "unece:cefactUNId": "UN01013261",
                    "unece:cefactBieDomainClass": "cefact:Financing_FinancialAccount.Details",
                    "rdfs:comment": "The proprietary identifier for this financing financial account."
                }
            ]
        },
        {
            "@id": "core:proprietaryType",
            "@type": "rdf:Property",
            "schema:rangeIncludes": {
                "@id": "xsd:string"
            },
            "schema:domainIncludes": [
                {
                    "@id": "core:FinancingFinancialAccount"
                },
                {
                    "@id": ":ReferencedDocument"
                }
            ],
            "rdfs:comment": [
                "A proprietary type, expressed as text, for this referenced document.",
                "The proprietary type, expressed as text, of this financing financial account, such as the nature or use."
            ],
            "rdfs:label": "proprietaryType",
            "unece:cefactElementMetadata": [
                {
                    "@id": "cefact:Financing_FinancialAccount.Proprietary_Type.Text",
                    "@type": "unece:BasicBIE",
                    "unece:cefactUNId": "UN01013258",
                    "unece:cefactBieDomainClass": "cefact:Financing_FinancialAccount.Details",
                    "rdfs:comment": "The proprietary type, expressed as text, of this financing financial account, such as the nature or use."
                },
                {
                    "@id": "cefact:Referenced_Document.Proprietary_Type.Text",
                    "@type": "unece:BasicBIE",
                    "unece:cefactUNId": "UN01013290",
                    "unece:cefactBieDomainClass": "cefact:Referenced_Document.Details",
                    "rdfs:comment": "A proprietary type, expressed as text, for this referenced document."
                }
            ]
        },
        {
            "@id": "core:providedProcess",
            "@type": "rdf:Property",
            "schema:rangeIncludes": {
                "@id": "core:Process"
            },
            "schema:domainIncludes": {
                "@id": "core:TradeParty"
            },
            "rdfs:comment": "A production process provided by this trade party.",
            "rdfs:label": "providedProcess",
            "unece:cefactElementMetadata": [
                {
                    "@id": "cefact:Trade_Party.Provided.Production_Process",
                    "@type": "unece:AssociationBIE",
                    "unece:cefactUNId": "UN01014536",
                    "unece:cefactBieDomainClass": "cefact:Trade_Party.Details",
                    "rdfs:comment": "A production process provided by this trade party."
                }
            ]
        },
        {
            "@id": "core:providedService",
            "@type": "rdf:Property",
            "schema:rangeIncludes": {
                "@id": "core:Service"
            },
            "schema:domainIncludes": {
                "@id": "core:TradeParty"
            },
            "rdfs:comment": "A transport service provided by this trade party.",
            "rdfs:label": "providedService",
            "unece:cefactElementMetadata": [
                {
                    "@id": "cefact:Trade_Party.Provided.Transport_Service",
                    "@type": "unece:AssociationBIE",
                    "unece:cefactUNId": "UN01004608",
                    "unece:cefactBieDomainClass": "cefact:Trade_Party.Details",
                    "rdfs:comment": "A transport service provided by this trade party."
                }
            ]
        },
        {
            "@id": "core:qualityAssuranceIndicator",
            "@type": "rdf:Property",
            "schema:rangeIncludes": {
                "@id": "xsd:boolean"
            },
            "schema:domainIncludes": {
                "@id": "core:TradeParty"
            },
            "rdfs:comment": "The indication of whether or not this trade party is quality assured.",
            "rdfs:label": "qualityAssuranceIndicator",
            "unece:cefactElementMetadata": [
                {
                    "@id": "cefact:Trade_Party.QualityAssurance.Indicator",
                    "@type": "unece:BasicBIE",
                    "unece:cefactUNId": "UN01004600",
                    "unece:cefactBieDomainClass": "cefact:Trade_Party.Details",
                    "rdfs:comment": "The indication of whether or not this trade party is quality assured."
                }
            ]
        },
        {
            "@id": "core:rICId",
            "@type": "rdf:Property",
            "schema:rangeIncludes": {
                "@id": "xsd:token"
            },
            "schema:domainIncludes": {
                "@id": "core:TradeParty"
            },
            "rdfs:comment": "The unique Routing Identifier Code (RIC) identifier for this trade party.",
            "rdfs:label": "rICId",
            "unece:cefactElementMetadata": [
                {
                    "@id": "cefact:Trade_Party.RIC_Identification.Identifier",
                    "@type": "unece:BasicBIE",
                    "unece:TDED": "3039",
                    "unece:cefactUNId": "UN01006090",
                    "unece:cefactBieDomainClass": "cefact:Trade_Party.Details",
                    "rdfs:comment": "The unique Routing Identifier Code (RIC) identifier for this trade party."
                }
            ]
        },
        {
            "@id": "core:reasonTypeCode",
            "@type": "rdf:Property",
            "schema:rangeIncludes": {
                "@id": "xsd:token"
            },
            "schema:domainIncludes": {
                "@id": "core:Referenced_TransportEvent"
            },
            "rdfs:comment": "The code specifying the reason type for this referenced transport event.",
            "rdfs:label": "reasonTypeCode",
            "unece:cefactElementMetadata": [
                {
                    "@id": "cefact:Referenced_Transport_Event.Reason_Type.Code",
                    "@type": "unece:BasicBIE",
                    "unece:TDED": "9171",
                    "unece:cefactUNId": "UN01010084",
                    "unece:cefactBieDomainClass": "cefact:Referenced_Transport_Event.Details",
                    "rdfs:comment": "The code specifying the reason type for this referenced transport event."
                }
            ]
        },
        {
            "@id": "core:receivedDateTime",
            "@type": "rdf:Property",
            "schema:rangeIncludes": {
                "@id": "xsd:dateTime"
            },
            "schema:domainIncludes": {
                "@id": ":TransportEvent"
            },
            "rdfs:comment": "The date, time, date time, or other date time value when information related to this transport event was received, from the perspective of the receiver.",
            "rdfs:label": "receivedDateTime",
            "unece:cefactElementMetadata": [
                {
                    "@id": "cefact:Transport_Event.Received.DateTime",
                    "@type": "unece:BasicBIE",
                    "unece:cefactUNId": "UN01013584",
                    "unece:cefactBieDomainClass": "cefact:Transport_Event.Details",
                    "rdfs:comment": "The date, time, date time, or other date time value when information related to this transport event was received, from the perspective of the receiver."
                }
            ]
        },
        {
            "@id": "core:referenceDateTime",
            "@type": "rdf:Property",
            "schema:rangeIncludes": {
                "@id": "xsd:dateTime"
            },
            "schema:domainIncludes": {
                "@id": ":ReferencedDocument"
            },
            "rdfs:comment": "The reference date or date time for this referenced document.",
            "rdfs:label": "referenceDateTime",
            "unece:cefactElementMetadata": [
                {
                    "@id": "cefact:Referenced_Document.Reference.DateTime",
                    "@type": "unece:BasicBIE",
                    "unece:cefactUNId": "UN01013289",
                    "unece:cefactBieDomainClass": "cefact:Referenced_Document.Details",
                    "rdfs:comment": "The reference date or date time for this referenced document."
                }
            ]
        },
        {
            "@id": "core:registeredId",
            "@type": "rdf:Property",
            "schema:rangeIncludes": {
                "@id": "xsd:token"
            },
            "schema:domainIncludes": {
                "@id": "core:TradeParty"
            },
            "rdfs:comment": "A registered identifier of this trade party.",
            "rdfs:label": "registeredId",
            "unece:cefactElementMetadata": [
                {
                    "@id": "cefact:Trade_Party.Registered_Identification.Identifier",
                    "@type": "unece:BasicBIE",
                    "unece:TDED": "3039",
                    "unece:cefactUNId": "UN01013041",
                    "unece:cefactBieDomainClass": "cefact:Trade_Party.Details",
                    "rdfs:comment": "A registered identifier of this trade party."
                }
            ]
        },
        {
            "@id": "core:relatedBatch",
            "@type": "rdf:Property",
            "schema:rangeIncludes": {
                "@id": "core:Batch"
            },
            "schema:domainIncludes": {
                "@id": "core:TradeParty"
            },
            "rdfs:comment": "A product batch related to this trade party.",
            "rdfs:label": "relatedBatch",
            "unece:cefactElementMetadata": [
                {
                    "@id": "cefact:Trade_Party.Related.Product_Batch",
                    "@type": "unece:AssociationBIE",
                    "unece:cefactUNId": "UN01014545",
                    "unece:cefactBieDomainClass": "cefact:Trade_Party.Details",
                    "rdfs:comment": "A product batch related to this trade party."
                }
            ]
        },
        {
            "@id": "core:relatedBooking",
            "@type": "rdf:Property",
            "schema:rangeIncludes": {
                "@id": "core:Booking"
            },
            "schema:domainIncludes": {
                "@id": "core:FinancingSummaryDocument"
            },
            "rdfs:comment": "The financial booking related to this financing summary document.",
            "rdfs:label": "relatedBooking",
            "unece:cefactElementMetadata": [
                {
                    "@id": "cefact:FinancingSummary_Document.Related.Financial_Booking",
                    "@type": "unece:AssociationBIE",
                    "unece:cefactUNId": "UN01013250",
                    "unece:cefactBieDomainClass": "cefact:FinancingSummary_Document.Details",
                    "rdfs:comment": "The financial booking related to this financing summary document."
                }
            ]
        },
        {
            "@id": "core:relatedCharacteristic",
            "@type": "rdf:Property",
            "schema:rangeIncludes": {
                "@id": "core:Characteristic"
            },
            "schema:domainIncludes": {
                "@id": "core:SupplyChainEvent"
            },
            "rdfs:comment": [
                "A sustainability characteristic related to this supply chain event.",
                "A technical characteristic related to this supply chain event."
            ],
            "rdfs:label": "relatedCharacteristic",
            "unece:cefactElementMetadata": [
                {
                    "@id": "cefact:SupplyChain_Event.Related.Sustainability_Characteristic",
                    "@type": "unece:AssociationBIE",
                    "unece:cefactUNId": "UN01014453",
                    "unece:cefactBieDomainClass": "cefact:SupplyChain_Event.Details",
                    "rdfs:comment": "A sustainability characteristic related to this supply chain event."
                },
                {
                    "@id": "cefact:SupplyChain_Event.Related.Technical_Characteristic",
                    "@type": "unece:AssociationBIE",
                    "unece:cefactUNId": "UN01014452",
                    "unece:cefactBieDomainClass": "cefact:SupplyChain_Event.Details",
                    "rdfs:comment": "A technical characteristic related to this supply chain event."
                }
            ]
        },
        {
            "@id": "core:relatedMaterial",
            "@type": "rdf:Property",
            "schema:rangeIncludes": {
                "@id": "core:Material"
            },
            "schema:domainIncludes": {
                "@id": "core:TradeParty"
            },
            "rdfs:comment": "Material related to this trade party.",
            "rdfs:label": "relatedMaterial",
            "unece:cefactElementMetadata": [
                {
                    "@id": "cefact:Trade_Party.Related.Specified_Material",
                    "@type": "unece:AssociationBIE",
                    "unece:cefactUNId": "UN01014546",
                    "unece:cefactBieDomainClass": "cefact:Trade_Party.Details",
                    "rdfs:comment": "Material related to this trade party."
                }
            ]
        },
        {
            "@id": "core:relatedObservation",
            "@type": "rdf:Property",
            "schema:rangeIncludes": {
                "@id": "core:Observation"
            },
            "schema:domainIncludes": {
                "@id": ":TransportEvent"
            },
            "rdfs:comment": "An observation related to this transport event.",
            "rdfs:label": "relatedObservation",
            "unece:cefactElementMetadata": [
                {
                    "@id": "cefact:Transport_Event.Related.Specified_Observation",
                    "@type": "unece:AssociationBIE",
                    "unece:cefactUNId": "UN01012581",
                    "unece:cefactBieDomainClass": "cefact:Transport_Event.Details",
                    "rdfs:comment": "An observation related to this transport event."
                }
            ]
        },
        {
            "@id": "core:relatedRoute",
            "@type": "rdf:Property",
            "schema:rangeIncludes": {
                "@id": "core:Route"
            },
            "schema:domainIncludes": {
                "@id": ":TransportEvent"
            },
            "rdfs:comment": "The route related to this transport event.",
            "rdfs:label": "relatedRoute",
            "unece:cefactElementMetadata": [
                {
                    "@id": "cefact:Transport_Event.Related.Transport_Route",
                    "@type": "unece:AssociationBIE",
                    "unece:cefactUNId": "UN01010151",
                    "unece:cefactBieDomainClass": "cefact:Transport_Event.Details",
                    "rdfs:comment": "The route related to this transport event."
                }
            ]
        },
        {
            "@id": "core:reportedConditionTypeCode",
            "@type": "rdf:Property",
            "schema:rangeIncludes": {
                "@id": "xsd:token"
            },
            "schema:domainIncludes": {
                "@id": ":TransportEvent"
            },
            "rdfs:comment": "The code specifying the type of reported condition for this transport event.",
            "rdfs:label": "reportedConditionTypeCode",
            "unece:cefactElementMetadata": [
                {
                    "@id": "cefact:Transport_Event.ReportedCondition_Type.Code",
                    "@type": "unece:BasicBIE",
                    "unece:TDED": "9171",
                    "unece:cefactUNId": "UN01013582",
                    "unece:cefactBieDomainClass": "cefact:Transport_Event.Details",
                    "rdfs:comment": "The code specifying the type of reported condition for this transport event."
                }
            ]
        },
        {
            "@id": "core:reportingIOTDevice",
            "@type": "rdf:Property",
            "schema:rangeIncludes": {
                "@id": "core:IOTDevice"
            },
            "schema:domainIncludes": {
                "@id": ":TransportEvent"
            },
            "rdfs:comment": "An IOT device for this transport reporting event.",
            "rdfs:label": "reportingIOTDevice",
            "unece:cefactElementMetadata": [
                {
                    "@id": "cefact:Transport_Event.Reporting.Monitoring_IOTDevice",
                    "@type": "unece:AssociationBIE",
                    "unece:cefactUNId": "UN01013586",
                    "unece:cefactBieDomainClass": "cefact:Transport_Event.Details",
                    "rdfs:comment": "An IOT device for this transport reporting event."
                }
            ]
        },
        {
            "@id": "core:requestedNotificationReferencedDocument",
            "@type": "rdf:Property",
            "schema:rangeIncludes": {
                "@id": "core:Document"
            },
            "schema:domainIncludes": {
                "@id": "core:TradeParty"
            },
            "rdfs:comment": "A referenced notification document requested by this trade party.",
            "rdfs:label": "requestedNotificationReferencedDocument",
            "unece:cefactElementMetadata": [
                {
                    "@id": "cefact:Trade_Party.RequestedNotification_Referenced.Referenced_Document",
                    "@type": "unece:AssociationBIE",
                    "unece:cefactUNId": "UN01004614",
                    "unece:cefactBieDomainClass": "cefact:Trade_Party.Details",
                    "rdfs:comment": "A referenced notification document requested by this trade party."
                }
            ]
        },
        {
            "@id": "core:requestedRelatedService",
            "@type": "rdf:Property",
            "schema:rangeIncludes": {
                "@id": "core:Service"
            },
            "schema:domainIncludes": {
                "@id": ":TransportEvent"
            },
            "rdfs:comment": "A requested service related to this transport event.",
            "rdfs:label": "requestedRelatedService",
            "unece:cefactElementMetadata": [
                {
                    "@id": "cefact:Transport_Event.Requested_Related.ReferencedTransport_Service",
                    "@type": "unece:AssociationBIE",
                    "unece:cefactUNId": "UN01010152",
                    "unece:cefactBieDomainClass": "cefact:Transport_Event.Details",
                    "rdfs:comment": "A requested service related to this transport event."
                }
            ]
        },
        {
            "@id": "core:responsibility",
            "@type": "rdf:Property",
            "schema:rangeIncludes": {
                "@id": "xsd:string"
            },
            "schema:domainIncludes": {
                "@id": ":TradeContact"
            },
            "rdfs:comment": "A responsibility, expressed as text, of this trade contact.",
            "rdfs:label": "responsibility",
            "unece:cefactElementMetadata": [
                {
                    "@id": "cefact:Trade_Contact.Responsibility.Text",
                    "@type": "unece:BasicBIE",
                    "unece:cefactUNId": "UN01004562",
                    "unece:cefactBieDomainClass": "cefact:Trade_Contact.Details",
                    "rdfs:comment": "A responsibility, expressed as text, of this trade contact."
                }
            ]
        },
        {
            "@id": "core:role",
            "@type": "rdf:Property",
            "schema:rangeIncludes": {
                "@id": "xsd:string"
            },
            "schema:domainIncludes": {
                "@id": "core:TradeParty"
            },
            "rdfs:comment": "A role, expressed as text, for this trade party.",
            "rdfs:label": "role",
            "unece:cefactElementMetadata": [
                {
                    "@id": "cefact:Trade_Party.Role.Text",
                    "@type": "unece:BasicBIE",
                    "unece:cefactUNId": "UN01013115",
                    "unece:cefactBieDomainClass": "cefact:Trade_Party.Details",
                    "rdfs:comment": "A role, expressed as text, for this trade party."
                }
            ]
        },
        {
            "@id": "core:scheduledArrivalRelatedDateTime",
            "@type": "rdf:Property",
            "schema:rangeIncludes": {
                "@id": "xsd:dateTime"
            },
            "schema:domainIncludes": [
                {
                    "@id": "core:Referenced_TransportEvent"
                },
                {
                    "@id": ":TransportEvent"
                }
            ],
            "rdfs:comment": [
                "The date, time, date time or other date time value of the scheduled arrival related to this referenced transport event.",
                "The date, time, date time or other date time value of the scheduled arrival related to this transport event."
            ],
            "rdfs:label": "scheduledArrivalRelatedDateTime",
            "unece:cefactElementMetadata": [
                {
                    "@id": "cefact:Transport_Event.ScheduledArrival_Related.DateTime",
                    "@type": "unece:BasicBIE",
                    "unece:cefactUNId": "UN01010147",
                    "unece:cefactBieDomainClass": "cefact:Transport_Event.Details",
                    "rdfs:comment": "The date, time, date time or other date time value of the scheduled arrival related to this transport event."
                },
                {
                    "@id": "cefact:Referenced_Transport_Event.ScheduledArrival_Related.DateTime",
                    "@type": "unece:BasicBIE",
                    "unece:TDED": "2379",
                    "unece:cefactUNId": "UN01010082",
                    "unece:cefactBieDomainClass": "cefact:Referenced_Transport_Event.Details",
                    "rdfs:comment": "The date, time, date time or other date time value of the scheduled arrival related to this referenced transport event."
                }
            ]
        },
        {
            "@id": "core:scheduledDepartureRelatedDateTime",
            "@type": "rdf:Property",
            "schema:rangeIncludes": {
                "@id": "xsd:dateTime"
            },
            "schema:domainIncludes": [
                {
                    "@id": "core:Referenced_TransportEvent"
                },
                {
                    "@id": ":TransportEvent"
                }
            ],
            "rdfs:comment": [
                "The date, time, date time or other date time value of the scheduled departure related to this referenced transport event.",
                "The date, time, date time or other date time value of the scheduled departure related to this transport event."
            ],
            "rdfs:label": "scheduledDepartureRelatedDateTime",
            "unece:cefactElementMetadata": [
                {
                    "@id": "cefact:Transport_Event.ScheduledDeparture_Related.DateTime",
                    "@type": "unece:BasicBIE",
                    "unece:cefactUNId": "UN01010149",
                    "unece:cefactBieDomainClass": "cefact:Transport_Event.Details",
                    "rdfs:comment": "The date, time, date time or other date time value of the scheduled departure related to this transport event."
                },
                {
                    "@id": "cefact:Referenced_Transport_Event.ScheduledDeparture_Related.DateTime",
                    "@type": "unece:BasicBIE",
                    "unece:TDED": "2379",
                    "unece:cefactUNId": "UN01010083",
                    "unece:cefactBieDomainClass": "cefact:Referenced_Transport_Event.Details",
                    "rdfs:comment": "The date, time, date time or other date time value of the scheduled departure related to this referenced transport event."
                }
            ]
        },
        {
            "@id": "core:scheduledOccurrencePeriod",
            "@type": "rdf:Property",
            "schema:rangeIncludes": {
                "@id": "core:Period"
            },
            "schema:domainIncludes": {
                "@id": ":TransportEvent"
            },
            "rdfs:comment": "The scheduled period of time specified for the occurrence of this transport event.",
            "rdfs:label": "scheduledOccurrencePeriod",
            "unece:cefactElementMetadata": [
                {
                    "@id": "cefact:Transport_Event.Scheduled_Occurrence.Specified_Period",
                    "@type": "unece:AssociationBIE",
                    "unece:cefactUNId": "UN01013590",
                    "unece:cefactBieDomainClass": "cefact:Transport_Event.Details",
                    "rdfs:comment": "The scheduled period of time specified for the occurrence of this transport event."
                }
            ]
        },
        {
            "@id": "core:securityLevelCode",
            "@type": "rdf:Property",
            "schema:rangeIncludes": {
                "@id": "xsd:token"
            },
            "schema:domainIncludes": {
                "@id": ":TransportEvent"
            },
            "rdfs:comment": "A security level code for this transport event.",
            "rdfs:label": "securityLevelCode",
            "unece:cefactElementMetadata": [
                {
                    "@id": "cefact:Transport_Event.SecurityLevel.Code",
                    "@type": "unece:BasicBIE",
                    "unece:cefactUNId": "UN01013132",
                    "unece:cefactBieDomainClass": "cefact:Transport_Event.Details",
                    "rdfs:comment": "A security level code for this transport event."
                }
            ]
        },
        {
            "@id": "core:sequenceId",
            "@type": "rdf:Property",
            "schema:rangeIncludes": {
                "@id": "xsd:token"
            },
            "schema:domainIncludes": {
                "@id": "core:InstalmentPayment"
            },
            "rdfs:comment": "The sequence identifier for this instalment payment.",
            "rdfs:label": "sequenceId",
            "unece:cefactElementMetadata": [
                {
                    "@id": "cefact:Instalment_Payment.Sequence.Identifier",
                    "@type": "unece:BasicBIE",
                    "unece:cefactUNId": "UN01013273",
                    "unece:cefactBieDomainClass": "cefact:Instalment_Payment.Details",
                    "rdfs:comment": "The sequence identifier for this instalment payment."
                }
            ]
        },
        {
            "@id": "core:servicingSpecifiedParty",
            "@type": "rdf:Property",
            "schema:rangeIncludes": {
                "@id": "core:Party"
            },
            "schema:domainIncludes": {
                "@id": "core:LogisticsLocation"
            },
            "rdfs:comment": "A servicing party specified for this logistics related location.",
            "rdfs:label": "servicingSpecifiedParty",
            "unece:cefactElementMetadata": [
                {
                    "@id": "cefact:Logistics_Location.Servicing_Specified.Location_Party",
                    "@type": "unece:AssociationBIE",
                    "unece:cefactUNId": "UN01003688",
                    "unece:cefactBieDomainClass": "cefact:Logistics_Location.Details",
                    "rdfs:comment": "A servicing party specified for this logistics related location."
                }
            ]
        },
        {
            "@id": "core:socialSecurityId",
            "@type": "rdf:Property",
            "schema:rangeIncludes": {
                "@id": "xsd:token"
            },
            "schema:domainIncludes": {
                "@id": "core:PersonIdentity"
            },
            "rdfs:comment": "The social security identifier for this person.",
            "rdfs:label": "socialSecurityId",
            "unece:cefactElementMetadata": [
                {
                    "@id": "cefact:Person_Identity.SocialSecurity_Identification.Identifier",
                    "@type": "unece:BasicBIE",
                    "unece:cefactUNId": "UN01013281",
                    "unece:cefactBieDomainClass": "cefact:Person_Identity.Details",
                    "rdfs:comment": "The social security identifier for this person."
                }
            ]
        },
        {
            "@id": "core:specificAccreditation",
            "@type": "rdf:Property",
            "schema:rangeIncludes": {
                "@id": "core:Accreditation"
            },
            "schema:domainIncludes": {
                "@id": ":TransportPerson"
            },
            "rdfs:comment": "A certified accreditation specific to this transport person.",
            "rdfs:label": "specificAccreditation",
            "unece:cefactElementMetadata": [
                {
                    "@id": "cefact:Transport_Person.Specific.Certified_Accreditation",
                    "@type": "unece:AssociationBIE",
                    "unece:cefactUNId": "UN01010155",
                    "unece:cefactBieDomainClass": "cefact:Transport_Person.Details",
                    "rdfs:comment": "A certified accreditation specific to this transport person."
                }
            ]
        },
        {
            "@id": "core:specifiedDocument",
            "@type": "rdf:Property",
            "schema:rangeIncludes": {
                "@id": "core:Document"
            },
            "schema:domainIncludes": {
                "@id": "core:InstalmentPayment"
            },
            "rdfs:comment": "The financing request result document specified for this instalment payment.",
            "rdfs:label": "specifiedDocument",
            "unece:cefactElementMetadata": [
                {
                    "@id": "cefact:Instalment_Payment.Specified.FinancingRequestResult_Document",
                    "@type": "unece:AssociationBIE",
                    "unece:cefactUNId": "UN01013276",
                    "unece:cefactBieDomainClass": "cefact:Instalment_Payment.Details",
                    "rdfs:comment": "The financing request result document specified for this instalment payment."
                }
            ]
        },
        {
            "@id": "core:specifiedEvent",
            "@type": "rdf:Property",
            "schema:rangeIncludes": {
                "@id": "core:Event"
            },
            "schema:domainIncludes": {
                "@id": "core:LogisticsLocation"
            },
            "rdfs:comment": "An inspection event specified for this logistics location.",
            "rdfs:label": "specifiedEvent",
            "unece:cefactElementMetadata": [
                {
                    "@id": "cefact:Logistics_Location.Specified.Inspection_Event",
                    "@type": "unece:AssociationBIE",
                    "unece:cefactUNId": "UN01013830",
                    "unece:cefactBieDomainClass": "cefact:Logistics_Location.Details",
                    "rdfs:comment": "An inspection event specified for this logistics location."
                }
            ]
        },
        {
            "@id": "core:specifiedFacility",
            "@type": "rdf:Property",
            "schema:rangeIncludes": {
                "@id": "core:Facility"
            },
            "schema:domainIncludes": {
                "@id": "core:TradeParty"
            },
            "rdfs:comment": "A production facility specified for this trade party.",
            "rdfs:label": "specifiedFacility",
            "unece:cefactElementMetadata": [
                {
                    "@id": "cefact:Trade_Party.Specified.Production_Facility",
                    "@type": "unece:AssociationBIE",
                    "unece:cefactUNId": "UN01014535",
                    "unece:cefactBieDomainClass": "cefact:Trade_Party.Details",
                    "rdfs:comment": "A production facility specified for this trade party."
                }
            ]
        },
        {
            "@id": "core:specifiedFinancialAccount",
            "@type": "rdf:Property",
            "schema:rangeIncludes": {
                "@id": "core:FinancialAccount"
            },
            "schema:domainIncludes": [
                {
                    "@id": "core:FinancingSummaryDocument"
                },
                {
                    "@id": ":RequestingParty"
                },
                {
                    "@id": "core:TradeSettlementPaymentMeans"
                }
            ],
            "rdfs:comment": [
                "A creditor financial account specified for this trade settlement payment means.",
                "The creditor financial account, used for crediting, specified for this financing summary document.",
                "The creditor financial account, used for crediting, specified for this requesting party."
            ],
            "rdfs:label": "specifiedFinancialAccount",
            "unece:cefactElementMetadata": [
                {
                    "@id": "cefact:TradeSettlement_PaymentMeans.Specified.Creditor_FinancialAccount",
                    "@type": "unece:AssociationBIE",
                    "unece:cefactUNId": "UN01013300",
                    "unece:cefactBieDomainClass": "cefact:TradeSettlement_PaymentMeans.Details",
                    "rdfs:comment": "A creditor financial account specified for this trade settlement payment means."
                },
                {
                    "@id": "cefact:Requesting_Party.Specified.Creditor_FinancialAccount",
                    "@type": "unece:AssociationBIE",
                    "unece:cefactUNId": "UN01013294",
                    "unece:cefactBieDomainClass": "cefact:Requesting_Party.Details",
                    "rdfs:comment": "The creditor financial account, used for crediting, specified for this requesting party."
                },
                {
                    "@id": "cefact:FinancingSummary_Document.Specified.Creditor_FinancialAccount",
                    "@type": "unece:AssociationBIE",
                    "unece:cefactUNId": "UN01013252",
                    "unece:cefactBieDomainClass": "cefact:FinancingSummary_Document.Details",
                    "rdfs:comment": "The creditor financial account, used for crediting, specified for this financing summary document."
                }
            ]
        },
        {
            "@id": "core:specifiedFinancialInstitution",
            "@type": "rdf:Property",
            "schema:rangeIncludes": {
                "@id": "core:FinancialInstitution"
            },
            "schema:domainIncludes": [
                {
                    "@id": "core:TradeParty"
                },
                {
                    "@id": "core:TradeSettlementPaymentMeans"
                }
            ],
            "rdfs:comment": [
                "A creditor financial institution specified for this trade party.",
                "A financial institution specified for this trade settlement payment means."
            ],
            "rdfs:label": "specifiedFinancialInstitution",
            "unece:cefactElementMetadata": [
                {
                    "@id": "cefact:TradeSettlement_PaymentMeans.Specified.Payment_FinancialInstitution",
                    "@type": "unece:AssociationBIE",
                    "unece:cefactUNId": "UN01015458",
                    "unece:cefactBieDomainClass": "cefact:TradeSettlement_PaymentMeans.Details",
                    "rdfs:comment": "A financial institution specified for this trade settlement payment means."
                },
                {
                    "@id": "cefact:Trade_Party.Specified.Creditor_FinancialInstitution",
                    "@type": "unece:AssociationBIE",
                    "unece:cefactUNId": "UN01013664",
                    "unece:cefactBieDomainClass": "cefact:Trade_Party.Details",
                    "rdfs:comment": "A creditor financial institution specified for this trade party."
                }
            ]
        },
        {
            "@id": "core:specifiedIdentity",
            "@type": "rdf:Property",
            "schema:rangeIncludes": {
                "@id": "core:Identity"
            },
            "schema:domainIncludes": [
                {
                    "@id": "accounting:CreditorFinancialInstitution"
                },
                {
                    "@id": "core:PersonIdentity"
                },
                {
                    "@id": ":RequestingParty"
                },
                {
                    "@id": "core:TradeParty"
                }
            ],
            "rdfs:comment": [
                "A proprietary Identity specified for this person.",
                "A proprietary identity specified for this creditor financial institution.",
                "A proprietary identity specified for this requesting party.",
                "A proprietary identity specified for this trade party.",
                "The financial identity specified for this trade party."
            ],
            "rdfs:label": "specifiedIdentity",
            "unece:cefactElementMetadata": [
                {
                    "@id": "cefact:Trade_Party.Specified.Financial_Identity",
                    "@type": "unece:AssociationBIE",
                    "unece:cefactUNId": "UN01013303",
                    "unece:cefactBieDomainClass": "cefact:Trade_Party.Details",
                    "rdfs:comment": "The financial identity specified for this trade party."
                },
                {
                    "@id": "cefact:Person_Identity.Specified.Proprietary_Identity",
                    "@type": "unece:AssociationBIE",
                    "unece:cefactUNId": "UN01013285",
                    "unece:cefactBieDomainClass": "cefact:Person_Identity.Details",
                    "rdfs:comment": "A proprietary Identity specified for this person."
                },
                {
                    "@id": "cefact:Creditor_FinancialInstitution.Specified.Proprietary_Identity",
                    "@type": "unece:AssociationBIE",
                    "unece:cefactUNId": "UN01013210",
                    "unece:cefactBieDomainClass": "cefact:Creditor_FinancialInstitution.Details",
                    "rdfs:comment": "A proprietary identity specified for this creditor financial institution."
                },
                {
                    "@id": "cefact:Requesting_Party.Specified.Proprietary_Identity",
                    "@type": "unece:AssociationBIE",
                    "unece:cefactUNId": "UN01013292",
                    "unece:cefactBieDomainClass": "cefact:Requesting_Party.Details",
                    "rdfs:comment": "A proprietary identity specified for this requesting party."
                },
                {
                    "@id": "cefact:Trade_Party.Specified.Proprietary_Identity",
                    "@type": "unece:AssociationBIE",
                    "unece:cefactUNId": "UN01013302",
                    "unece:cefactBieDomainClass": "cefact:Trade_Party.Details",
                    "rdfs:comment": "A proprietary identity specified for this trade party."
                }
            ]
        },
        {
            "@id": "core:specifiedLocation",
            "@type": "rdf:Property",
            "schema:rangeIncludes": {
                "@id": "core:Location"
            },
            "schema:domainIncludes": [
                {
                    "@id": ":LocationParty"
                },
                {
                    "@id": "core:TradeParty"
                }
            ],
            "rdfs:comment": [
                "A logistics location or place specified for this party.",
                "A logistics related location or place specified for this trade party."
            ],
            "rdfs:label": "specifiedLocation",
            "unece:cefactElementMetadata": [
                {
                    "@id": "cefact:Trade_Party.Specified.Logistics_Location",
                    "@type": "unece:AssociationBIE",
                    "unece:cefactUNId": "UN01004610",
                    "unece:cefactBieDomainClass": "cefact:Trade_Party.Details",
                    "rdfs:comment": "A logistics related location or place specified for this trade party."
                },
                {
                    "@id": "cefact:Location_Party.Specified.Logistics_Location",
                    "@type": "unece:AssociationBIE",
                    "unece:cefactUNId": "UN01010091",
                    "unece:cefactBieDomainClass": "cefact:Location_Party.Details",
                    "rdfs:comment": "A logistics location or place specified for this party."
                }
            ]
        },
        {
            "@id": "core:specifiedNote",
            "@type": "rdf:Property",
            "schema:rangeIncludes": {
                "@id": "core:Note"
            },
            "schema:domainIncludes": {
                "@id": ":TradeContact"
            },
            "rdfs:comment": "A note specified for this trade contact.",
            "rdfs:label": "specifiedNote",
            "unece:cefactElementMetadata": [
                {
                    "@id": "cefact:Trade_Contact.Specified.Note",
                    "@type": "unece:AssociationBIE",
                    "unece:cefactUNId": "UN01004573",
                    "unece:cefactBieDomainClass": "cefact:Trade_Contact.Details",
                    "rdfs:comment": "A note specified for this trade contact."
                }
            ]
        },
        {
            "@id": "core:specifiedOrganization",
            "@type": "rdf:Property",
            "schema:rangeIncludes": {
                "@id": "core:Organization"
            },
            "schema:domainIncludes": {
                "@id": "core:TradeParty"
            },
            "rdfs:comment": "The legally constituted organization specified for this trade party.",
            "rdfs:label": "specifiedOrganization",
            "unece:cefactElementMetadata": [
                {
                    "@id": "cefact:Trade_Party.Specified.Legal_Organization",
                    "@type": "unece:AssociationBIE",
                    "unece:cefactUNId": "UN01004601",
                    "unece:cefactBieDomainClass": "cefact:Trade_Party.Details",
                    "rdfs:comment": "The legally constituted organization specified for this trade party."
                }
            ]
        },
        {
            "@id": "core:specifiedParty",
            "@type": "rdf:Property",
            "schema:rangeIncludes": {
                "@id": "core:Party"
            },
            "schema:domainIncludes": {
                "@id": "core:FinancingRequestDocument"
            },
            "rdfs:comment": "The requesting party specified in this financing request document.",
            "rdfs:label": "specifiedParty",
            "unece:cefactElementMetadata": [
                {
                    "@id": "cefact:FinancingRequest_Document.Specified.Requesting_Party",
                    "@type": "unece:AssociationBIE",
                    "unece:cefactUNId": "UN01013240",
                    "unece:cefactBieDomainClass": "cefact:FinancingRequest_Document.Details",
                    "rdfs:comment": "The requesting party specified in this financing request document."
                }
            ]
        },
        {
            "@id": "core:specifiedPerson",
            "@type": "rdf:Property",
            "schema:rangeIncludes": {
                "@id": "core:Person"
            },
            "schema:domainIncludes": {
                "@id": "core:TradeParty"
            },
            "rdfs:comment": [
                "A contact person specified for this trade party.",
                "A person specified to sign on behalf of this trade party.",
                "The specified representative person for this trade party."
            ],
            "rdfs:label": "specifiedPerson",
            "unece:cefactElementMetadata": [
                {
                    "@id": "cefact:Trade_Party.Specified.Contact_Person",
                    "@type": "unece:AssociationBIE",
                    "unece:cefactUNId": "UN01013301",
                    "unece:cefactBieDomainClass": "cefact:Trade_Party.Details",
                    "rdfs:comment": "A contact person specified for this trade party."
                },
                {
                    "@id": "cefact:Trade_Party.Specified.AuthoritativeSignatory_Person",
                    "@type": "unece:AssociationBIE",
                    "unece:cefactUNId": "UN01006142",
                    "unece:cefactBieDomainClass": "cefact:Trade_Party.Details",
                    "rdfs:comment": "A person specified to sign on behalf of this trade party."
                },
                {
                    "@id": "cefact:Trade_Party.Specified.Representative_Person",
                    "@type": "unece:AssociationBIE",
                    "unece:cefactUNId": "UN01004612",
                    "unece:cefactBieDomainClass": "cefact:Trade_Party.Details",
                    "rdfs:comment": "The specified representative person for this trade party."
                }
            ]
        },
        {
            "@id": "core:specifiedProduct",
            "@type": "rdf:Property",
            "schema:rangeIncludes": {
                "@id": "core:Product"
            },
            "schema:domainIncludes": {
                "@id": "core:TradeParty"
            },
            "rdfs:comment": "A product specified for this trade party.",
            "rdfs:label": "specifiedProduct",
            "unece:cefactElementMetadata": [
                {
                    "@id": "cefact:Trade_Party.Specified.Trade_Product",
                    "@type": "unece:AssociationBIE",
                    "unece:cefactUNId": "UN01014544",
                    "unece:cefactBieDomainClass": "cefact:Trade_Party.Details",
                    "rdfs:comment": "A product specified for this trade party."
                }
            ]
        },
        {
            "@id": "core:specifiedQuantity",
            "@type": "rdf:Property",
            "schema:rangeIncludes": {
                "@id": "xsd:decimal"
            },
            "schema:domainIncludes": {
                "@id": ":TradeCountry"
            },
            "rdfs:comment": "A quantity specified for this trade country.",
            "rdfs:label": "specifiedQuantity",
            "unece:cefactElementMetadata": [
                {
                    "@id": "cefact:Trade_Country.Specified.Quantity",
                    "@type": "unece:BasicBIE",
                    "unece:cefactUNId": "UN01010145",
                    "unece:cefactBieDomainClass": "cefact:Trade_Country.Details",
                    "rdfs:comment": "A quantity specified for this trade country."
                }
            ]
        },
        {
            "@id": "core:specifiedRegistration",
            "@type": "rdf:Property",
            "schema:rangeIncludes": {
                "@id": "core:Registration"
            },
            "schema:domainIncludes": {
                "@id": "core:TradeParty"
            },
            "rdfs:comment": [
                "A governmental registration specified for this trade party.",
                "A tax registration specified for this trade party."
            ],
            "rdfs:label": "specifiedRegistration",
            "unece:cefactElementMetadata": [
                {
                    "@id": "cefact:Trade_Party.Specified.Government_Registration",
                    "@type": "unece:AssociationBIE",
                    "unece:cefactUNId": "UN01011071",
                    "unece:cefactBieDomainClass": "cefact:Trade_Party.Details",
                    "rdfs:comment": "A governmental registration specified for this trade party."
                },
                {
                    "@id": "cefact:Trade_Party.Specified.Tax_Registration",
                    "@type": "unece:AssociationBIE",
                    "unece:cefactUNId": "UN01004611",
                    "unece:cefactBieDomainClass": "cefact:Trade_Party.Details",
                    "rdfs:comment": "A tax registration specified for this trade party."
                }
            ]
        },
        {
            "@id": "core:specifiedRiskAnalysisResult",
            "@type": "rdf:Property",
            "schema:rangeIncludes": {
                "@id": "core:RiskAnalysisResult"
            },
            "schema:domainIncludes": {
                "@id": "core:TradeParty"
            },
            "rdfs:comment": "A result of a logistics risk analysis calculation specified for this trade party.",
            "rdfs:label": "specifiedRiskAnalysisResult",
            "unece:cefactElementMetadata": [
                {
                    "@id": "cefact:Trade_Party.Specified.Logistics_RiskAnalysisResult",
                    "@type": "unece:AssociationBIE",
                    "unece:cefactUNId": "UN01013054",
                    "unece:cefactBieDomainClass": "cefact:Trade_Party.Details",
                    "rdfs:comment": "A result of a logistics risk analysis calculation specified for this trade party."
                }
            ]
        },
        {
            "@id": "core:specifiedStatus",
            "@type": "rdf:Property",
            "schema:rangeIncludes": {
                "@id": "core:Status"
            },
            "schema:domainIncludes": [
                {
                    "@id": "core:FinancingRequestDocument"
                },
                {
                    "@id": "core:FinancingRequestResultDocument"
                }
            ],
            "rdfs:comment": [
                "A status of a cancellation specified for this financing request document, such as accepted.",
                "The financing status specified in this financing request result document.",
                "The status of the validation specified for this financing request document, such as error."
            ],
            "rdfs:label": "specifiedStatus",
            "unece:cefactElementMetadata": [
                {
                    "@id": "cefact:FinancingRequest_Document.Specified.Validation_Status",
                    "@type": "unece:AssociationBIE",
                    "unece:cefactUNId": "UN01013242",
                    "unece:cefactBieDomainClass": "cefact:FinancingRequest_Document.Details",
                    "rdfs:comment": "The status of the validation specified for this financing request document, such as error."
                },
                {
                    "@id": "cefact:FinancingRequestResult_Document.Specified.Financing_Status",
                    "@type": "unece:AssociationBIE",
                    "unece:cefactUNId": "UN01013227",
                    "unece:cefactBieDomainClass": "cefact:FinancingRequestResult_Document.Details",
                    "rdfs:comment": "The financing status specified in this financing request result document."
                },
                {
                    "@id": "cefact:FinancingRequest_Document.Specified.Cancellation_Status",
                    "@type": "unece:AssociationBIE",
                    "unece:cefactUNId": "UN01013241",
                    "unece:cefactBieDomainClass": "cefact:FinancingRequest_Document.Details",
                    "rdfs:comment": "A status of a cancellation specified for this financing request document, such as accepted."
                }
            ]
        },
        {
            "@id": "core:status",
            "@type": "rdf:Property",
            "schema:rangeIncludes": {
                "@id": "xsd:string"
            },
            "schema:domainIncludes": {
                "@id": ":AcknowledgementDocument"
            },
            "rdfs:comment": "A status, expressed as text, for this acknowledgement document.",
            "rdfs:label": "status",
            "unece:cefactElementMetadata": [
                {
                    "@id": "cefact:Acknowledgement_Document.Status.Text",
                    "@type": "unece:BasicBIE",
                    "unece:cefactUNId": "UN01014633",
                    "unece:cefactBieDomainClass": "cefact:Acknowledgement_Document.Details",
                    "rdfs:comment": "A status, expressed as text, for this acknowledgement document."
                }
            ]
        },
        {
            "@id": "core:stayPeriod",
            "@type": "rdf:Property",
            "schema:rangeIncludes": {
                "@id": "core:Period"
            },
            "schema:domainIncludes": {
                "@id": "core:LogisticsLocation"
            },
            "rdfs:comment": "A period of stay at this logistics location.",
            "rdfs:label": "stayPeriod",
            "unece:cefactElementMetadata": [
                {
                    "@id": "cefact:Logistics_Location.Stay.Specified_Period",
                    "@type": "unece:AssociationBIE",
                    "unece:cefactUNId": "UN01013166",
                    "unece:cefactBieDomainClass": "cefact:Logistics_Location.Details",
                    "rdfs:comment": "A period of stay at this logistics location."
                }
            ]
        },
        {
            "@id": "core:staySpecifiedEvent",
            "@type": "rdf:Property",
            "schema:rangeIncludes": {
                "@id": "core:Event"
            },
            "schema:domainIncludes": {
                "@id": ":TransportEvent"
            },
            "rdfs:comment": "A stay specified for this referenced transport event.",
            "rdfs:label": "staySpecifiedEvent",
            "unece:cefactElementMetadata": [
                {
                    "@id": "cefact:Transport_Event.Stay_Specified.Referenced_Transport_Event",
                    "@type": "unece:AssociationBIE",
                    "unece:cefactUNId": "UN01010154",
                    "unece:cefactBieDomainClass": "cefact:Transport_Event.Details",
                    "rdfs:comment": "A stay specified for this referenced transport event."
                }
            ]
        },
        {
            "@id": "core:streetName",
            "@type": "rdf:Property",
            "schema:rangeIncludes": {
                "@id": "xsd:string"
            },
            "schema:domainIncludes": {
                "@id": "core:TradeAddress"
            },
            "rdfs:comment": "A name, expressed as text, of a street or thoroughfare for this trade address.",
            "rdfs:label": "streetName",
            "unece:cefactElementMetadata": [
                {
                    "@id": "cefact:Trade_Address.StreetName.Text",
                    "@type": "unece:BasicBIE",
                    "unece:cefactUNId": "UN01004543",
                    "unece:cefactBieDomainClass": "cefact:Trade_Address.Details",
                    "rdfs:comment": "A name, expressed as text, of a street or thoroughfare for this trade address."
                }
            ]
        },
        {
            "@id": "core:subcontractorParty",
            "@type": "rdf:Property",
            "schema:rangeIncludes": {
                "@id": "core:Party"
            },
            "schema:domainIncludes": {
                "@id": "core:TradeParty"
            },
            "rdfs:comment": "A subcontractor for this trade party.",
            "rdfs:label": "subcontractorParty",
            "unece:cefactElementMetadata": [
                {
                    "@id": "cefact:Trade_Party.Subcontractor.Trade_Party",
                    "@type": "unece:AssociationBIE",
                    "unece:cefactUNId": "UN01014534",
                    "unece:cefactBieDomainClass": "cefact:Trade_Party.Details",
                    "rdfs:comment": "A subcontractor for this trade party."
                }
            ]
        },
        {
            "@id": "core:subordinateLocation",
            "@type": "rdf:Property",
            "schema:rangeIncludes": {
                "@id": "core:Location"
            },
            "schema:domainIncludes": {
                "@id": "core:LogisticsLocation"
            },
            "rdfs:comment": "A location subordinate to this logistics related location.",
            "rdfs:label": "subordinateLocation",
            "unece:cefactElementMetadata": [
                {
                    "@id": "cefact:Logistics_Location.Subordinate.Subordinate_Location",
                    "@type": "unece:AssociationBIE",
                    "unece:cefactUNId": "UN01003687",
                    "unece:cefactBieDomainClass": "cefact:Logistics_Location.Details",
                    "rdfs:comment": "A location subordinate to this logistics related location."
                }
            ]
        },
        {
            "@id": "core:subordinateRelatedLocation",
            "@type": "rdf:Property",
            "schema:rangeIncludes": {
                "@id": "core:Location"
            },
            "schema:domainIncludes": {
                "@id": "core:LogisticsLocation"
            },
            "rdfs:comment": "A logistics location subordinate to this logistics location.",
            "rdfs:label": "subordinateRelatedLocation",
            "unece:cefactElementMetadata": [
                {
                    "@id": "cefact:Logistics_Location.Subordinate_Related.Logistics_Location",
                    "@type": "unece:AssociationBIE",
                    "unece:cefactUNId": "UN01014634",
                    "unece:cefactBieDomainClass": "cefact:Logistics_Location.Details",
                    "rdfs:comment": "A logistics location subordinate to this logistics location."
                }
            ]
        },
        {
            "@id": "core:subtypeCode",
            "@type": "rdf:Property",
            "schema:rangeIncludes": {
                "@id": "xsd:token"
            },
            "schema:domainIncludes": {
                "@id": ":ReferencedDocument"
            },
            "rdfs:comment": "A code specifying a subtype of this referenced document.",
            "rdfs:label": "subtypeCode",
            "unece:cefactElementMetadata": [
                {
                    "@id": "cefact:Referenced_Document.Subtype.Code",
                    "@type": "unece:BasicBIE",
                    "unece:cefactUNId": "UN01014905",
                    "unece:cefactBieDomainClass": "cefact:Referenced_Document.Details",
                    "rdfs:comment": "A code specifying a subtype of this referenced document."
                }
            ]
        },
        {
            "@id": "core:telephoneCommunication",
            "@type": "rdf:Property",
            "schema:rangeIncludes": {
                "@id": "core:Communication"
            },
            "schema:domainIncludes": [
                {
                    "@id": ":TradeContact"
                },
                {
                    "@id": "core:TradeParty"
                }
            ],
            "rdfs:comment": [
                "A telephone communication for this trade party.",
                "Telephone communication information for this trade contact."
            ],
            "rdfs:label": "telephoneCommunication",
            "unece:cefactElementMetadata": [
                {
                    "@id": "cefact:Trade_Contact.Telephone.Universal_Communication",
                    "@type": "unece:AssociationBIE",
                    "unece:cefactUNId": "UN01004564",
                    "unece:cefactBieDomainClass": "cefact:Trade_Contact.Details",
                    "rdfs:comment": "Telephone communication information for this trade contact."
                },
                {
                    "@id": "cefact:Trade_Party.Telephone.Universal_Communication",
                    "@type": "unece:AssociationBIE",
                    "unece:cefactUNId": "UN01004604",
                    "unece:cefactBieDomainClass": "cefact:Trade_Party.Details",
                    "rdfs:comment": "A telephone communication for this trade party."
                }
            ]
        },
        {
            "@id": "core:telexCommunication",
            "@type": "rdf:Property",
            "schema:rangeIncludes": {
                "@id": "core:Communication"
            },
            "schema:domainIncludes": {
                "@id": ":TradeContact"
            },
            "rdfs:comment": "Telegraphy (Telex) communication information for this trade contact.",
            "rdfs:label": "telexCommunication",
            "unece:cefactElementMetadata": [
                {
                    "@id": "cefact:Trade_Contact.Telex.Universal_Communication",
                    "@type": "unece:AssociationBIE",
                    "unece:cefactUNId": "UN01004570",
                    "unece:cefactBieDomainClass": "cefact:Trade_Contact.Details",
                    "rdfs:comment": "Telegraphy (Telex) communication information for this trade contact."
                }
            ]
        },
        {
            "@id": "core:timeOccurrenceDateTime",
            "@type": "rdf:Property",
            "schema:rangeIncludes": {
                "@id": "xsd:dateTime"
            },
            "schema:domainIncludes": {
                "@id": "core:SupplyChainEvent"
            },
            "rdfs:comment": "A time value of an occurrence of this supply chain event.",
            "rdfs:label": "timeOccurrenceDateTime",
            "unece:cefactElementMetadata": [
                {
                    "@id": "cefact:SupplyChain_Event.Time_Occurrence.DateTime",
                    "@type": "unece:BasicBIE",
                    "unece:TDED": "2193",
                    "unece:cefactUNId": "UN01012565",
                    "unece:cefactBieDomainClass": "cefact:SupplyChain_Event.Details",
                    "rdfs:comment": "A time value of an occurrence of this supply chain event."
                }
            ]
        },
        {
            "@id": "core:tradePaymentTermsDirectDebitMandateId",
            "@type": "rdf:Property",
            "schema:rangeIncludes": {
                "@id": "unece:UNECECL4277Code"
            },
            "schema:domainIncludes": {
                "@id": ":TradePaymentTerms"
            },
            "rdfs:comment": "An identifier of a direct debit mandate in these trade payment terms.",
            "rdfs:label": "tradePaymentTermsDirectDebitMandateId",
            "unece:cefactElementMetadata": [
                {
                    "@id": "cefact:Trade_PaymentTerms.DirectDebitMandate_Identification.Identifier",
                    "@type": "unece:BasicBIE",
                    "unece:TDED": "4277",
                    "unece:cefactUNId": "UN01006046",
                    "unece:cefactBieDomainClass": "cefact:Trade_PaymentTerms.Details",
                    "rdfs:comment": "An identifier of a direct debit mandate in these trade payment terms."
                }
            ]
        },
        {
            "@id": "core:tradePaymentTermsInstructionTypeCode",
            "@type": "rdf:Property",
            "schema:rangeIncludes": {
                "@id": "unece:UNECECL4279Code"
            },
            "schema:domainIncludes": {
                "@id": ":TradePaymentTerms"
            },
            "rdfs:comment": "A code specifying a type of instruction for these trade payment terms.",
            "rdfs:label": "tradePaymentTermsInstructionTypeCode",
            "unece:cefactElementMetadata": [
                {
                    "@id": "cefact:Trade_PaymentTerms.Instruction_Type.Code",
                    "@type": "unece:BasicBIE",
                    "unece:TDED": "4279",
                    "unece:cefactUNId": "UN01004638",
                    "unece:cefactBieDomainClass": "cefact:Trade_PaymentTerms.Details",
                    "rdfs:comment": "A code specifying a type of instruction for these trade payment terms."
                }
            ]
        },
        {
            "@id": "core:tradePaymentTermsPaymentMeansId",
            "@type": "rdf:Property",
            "schema:rangeIncludes": {
                "@id": "unece:UNECECL4277Code"
            },
            "schema:domainIncludes": {
                "@id": ":TradePaymentTerms"
            },
            "rdfs:comment": "An identifier of a payment means in these trade payment terms.",
            "rdfs:label": "tradePaymentTermsPaymentMeansId",
            "unece:cefactElementMetadata": [
                {
                    "@id": "cefact:Trade_PaymentTerms.PaymentMeans_Identification.Identifier",
                    "@type": "unece:BasicBIE",
                    "unece:TDED": "4277",
                    "unece:cefactUNId": "UN01006048",
                    "unece:cefactBieDomainClass": "cefact:Trade_PaymentTerms.Details",
                    "rdfs:comment": "An identifier of a payment means in these trade payment terms."
                }
            ]
        },
        {
            "@id": "core:tradeSettlementPaymentMeansId",
            "@type": "rdf:Property",
            "schema:rangeIncludes": {
                "@id": "unece:UNECECL4461Code"
            },
            "schema:domainIncludes": {
                "@id": "core:TradeSettlementPaymentMeans"
            },
            "rdfs:comment": "An identifier for this trade settlement payment means.",
            "rdfs:label": "tradeSettlementPaymentMeansId",
            "unece:cefactElementMetadata": [
                {
                    "@id": "cefact:TradeSettlement_PaymentMeans.Identification.Identifier",
                    "@type": "unece:BasicBIE",
                    "unece:TDED": "4461",
                    "unece:cefactUNId": "UN01006055",
                    "unece:cefactBieDomainClass": "cefact:TradeSettlement_PaymentMeans.Details",
                    "rdfs:comment": "An identifier for this trade settlement payment means."
                }
            ]
        },
        {
            "@id": "core:typeCode",
            "@type": "rdf:Property",
            "schema:rangeIncludes": {
                "@id": "xsd:token"
            },
            "schema:domainIncludes": [
                {
                    "@id": "core:SupplyChainEvent"
                },
                {
                    "@id": ":TradeCountrySubDivision"
                },
                {
                    "@id": "core:TradeGeopoliticalRegion"
                },
                {
                    "@id": "core:TradeParty"
                },
                {
                    "@id": "core:TradeSettlementFinancialCard"
                }
            ],
            "rdfs:comment": [
                "A code specifying a type of country sub-division for trade purposes.",
                "A code specifying the type of supply chain event.",
                "A code specifying the type of trade party that is independent of its role.",
                "The code specifying the type of this trade settlement financial card, such as debit or credit.",
                "The code specifying the type of trade geopolitical region."
            ],
            "rdfs:label": "typeCode",
            "unece:cefactElementMetadata": [
                {
                    "@id": "cefact:TradeSettlement_FinancialCard.Type.Code",
                    "@type": "unece:BasicBIE",
                    "unece:cefactUNId": "UN01004496",
                    "unece:cefactBieDomainClass": "cefact:TradeSettlement_FinancialCard.Details",
                    "rdfs:comment": "The code specifying the type of this trade settlement financial card, such as debit or credit."
                },
                {
                    "@id": "cefact:Trade_CountrySub-Division.Type.Code",
                    "@type": "unece:BasicBIE",
                    "unece:cefactUNId": "UN01004574",
                    "unece:cefactBieDomainClass": "cefact:Trade_CountrySubDivision.Details",
                    "rdfs:comment": "A code specifying a type of country sub-division for trade purposes."
                },
                {
                    "@id": "cefact:SupplyChain_Event.Type.Code",
                    "@type": "unece:BasicBIE",
                    "unece:TDED": "9171",
                    "unece:cefactUNId": "UN01004294",
                    "unece:cefactBieDomainClass": "cefact:SupplyChain_Event.Details",
                    "rdfs:comment": "A code specifying the type of supply chain event."
                },
                {
                    "@id": "cefact:Trade_GeopoliticalRegion.Type.Code",
                    "@type": "unece:BasicBIE",
                    "unece:cefactUNId": "UN01004589",
                    "unece:cefactBieDomainClass": "cefact:Trade_GeopoliticalRegion.Details",
                    "rdfs:comment": "The code specifying the type of trade geopolitical region."
                },
                {
                    "@id": "cefact:Trade_Party.Type.Code",
                    "@type": "unece:BasicBIE",
                    "unece:cefactUNId": "UN01004597",
                    "unece:cefactBieDomainClass": "cefact:Trade_Party.Details",
                    "rdfs:comment": "A code specifying the type of trade party that is independent of its role."
                }
            ]
        },
        {
            "@id": "core:uPICId",
            "@type": "rdf:Property",
            "schema:rangeIncludes": {
                "@id": "xsd:token"
            },
            "schema:domainIncludes": {
                "@id": "core:FinancingFinancialAccount"
            },
            "rdfs:comment": "The unique Universal Payment Identification Code (UPIC) identifier used by the New York Clearing House for this financing financial account.",
            "rdfs:label": "uPICId",
            "unece:cefactElementMetadata": [
                {
                    "@id": "cefact:Financing_FinancialAccount.UPIC_Identification.Identifier",
                    "@type": "unece:BasicBIE",
                    "unece:TDED": "3492",
                    "unece:cefactUNId": "UN01013256",
                    "unece:cefactBieDomainClass": "cefact:Financing_FinancialAccount.Details",
                    "rdfs:comment": "The unique Universal Payment Identification Code (UPIC) identifier used by the New York Clearing House for this financing financial account."
                }
            ]
        },
        {
            "@id": "core:uRICommunication",
            "@type": "rdf:Property",
            "schema:rangeIncludes": {
                "@id": "core:Communication"
            },
            "schema:domainIncludes": [
                {
                    "@id": ":TradeContact"
                },
                {
                    "@id": "core:TradeParty"
                }
            ],
            "rdfs:comment": [
                "A Uniform Resource Identifier (URI) communication for this trade party, such as a web or email address.",
                "Uniform Resource Identifier (URI) communication information for this trade contact, such as a web or an email address."
            ],
            "rdfs:label": "uRICommunication",
            "unece:cefactElementMetadata": [
                {
                    "@id": "cefact:Trade_Party.URI.Universal_Communication",
                    "@type": "unece:AssociationBIE",
                    "unece:cefactUNId": "UN01004606",
                    "unece:cefactBieDomainClass": "cefact:Trade_Party.Details",
                    "rdfs:comment": "A Uniform Resource Identifier (URI) communication for this trade party, such as a web or email address."
                },
                {
                    "@id": "cefact:Trade_Contact.URI.Universal_Communication",
                    "@type": "unece:AssociationBIE",
                    "unece:cefactUNId": "UN01004568",
                    "unece:cefactBieDomainClass": "cefact:Trade_Contact.Details",
                    "rdfs:comment": "Uniform Resource Identifier (URI) communication information for this trade contact, such as a web or an email address."
                }
            ]
        },
        {
            "@id": "core:uTCOffsetNumeric",
            "@type": "rdf:Property",
            "schema:rangeIncludes": {
                "@id": "xsd:decimal"
            },
            "schema:domainIncludes": {
                "@id": "core:LogisticsLocation"
            },
            "rdfs:comment": "The time offset value from the Universal Time Coordinate (UTC) for this logistics related location.",
            "rdfs:label": "uTCOffsetNumeric",
            "unece:cefactElementMetadata": [
                {
                    "@id": "cefact:Logistics_Location.UTCOffset.Numeric",
                    "@type": "unece:BasicBIE",
                    "unece:cefactUNId": "UN01003684",
                    "unece:cefactBieDomainClass": "cefact:Logistics_Location.Details",
                    "rdfs:comment": "The time offset value from the Universal Time Coordinate (UTC) for this logistics related location."
                }
            ]
        },
        {
            "@id": "core:unitQuantity",
            "@type": "rdf:Property",
            "schema:rangeIncludes": {
                "@id": "xsd:decimal"
            },
            "schema:domainIncludes": [
                {
                    "@id": "core:SupplyChainEvent"
                },
                {
                    "@id": ":TransportEvent"
                }
            ],
            "rdfs:comment": [
                "A number of units for this supply chain event.",
                "The number of units for this transport event."
            ],
            "rdfs:label": "unitQuantity",
            "unece:cefactElementMetadata": [
                {
                    "@id": "cefact:SupplyChain_Event.Unit.Quantity",
                    "@type": "unece:BasicBIE",
                    "unece:cefactUNId": "UN01004297",
                    "unece:cefactBieDomainClass": "cefact:SupplyChain_Event.Details",
                    "rdfs:comment": "A number of units for this supply chain event."
                },
                {
                    "@id": "cefact:Transport_Event.Unit.Quantity",
                    "@type": "unece:BasicBIE",
                    "unece:cefactUNId": "UN01006146",
                    "unece:cefactBieDomainClass": "cefact:Transport_Event.Details",
                    "rdfs:comment": "The number of units for this transport event."
                }
            ]
        },
        {
            "@id": "core:vOIPCommunication",
            "@type": "rdf:Property",
            "schema:rangeIncludes": {
                "@id": "core:Communication"
            },
            "schema:domainIncludes": {
                "@id": ":TradeContact"
            },
            "rdfs:comment": "Voice Over Internet Protocol (VOIP) communication information for this trade contact.",
            "rdfs:label": "vOIPCommunication",
            "unece:cefactElementMetadata": [
                {
                    "@id": "cefact:Trade_Contact.VOIP.Universal_Communication",
                    "@type": "unece:AssociationBIE",
                    "unece:cefactUNId": "UN01004571",
                    "unece:cefactBieDomainClass": "cefact:Trade_Contact.Details",
                    "rdfs:comment": "Voice Over Internet Protocol (VOIP) communication information for this trade contact."
                }
            ]
        },
        {
            "@id": "core:validFromDateTime",
            "@type": "rdf:Property",
            "schema:rangeIncludes": {
                "@id": "xsd:dateTime"
            },
            "schema:domainIncludes": {
                "@id": "core:TradeSettlementFinancialCard"
            },
            "rdfs:comment": "The date from which this trade settlement financial card is valid.",
            "rdfs:label": "validFromDateTime",
            "unece:cefactElementMetadata": [
                {
                    "@id": "cefact:TradeSettlement_FinancialCard.ValidFrom.DateTime",
                    "@type": "unece:BasicBIE",
                    "unece:cefactUNId": "UN01004500",
                    "unece:cefactBieDomainClass": "cefact:TradeSettlement_FinancialCard.Details",
                    "rdfs:comment": "The date from which this trade settlement financial card is valid."
                }
            ]
        },
        {
            "@id": "core:valueMeasure",
            "@type": "rdf:Property",
            "schema:rangeIncludes": {
                "@id": "xsd:decimal"
            },
            "schema:domainIncludes": {
                "@id": ":TransportEvent"
            },
            "rdfs:comment": "The measure of a value for this transport event.",
            "rdfs:label": "valueMeasure",
            "unece:cefactElementMetadata": [
                {
                    "@id": "cefact:Transport_Event.Value.Measure",
                    "@type": "unece:BasicBIE",
                    "unece:cefactUNId": "UN01013583",
                    "unece:cefactBieDomainClass": "cefact:Transport_Event.Details",
                    "rdfs:comment": "The measure of a value for this transport event."
                }
            ]
        },
        {
            "@id": "core:verificationNumeric",
            "@type": "rdf:Property",
            "schema:rangeIncludes": {
                "@id": "xsd:decimal"
            },
            "schema:domainIncludes": {
                "@id": "core:TradeSettlementFinancialCard"
            },
            "rdfs:comment": "The unique card verification number for security purposes to help verify the card user is in actual possession of this trade settlement financial card.",
            "rdfs:label": "verificationNumeric",
            "unece:cefactElementMetadata": [
                {
                    "@id": "cefact:TradeSettlement_FinancialCard.Verification.Numeric",
                    "@type": "unece:BasicBIE",
                    "unece:cefactUNId": "UN01004499",
                    "unece:cefactBieDomainClass": "cefact:TradeSettlement_FinancialCard.Details",
                    "rdfs:comment": "The unique card verification number for security purposes to help verify the card user is in actual possession of this trade settlement financial card."
                }
            ]
        }
    ]
}